remove modules we don't need. remove two clauses of GoodVar

examples/ghc/lib/Literal.v
@@ -18,19 +18,14 @@ Require GHC.Nat.
 
 Require AxiomatizedTypes.
 Require BasicTypes.
-Require Data.Maybe.
 Require DynFlags.
 Require FastString.
 Require GHC.Base.
 Require GHC.Char.
-Require GHC.Enum.
 Require GHC.Err.
 Require GHC.Num.
 Require GHC.Real.
-Require Panic.
 Require UniqFM.
-Import GHC.Base.Notations.
-Import GHC.Num.Notations.
 
 (* Converted type declarations: *)
 
@@ -53,267 +48,74 @@ Instance Default__Literal : GHC.Err.Default Literal :=
 
 (* Converted value declarations: *)
 
-Definition word2IntLit : DynFlags.DynFlags -> Literal -> Literal :=
-  fun arg_0__ arg_1__ =>
-    match arg_0__, arg_1__ with
-    | dflags, MachWord w =>
-        if w GHC.Base.> DynFlags.tARGET_MAX_INT dflags : bool
-        then MachInt ((w GHC.Num.- DynFlags.tARGET_MAX_WORD dflags) GHC.Num.- #1) else
-        MachInt w
-    | _, _ =>
-        match arg_0__, arg_1__ with
-        | _, l => Panic.panicStr (GHC.Base.hs_string__ "word2IntLit") (Panic.someSDoc)
-        end
-    end.
+Axiom word2IntLit : DynFlags.DynFlags -> Literal -> Literal.
 
-Definition nullAddrLit : Literal :=
-  MachNullAddr.
+Axiom nullAddrLit : Literal.
 
-Definition mkMachString : GHC.Base.String -> Literal :=
-  fun s =>
-    MachStr (FastString.fastStringToByteString (FastString.mkFastString s)).
+Axiom mkMachString : GHC.Base.String -> Literal.
 
-Definition mkMachFloat : GHC.Real.Rational -> Literal :=
-  MachFloat.
+Axiom mkMachFloat : GHC.Real.Rational -> Literal.
 
-Definition mkMachDouble : GHC.Real.Rational -> Literal :=
-  MachDouble.
+Axiom mkMachDouble : GHC.Real.Rational -> Literal.
 
-Definition mkMachChar : GHC.Char.Char -> Literal :=
-  MachChar.
+Axiom mkMachChar : GHC.Char.Char -> Literal.
 
-Definition mkLitInteger
-   : GHC.Num.Integer -> AxiomatizedTypes.Type_ -> Literal :=
-  LitInteger.
+Axiom mkLitInteger : GHC.Num.Integer -> AxiomatizedTypes.Type_ -> Literal.
 
-Definition litTag : Literal -> nat :=
-  fun arg_0__ =>
-    match arg_0__ with
-    | MachChar _ => #1
-    | MachStr _ => #2
-    | MachNullAddr => #3
-    | MachInt _ => #4
-    | MachWord _ => #5
-    | MachInt64 _ => #6
-    | MachWord64 _ => #7
-    | MachFloat _ => #8
-    | MachDouble _ => #9
-    | MachLabel _ _ _ => #10
-    | LitInteger _ _ => #11
-    end.
+Axiom literalType : Literal -> AxiomatizedTypes.Type_.
 
-Definition litIsTrivial : Literal -> bool :=
-  fun arg_0__ =>
-    match arg_0__ with
-    | MachStr _ => false
-    | LitInteger _ _ => false
-    | _ => true
-    end.
+Axiom litValue : Literal -> GHC.Num.Integer.
 
-Definition litIsLifted : Literal -> bool :=
-  fun arg_0__ => match arg_0__ with | LitInteger _ _ => true | _ => false end.
+Axiom litTag : Literal -> nat.
 
-Definition litFitsInChar : Literal -> bool :=
-  fun arg_0__ =>
-    match arg_0__ with
-    | MachInt i =>
-        andb (i GHC.Base.>= GHC.Real.toInteger (GHC.Base.ord GHC.Enum.minBound)) (i
-              GHC.Base.<=
-              GHC.Real.toInteger (GHC.Base.ord GHC.Enum.maxBound))
-    | _ => false
-    end.
+Axiom litIsTrivial : Literal -> bool.
 
-Definition isZeroLit : Literal -> bool :=
-  fun arg_0__ =>
-    match arg_0__ with
-    | MachInt num_1__ => if num_1__ GHC.Base.== #0 : bool then true else false
-    | MachInt64 num_2__ => if num_2__ GHC.Base.== #0 : bool then true else false
-    | MachWord num_3__ => if num_3__ GHC.Base.== #0 : bool then true else false
-    | MachWord64 num_4__ => if num_4__ GHC.Base.== #0 : bool then true else false
-    | MachFloat num_5__ => if num_5__ GHC.Base.== #0 : bool then true else false
-    | MachDouble num_6__ => if num_6__ GHC.Base.== #0 : bool then true else false
-    | _ => false
-    end.
+Axiom litIsLifted : Literal -> bool.
 
-Definition isLitValue_maybe : Literal -> option GHC.Num.Integer :=
-  fun arg_0__ =>
-    match arg_0__ with
-    | MachChar c => Some (GHC.Real.toInteger (GHC.Base.ord c))
-    | MachInt i => Some i
-    | MachInt64 i => Some i
-    | MachWord i => Some i
-    | MachWord64 i => Some i
-    | LitInteger i _ => Some i
-    | _ => None
-    end.
+Axiom litIsDupable : DynFlags.DynFlags -> Literal -> bool.
 
-Definition litValue : Literal -> GHC.Num.Integer :=
-  fun l =>
-    match isLitValue_maybe l with
-    | Some x => x
-    | None => Panic.panicStr (GHC.Base.hs_string__ "litValue") (Panic.someSDoc)
-    end.
+Axiom litFitsInChar : Literal -> bool.
 
-Definition isLitValue : Literal -> bool :=
-  Data.Maybe.isJust GHC.Base.∘ isLitValue_maybe.
+Axiom isZeroLit : Literal -> bool.
 
-Definition int2WordLit : DynFlags.DynFlags -> Literal -> Literal :=
-  fun arg_0__ arg_1__ =>
-    match arg_0__, arg_1__ with
-    | dflags, MachInt i =>
-        if i GHC.Base.< #0 : bool
-        then MachWord ((#1 GHC.Num.+ DynFlags.tARGET_MAX_WORD dflags) GHC.Num.+ i) else
-        MachWord i
-    | _, _ =>
-        match arg_0__, arg_1__ with
-        | _, l => Panic.panicStr (GHC.Base.hs_string__ "int2WordLit") (Panic.someSDoc)
-        end
-    end.
+Axiom isLitValue_maybe : Literal -> option GHC.Num.Integer.
 
-Definition int2FloatLit : Literal -> Literal :=
-  fun arg_0__ =>
-    match arg_0__ with
-    | MachInt i => MachFloat (GHC.Num.fromInteger i)
-    | l => Panic.panicStr (GHC.Base.hs_string__ "int2FloatLit") (Panic.someSDoc)
-    end.
+Axiom isLitValue : Literal -> bool.
 
-Definition int2DoubleLit : Literal -> Literal :=
-  fun arg_0__ =>
-    match arg_0__ with
-    | MachInt i => MachDouble (GHC.Num.fromInteger i)
-    | l => Panic.panicStr (GHC.Base.hs_string__ "int2DoubleLit") (Panic.someSDoc)
-    end.
+Axiom int2WordLit : DynFlags.DynFlags -> Literal -> Literal.
 
-Definition int2CharLit : Literal -> Literal :=
-  fun arg_0__ =>
-    match arg_0__ with
-    | MachInt i => MachChar (GHC.Char.chr (GHC.Num.fromInteger i))
-    | l => Panic.panicStr (GHC.Base.hs_string__ "int2CharLit") (Panic.someSDoc)
-    end.
+Axiom int2FloatLit : Literal -> Literal.
 
-Definition inWordRange : DynFlags.DynFlags -> GHC.Num.Integer -> bool :=
-  fun dflags x =>
-    andb (x GHC.Base.>= #0) (x GHC.Base.<= DynFlags.tARGET_MAX_WORD dflags).
+Axiom int2DoubleLit : Literal -> Literal.
 
-Definition inIntRange : DynFlags.DynFlags -> GHC.Num.Integer -> bool :=
-  fun dflags x =>
-    andb (x GHC.Base.>= DynFlags.tARGET_MIN_INT dflags) (x GHC.Base.<=
-          DynFlags.tARGET_MAX_INT dflags).
+Axiom int2CharLit : Literal -> Literal.
 
-Definition litIsDupable : DynFlags.DynFlags -> Literal -> bool :=
-  fun arg_0__ arg_1__ =>
-    match arg_0__, arg_1__ with
-    | _, MachStr _ => false
-    | dflags, LitInteger i _ => inIntRange dflags i
-    | _, _ => true
-    end.
+Axiom inWordRange : DynFlags.DynFlags -> GHC.Num.Integer -> bool.
+
+Axiom inIntRange : DynFlags.DynFlags -> GHC.Num.Integer -> bool.
 
 Axiom inCharRange : GHC.Char.Char -> bool.
 
-Definition float2DoubleLit : Literal -> Literal :=
-  fun arg_0__ =>
-    match arg_0__ with
-    | MachFloat f => MachDouble f
-    | l => Panic.panicStr (GHC.Base.hs_string__ "float2DoubleLit") (Panic.someSDoc)
-    end.
+Axiom float2DoubleLit : Literal -> Literal.
 
-Definition double2FloatLit : Literal -> Literal :=
-  fun arg_0__ =>
-    match arg_0__ with
-    | MachDouble d => MachFloat d
-    | l => Panic.panicStr (GHC.Base.hs_string__ "double2FloatLit") (Panic.someSDoc)
-    end.
+Axiom double2FloatLit : Literal -> Literal.
 
-Definition cmpLit : Literal -> Literal -> comparison :=
-  fun arg_0__ arg_1__ =>
-    match arg_0__, arg_1__ with
-    | MachChar a, MachChar b => GHC.Base.compare a b
-    | MachStr a, MachStr b => GHC.Base.compare a b
-    | MachNullAddr, MachNullAddr => Eq
-    | MachInt a, MachInt b => GHC.Base.compare a b
-    | MachWord a, MachWord b => GHC.Base.compare a b
-    | MachInt64 a, MachInt64 b => GHC.Base.compare a b
-    | MachWord64 a, MachWord64 b => GHC.Base.compare a b
-    | MachFloat a, MachFloat b => GHC.Base.compare a b
-    | MachDouble a, MachDouble b => GHC.Base.compare a b
-    | MachLabel a _ _, MachLabel b _ _ => GHC.Base.compare a b
-    | LitInteger a _, LitInteger b _ => GHC.Base.compare a b
-    | lit1, lit2 => if litTag lit1 GHC.Base.< litTag lit2 : bool then Lt else Gt
-    end.
+Axiom cmpLit : Literal -> Literal -> comparison.
 
-Definition char2IntLit : Literal -> Literal :=
-  fun arg_0__ =>
-    match arg_0__ with
-    | MachChar c => MachInt (GHC.Real.toInteger (GHC.Base.ord c))
-    | l => Panic.panicStr (GHC.Base.hs_string__ "char2IntLit") (Panic.someSDoc)
-    end.
+Axiom char2IntLit : Literal -> Literal.
 
 Axiom absent_lits : UniqFM.UniqFM Literal.
 
 (* Skipping all instances of class `Data.Data.Data', including
    `Literal.Data__Literal' *)
 
-Local Definition Ord__Literal_compare : Literal -> Literal -> comparison :=
-  fun a b => cmpLit a b.
+Instance Eq___Literal : GHC.Base.Eq_ Literal := {}.
+Proof.
+Admitted.
 
-Local Definition Ord__Literal_op_zl__ : Literal -> Literal -> bool :=
-  fun a b =>
-    match (Ord__Literal_compare a b) with
-    | Lt => true
-    | Eq => false
-    | Gt => false
-    end.
-
-Local Definition Ord__Literal_op_zlze__ : Literal -> Literal -> bool :=
-  fun a b =>
-    match (Ord__Literal_compare a b) with
-    | Lt => true
-    | Eq => true
-    | Gt => false
-    end.
-
-Local Definition Ord__Literal_op_zg__ : Literal -> Literal -> bool :=
-  fun a b =>
-    match (Ord__Literal_compare a b) with
-    | Lt => false
-    | Eq => false
-    | Gt => true
-    end.
-
-Local Definition Ord__Literal_op_zgze__ : Literal -> Literal -> bool :=
-  fun a b =>
-    match (Ord__Literal_compare a b) with
-    | Lt => false
-    | Eq => true
-    | Gt => true
-    end.
-
-Local Definition Ord__Literal_max : Literal -> Literal -> Literal :=
-  fun x y => if Ord__Literal_op_zlze__ x y : bool then y else x.
-
-Local Definition Ord__Literal_min : Literal -> Literal -> Literal :=
-  fun x y => if Ord__Literal_op_zlze__ x y : bool then x else y.
-
-Local Definition Eq___Literal_op_zeze__ : Literal -> Literal -> bool :=
-  fun a b => match cmpLit a b with | Eq => true | _ => false end.
-
-Local Definition Eq___Literal_op_zsze__ : Literal -> Literal -> bool :=
-  fun a b => match cmpLit a b with | Eq => false | _ => true end.
-
-Program Instance Eq___Literal : GHC.Base.Eq_ Literal :=
-  fun _ k__ =>
-    k__ {| GHC.Base.op_zeze____ := Eq___Literal_op_zeze__ ;
-           GHC.Base.op_zsze____ := Eq___Literal_op_zsze__ |}.
-
-Program Instance Ord__Literal : GHC.Base.Ord Literal :=
-  fun _ k__ =>
-    k__ {| GHC.Base.op_zl____ := Ord__Literal_op_zl__ ;
-           GHC.Base.op_zlze____ := Ord__Literal_op_zlze__ ;
-           GHC.Base.op_zg____ := Ord__Literal_op_zg__ ;
-           GHC.Base.op_zgze____ := Ord__Literal_op_zgze__ ;
-           GHC.Base.compare__ := Ord__Literal_compare ;
-           GHC.Base.max__ := Ord__Literal_max ;
-           GHC.Base.min__ := Ord__Literal_min |}.
+Instance Ord__Literal : GHC.Base.Ord Literal := {}.
+Proof.
+Admitted.
 
 (* Skipping all instances of class `Outputable.Outputable', including
    `Literal.Outputable__Literal' *)
@@ -322,17 +124,8 @@ Program Instance Ord__Literal : GHC.Base.Ord Literal :=
    `Literal.Binary__Literal' *)
 
 (* External variables:
-     Eq Gt Lt None Some andb bool comparison false nat option true
-     AxiomatizedTypes.Type_ BasicTypes.FunctionOrData Data.Maybe.isJust
-     DynFlags.DynFlags DynFlags.tARGET_MAX_INT DynFlags.tARGET_MAX_WORD
-     DynFlags.tARGET_MIN_INT FastString.FastString FastString.fastStringToByteString
-     FastString.mkFastString GHC.Base.Eq_ GHC.Base.Ord GHC.Base.String
-     GHC.Base.compare GHC.Base.compare__ GHC.Base.max__ GHC.Base.min__
-     GHC.Base.op_z2218U__ GHC.Base.op_zeze__ GHC.Base.op_zeze____ GHC.Base.op_zg__
-     GHC.Base.op_zg____ GHC.Base.op_zgze__ GHC.Base.op_zgze____ GHC.Base.op_zl__
-     GHC.Base.op_zl____ GHC.Base.op_zlze__ GHC.Base.op_zlze____ GHC.Base.op_zsze____
-     GHC.Base.ord GHC.Char.Char GHC.Char.chr GHC.Enum.maxBound GHC.Enum.minBound
-     GHC.Err.Build_Default GHC.Err.Default GHC.Num.Integer GHC.Num.fromInteger
-     GHC.Num.op_zm__ GHC.Num.op_zp__ GHC.Real.Rational GHC.Real.toInteger
-     Panic.panicStr Panic.someSDoc UniqFM.UniqFM
+     bool comparison nat option AxiomatizedTypes.Type_ BasicTypes.FunctionOrData
+     DynFlags.DynFlags FastString.FastString GHC.Base.Eq_ GHC.Base.Ord
+     GHC.Base.String GHC.Char.Char GHC.Err.Build_Default GHC.Err.Default
+     GHC.Num.Integer GHC.Real.Rational UniqFM.UniqFM
 *)
