examples/ghc/lib/Core.v
@@ -17,9 +17,12 @@ Require Coq.Program.Wf.
 
 Require Import AxiomatizedTypes.
 Require BasicTypes.
+Require DynFlags.
 Require FastString.
+Require FieldLabel.
 Require GHC.Base.
 Require GHC.Num.
+Require Module.
 Require Name.
 Require OccName.
 Require Pair.
@@ -35,12 +38,8 @@ Require Coq.Init.Peano.
 Require Coq.Lists.List.
 Require Data.Foldable.
 Require Data.Function.
-Require Data.Maybe.
 Require Data.Tuple.
 Require Datatypes.
-Require DynFlags.
-Require FastStringEnv.
-Require FieldLabel.
 Require GHC.Char.
 Require GHC.DeferredFix.
 Require GHC.Err.
@@ -50,10 +49,8 @@ Require GHC.Real.
 Require GHC.Wf.
 Require Import Literal.
 Require Maybes.
-Require Module.
 Require NameEnv.
 Require Panic.
-Require PrelNames.
 Require SrcLoc.
 Require UniqDFM.
 Require UniqDSet.
@@ -2534,13 +2531,41 @@ Axiom zipCvSubst : list CoVar -> list Coercion -> TCvSubst.
 
 Axiom zipCoEnv : list CoVar -> list Coercion -> CvSubstEnv.
 
+Axiom zap_usg : KillFlags -> UseDmd -> UseDmd.
+
+Axiom zap_musg : KillFlags -> ArgUse -> ArgUse.
+
+Axiom zapUsedOnceSig : StrictSig -> StrictSig.
+
+Axiom zapUsedOnceDemand : Demand -> Demand.
+
+Axiom zapUsageEnvSig : StrictSig -> StrictSig.
+
+Axiom zapUsageDemand : Demand -> Demand.
+
 Axiom zapTCvSubst : TCvSubst -> TCvSubst.
 
 Axiom zapLiftingContext : LiftingContext -> LiftingContext.
 
+Axiom visibleDataCons : AlgTyConRhs -> list DataCon.
+
+Axiom vanillaCprProdRes : BasicTypes.Arity -> DmdResult.
+
 Axiom userTypeError_maybe : Type_ -> option Type_.
 
+Axiom useTop : ArgUse.
+
+Axiom useCount : forall {u}, Use u -> Count.
+
+Axiom useBot : ArgUse.
+
 Axiom unwrapNewTypeStepper : NormaliseStepper Coercion.
+
+Axiom unwrapNewTyCon_maybe : TyCon ->
+                             option (list TyVar * Type_ * CoAxiom Unbranched)%type.
+
+Axiom unwrapNewTyConEtad_maybe : TyCon ->
+                                 option (list TyVar * Type_ * CoAxiom Unbranched)%type.
 
 Axiom unionTCvSubst : TCvSubst -> TCvSubst -> TCvSubst.
 
@@ -2556,11 +2581,65 @@ Axiom tyThingCategory : TyThing -> GHC.Base.String.
 
 Axiom tyConsOfType : Type_ -> UniqSet.UniqSet TyCon.
 
+Axiom tyConVisibleTyVars : TyCon -> list TyVar.
+
+Axiom tyConTyVarBinders : list TyConBinder -> list TyVarBinder.
+
+Axiom tyConTuple_maybe : TyCon -> option BasicTypes.TupleSort.
+
+Axiom tyConStupidTheta : TyCon -> list PredType.
+
+Axiom tyConSingleDataCon_maybe : TyCon -> option DataCon.
+
+Axiom tyConSingleDataCon : TyCon -> DataCon.
+
+Axiom tyConSingleAlgDataCon_maybe : TyCon -> option DataCon.
+
 Axiom tyConRolesX : Role -> TyCon -> list Role.
 
 Axiom tyConRolesRepresentational : TyCon -> list Role.
 
+Axiom tyConRoles : TyCon -> list Role.
+
+Axiom tyConRepName_maybe : TyCon -> option TyConRepName.
+
+Axiom tyConRepModOcc : Module.Module ->
+                       OccName.OccName -> (Module.Module * OccName.OccName)%type.
+
+Axiom tyConInjectivityInfo : TyCon -> Injectivity.
+
+Axiom tyConFlavour : TyCon -> TyConFlavour.
+
+Axiom tyConFieldLabels : TyCon -> list FieldLabel.FieldLabel.
+
+Axiom tyConFieldLabelEnv : TyCon -> FieldLabel.FieldLabelEnv.
+
+Axiom tyConFamilySizeAtMost : TyCon -> nat -> bool.
+
+Axiom tyConFamilySize : TyCon -> nat.
+
+Axiom tyConFamilyResVar_maybe : TyCon -> option Name.Name.
+
+Axiom tyConFamilyCoercion_maybe : TyCon -> option (CoAxiom Unbranched).
+
+Axiom tyConFamInst_maybe : TyCon -> option (TyCon * list Type_)%type.
+
+Axiom tyConFamInstSig_maybe : TyCon ->
+                              option (TyCon * list Type_ * CoAxiom Unbranched)%type.
+
+Axiom tyConDataCons_maybe : TyCon -> option (list DataCon).
+
+Axiom tyConDataCons : TyCon -> list DataCon.
+
+Axiom tyConClass_maybe : TyCon -> option Class.
+
+Axiom tyConCType_maybe : TyCon -> option unit.
+
 Axiom tyConBindersTyBinders : list TyConBinder -> list TyBinder.
+
+Axiom tyConBinderArgFlag : TyConBinder -> ArgFlag.
+
+Axiom tyConAssoc_maybe : TyCon -> option Class.
 
 Axiom tyConAppTyCon_maybe : Type_ -> option TyCon.
 
@@ -2573,6 +2652,8 @@ Axiom tyConAppArgs_maybe : Type_ -> option (list Type_).
 Axiom tyConAppArgs : Type_ -> list Type_.
 
 Axiom tyConAppArgN : nat -> Type_ -> Type_.
+
+Axiom tyConATs : TyCon -> list TyCon.
 
 Axiom tyCoVarsOfTypesWellScoped : list Type_ -> list TyVar.
 
@@ -2606,14 +2687,24 @@ Axiom tyCoVarsOfCo : Coercion -> TyCoVarSet.
 
 Axiom tyBinderType : TyBinder -> Type_.
 
+Axiom trimCPRInfo : bool -> bool -> DmdResult -> DmdResult.
+
 Axiom toposortTyVars : list TyCoVar -> list TyCoVar.
+
+Axiom resTypeArgDmd : forall {r}, Termination r -> Demand.
+
+Axiom topRes : DmdResult.
 
 Axiom topNormaliseTypeX : forall {ev},
                           NormaliseStepper ev -> (ev -> ev -> ev) -> Type_ -> option (ev * Type_)%type.
 
 Axiom topNormaliseNewType_maybe : Type_ -> option (Coercion * Type_)%type.
 
+Axiom topDmd : Demand.
+
 Axiom toPhantomCo : Coercion -> Coercion.
+
+Axiom toBothDmdArg : DmdType -> BothDmdArg.
 
 Axiom tidyTypes : TidyEnv -> list Type_ -> list Type_.
 
@@ -2634,6 +2725,8 @@ Axiom tidyTyCoVarBndrs : TidyEnv ->
 Axiom tidyTyCoVarBndr : TidyEnv -> TyCoVar -> (TidyEnv * TyCoVar)%type.
 
 Axiom tidyTopType : Type_ -> Type_.
+
+Axiom tidyPatSynIds : (Id -> Id) -> PatSyn -> PatSyn.
 
 Axiom tidyOpenTypes : TidyEnv -> list Type_ -> (TidyEnv * list Type_)%type.
 
@@ -2664,7 +2757,15 @@ Axiom tcRepSplitTyConApp_maybe : forall `{Util.HasDebugCallStack},
 
 Axiom tcRepSplitAppTy_maybe : Type_ -> option (Type_ * Type_)%type.
 
+Axiom tcFlavourIsOpen : TyConFlavour -> bool.
+
+Axiom tcFlavourCanBeUnsaturated : TyConFlavour -> bool.
+
+Axiom synTyConRhs_maybe : TyCon -> option Type_.
+
 Axiom synTyConResKind : TyCon -> Kind.
+
+Axiom synTyConDefn_maybe : TyCon -> option (list TyVar * Type_)%type.
 
 Axiom swapLiftCoEnv : LiftCoEnv -> LiftCoEnv.
 
@@ -2754,9 +2855,21 @@ Axiom substCo : forall `{Util.HasDebugCallStack},
 
 Axiom stripCoercionTy : Type_ -> Coercion.
 
+Axiom strictenDmd : Demand -> CleanDemand.
+
+Axiom strictSigDmdEnv : StrictSig -> DmdEnv.
+
+Axiom strictApply1Dmd : Demand.
+
+Axiom strTop : ArgStr.
+
+Axiom strBot : ArgStr.
+
 Axiom splitVisVarsOfTypes : list Type_ -> Pair.Pair TyCoVarSet.
 
 Axiom splitVisVarsOfType : Type_ -> Pair.Pair TyCoVarSet.
+
+Axiom splitUseProdDmd : nat -> UseDmd -> option (list ArgUse).
 
 Axiom splitTyConApp_maybe : forall `{Util.HasDebugCallStack},
                             Type_ -> option (TyCon * list Type_)%type.
@@ -2764,6 +2877,12 @@ Axiom splitTyConApp_maybe : forall `{Util.HasDebugCallStack},
 Axiom splitTyConAppCo_maybe : Coercion -> option (TyCon * list Coercion)%type.
 
 Axiom splitTyConApp : Type_ -> (TyCon * list Type_)%type.
+
+Axiom splitStrictSig : StrictSig -> (list Demand * DmdResult)%type.
+
+Axiom splitStrProdDmd : nat -> StrDmd -> option (list ArgStr).
+
+Axiom splitProdDmd_maybe : Demand -> option (list Demand).
 
 Axiom splitPiTysInvisible : Type_ -> (list TyBinder * Type_)%type.
 
@@ -2796,9 +2915,15 @@ Axiom splitForAllTy : Type_ -> (TyVar * Type_)%type.
 Axiom splitForAllCo_maybe : Coercion ->
                             option (TyVar * Coercion * Coercion)%type.
 
+Axiom splitFVs : bool -> DmdEnv -> (DmdEnv * DmdEnv)%type.
+
+Axiom splitDmdTy : DmdType -> (Demand * DmdType)%type.
+
 Axiom splitCoercionType_maybe : Type_ -> option (Type_ * Type_)%type.
 
 Axiom splitCastTy_maybe : Type_ -> option (Type_ * Coercion)%type.
+
+Axiom splitArgStrProdDmd : nat -> ArgStr -> option (list ArgStr).
 
 Axiom splitAppTys : Type_ -> (Type_ * list Type_)%type.
 
@@ -2820,15 +2945,64 @@ Axiom setCoVarUnique : CoVar -> Unique.Unique -> CoVar.
 
 Axiom setCoVarName : CoVar -> Name.Name -> CoVar.
 
+Definition seqUseDmd : UseDmd -> unit :=
+  fun x => tt.
+
 Axiom seqTypes : list Type_ -> unit.
 
 Axiom seqType : Type_ -> unit.
 
+Definition seqStrictSig : StrictSig -> unit :=
+  fun x => tt.
+
+Definition seqStrDmdList : list ArgStr -> unit :=
+  fun x => tt.
+
+Definition seqStrDmd : StrDmd -> unit :=
+  fun x => tt.
+
 Axiom seqProv : UnivCoProvenance -> unit.
+
+Definition seqDmdType : DmdType -> unit :=
+  fun x => tt.
+
+Definition seqDmdResult : DmdResult -> unit :=
+  fun x => tt.
+
+Definition seqDmdEnv : DmdEnv -> unit :=
+  fun x => tt.
+
+Axiom seqDmd : Demand.
+
+Definition seqDemandList : list Demand -> unit :=
+  fun x => tt.
+
+Definition seqDemand : Demand -> unit :=
+  fun x => tt.
 
 Axiom seqCos : list Coercion -> unit.
 
 Axiom seqCo : Coercion -> unit.
+
+Definition seqCPRResult : CPRResult -> unit :=
+  fun x => tt.
+
+Definition seqArgUseList : list ArgUse -> unit :=
+  fun x => tt.
+
+Definition seqArgUse : ArgUse -> unit :=
+  fun x => tt.
+
+Definition seqArgStr : ArgStr -> unit :=
+  fun x => tt.
+
+Axiom saturatedByOneShots : nat -> Demand -> bool.
+
+Axiom reuseEnv : DmdEnv -> DmdEnv.
+
+Axiom returnsCPR_maybe : DmdResult -> option BasicTypes.ConTag.
+
+Axiom retCPR_maybe : CPRResult -> option BasicTypes.ConTag.
 
 Axiom resultIsLevPoly : Type_ -> bool.
 
@@ -2843,9 +3017,17 @@ Axiom repSplitAppTy_maybe : forall `{Util.HasDebugCallStack},
 
 Axiom repGetTyVar_maybe : Type_ -> option TyVar.
 
+Axiom removeDmdTyArgs : DmdType -> DmdType.
+
 Axiom provSize : UnivCoProvenance -> nat.
 
+Axiom promoteDataCon : DataCon -> TyCon.
+
 Axiom promoteCoercion : Coercion -> Coercion.
+
+Axiom primRepIsFloat : PrimRep -> option bool.
+
+Axiom primElemRepSizeB : PrimElemRep -> nat.
 
 Axiom predTypeEqRel : PredType -> EqRel.
 
@@ -2883,6 +3065,8 @@ Axiom pprSigmaType : Type_ -> GHC.Base.String.
 
 Axiom pprShortTyThing : TyThing -> GHC.Base.String.
 
+Axiom pprPromotionQuote : TyCon -> GHC.Base.String.
+
 Axiom pprPrecType : BasicTypes.TyPrec -> Type_ -> GHC.Base.String.
 
 Axiom pprParendType : Type_ -> GHC.Base.String.
@@ -2914,6 +3098,16 @@ Axiom pprClassPred : Class -> list Type_ -> GHC.Base.String.
 
 Axiom ppSuggestExplicitKinds : GHC.Base.String.
 
+Axiom postProcessUnsat : DmdShell -> DmdType -> DmdType.
+
+Axiom postProcessDmdType : DmdShell -> DmdType -> BothDmdArg.
+
+Axiom postProcessDmdResult : Str unit -> DmdResult -> DmdResult.
+
+Axiom postProcessDmdEnv : DmdShell -> DmdEnv -> DmdEnv.
+
+Axiom postProcessDmd : DmdShell -> Demand -> Demand.
+
 Axiom piResultTys : forall `{Util.HasDebugCallStack},
                     Type_ -> list Type_ -> Type_.
 
@@ -2921,12 +3115,53 @@ Axiom piResultTy_maybe : Type_ -> Type_ -> option Type_.
 
 Axiom piResultTy : forall `{Util.HasDebugCallStack}, Type_ -> Type_ -> Type_.
 
+Axiom peelUseCall : UseDmd -> option (Count * UseDmd)%type.
+
+Axiom peelManyCalls : nat -> CleanDemand -> DmdShell.
+
+Axiom peelFV : DmdType -> Var -> (DmdType * Demand)%type.
+
+Axiom peelCallDmd : CleanDemand -> (CleanDemand * DmdShell)%type.
+
+Axiom patSynUnivTyVarBinders : PatSyn -> list TyVarBinder.
+
+Axiom patSynSig : PatSyn ->
+                  (list TyVar * ThetaType * list TyVar * ThetaType * list Type_ * Type_)%type.
+
+Axiom patSynName : PatSyn -> Name.Name.
+
+Axiom patSynMatcher : PatSyn -> (Id * bool)%type.
+
+Axiom patSynIsInfix : PatSyn -> bool.
+
+Axiom patSynFieldType : PatSyn -> FieldLabel.FieldLabelString -> Type_.
+
+Axiom patSynFieldLabels : PatSyn -> list FieldLabel.FieldLabel.
+
+Axiom patSynExTyVars : PatSyn -> list TyVar.
+
+Axiom patSynExTyVarBinders : PatSyn -> list TyVarBinder.
+
+Axiom patSynBuilder : PatSyn -> option (Id * bool)%type.
+
+Axiom patSynArity : PatSyn -> BasicTypes.Arity.
+
+Axiom patSynArgs : PatSyn -> list Type_.
+
 Axiom partitionInvisibles : forall {a},
                             TyCon -> (a -> Type_) -> list a -> (list a * list a)%type.
+
+Axiom oneifyDmd : Demand -> Demand.
+
+Axiom okParent : Name.Name -> AlgTyConFlav -> bool.
 
 Axiom nthRole : Role -> TyCon -> nat -> Role.
 
 Axiom notElemTCvSubst : Var -> TCvSubst -> bool.
+
+Axiom nopSig : StrictSig.
+
+Axiom nopDmdType : DmdType.
 
 Axiom nonDetCmpTypesX : RnEnv2 -> list Type_ -> list Type_ -> comparison.
 
@@ -2946,9 +3181,23 @@ Axiom noFreeVarsOfCo : Coercion -> bool.
 
 Axiom nextRole : Type_ -> Role.
 
+Axiom newTyConRhs : TyCon -> (list TyVar * Type_)%type.
+
 Axiom newTyConInstRhs : TyCon -> list Type_ -> Type_.
 
+Axiom newTyConEtadRhs : TyCon -> (list TyVar * Type_)%type.
+
+Axiom newTyConEtadArity : TyCon -> nat.
+
+Axiom newTyConDataCon_maybe : TyCon -> option DataCon.
+
+Axiom newTyConCo_maybe : TyCon -> option (CoAxiom Unbranched).
+
+Axiom newTyConCo : TyCon -> CoAxiom Unbranched.
+
 Axiom modifyJoinResTy : nat -> (Type_ -> Type_) -> Type_ -> Type_.
+
+Axiom mkWorkerDemand : nat -> Demand.
 
 Axiom mkVisForAllTys : list TyVar -> Type_ -> Type_.
 
@@ -2965,11 +3214,71 @@ Axiom mkUnbranchedAxInstLHS : CoAxiom Unbranched ->
 Axiom mkUnbranchedAxInstCo : Role ->
                              CoAxiom Unbranched -> list Type_ -> list Coercion -> Coercion.
 
+Local Definition Eq___Count_op_zeze__ : Count -> Count -> bool :=
+  fun arg_0__ arg_1__ =>
+    match arg_0__, arg_1__ with
+    | One, One => true
+    | Many, Many => true
+    | _, _ => false
+    end.
+
+Local Definition Eq___Count_op_zsze__ : Count -> Count -> bool :=
+  fun x y => negb (Eq___Count_op_zeze__ x y).
+
+Program Instance Eq___Count : GHC.Base.Eq_ Count :=
+  fun _ k__ =>
+    k__ {| GHC.Base.op_zeze____ := Eq___Count_op_zeze__ ;
+           GHC.Base.op_zsze____ := Eq___Count_op_zsze__ |}.
+
+Local Definition Eq___Use_op_zeze__ {inst_u} `{GHC.Base.Eq_ inst_u}
+   : Use inst_u -> Use inst_u -> bool :=
+  fun arg_0__ arg_1__ =>
+    match arg_0__, arg_1__ with
+    | Abs, Abs => true
+    | Mk_Use a1 a2, Mk_Use b1 b2 =>
+        (andb ((a1 GHC.Base.== b1)) ((a2 GHC.Base.== b2)))
+    | _, _ => false
+    end.
+
+Local Definition Eq___Use_op_zsze__ {inst_u} `{GHC.Base.Eq_ inst_u}
+   : Use inst_u -> Use inst_u -> bool :=
+  fun x y => negb (Eq___Use_op_zeze__ x y).
+
+Program Instance Eq___Use {u} `{GHC.Base.Eq_ u} : GHC.Base.Eq_ (Use u) :=
+  fun _ k__ =>
+    k__ {| GHC.Base.op_zeze____ := Eq___Use_op_zeze__ ;
+           GHC.Base.op_zsze____ := Eq___Use_op_zsze__ |}.
+
+Local Definition Eq___UseDmd_op_zeze__ : UseDmd -> UseDmd -> bool :=
+  fix UseDmd_eq x y
+        := let eq' : GHC.Base.Eq_ UseDmd := GHC.Base.eq_default UseDmd_eq in
+           match x, y with
+           | UCall a1 a2, UCall b1 b2 => andb (a1 GHC.Base.== b1) (a2 GHC.Base.== b2)
+           | UProd a1, UProd b1 => a1 GHC.Base.== b1
+           | UHead, UHead => true
+           | Used, Used => true
+           | _, _ => false
+           end.
+
+Local Definition Eq___UseDmd_op_zsze__ : UseDmd -> UseDmd -> bool :=
+  fun x y => negb (Eq___UseDmd_op_zeze__ x y).
+
+Program Instance Eq___UseDmd : GHC.Base.Eq_ UseDmd :=
+  fun _ k__ =>
+    k__ {| GHC.Base.op_zeze____ := Eq___UseDmd_op_zeze__ ;
+           GHC.Base.op_zsze____ := Eq___UseDmd_op_zsze__ |}.
+
+Axiom mkUProd : list ArgUse -> UseDmd.
+
+Axiom mkUCall : Count -> UseDmd -> UseDmd.
+
 Axiom mkTyVarTys : list TyVar -> list Type_.
 
 Axiom mkTyVarTy : TyVar -> Type_.
 
 Axiom mkTyConTy : TyCon -> Type_.
+
+Axiom mkTyConKind : list TyConBinder -> Kind -> Kind.
 
 Axiom mkTyConBindersPreferAnon : list TyVar -> Type_ -> list TyConBinder.
 
@@ -2984,23 +3293,45 @@ Axiom mkTvSubstPrs : list (TyVar * Type_)%type -> TCvSubst.
 
 Axiom mkTvSubst : InScopeSet -> TvSubstEnv -> TCvSubst.
 
+Axiom mkTupleTyCon : Name.Name ->
+                     list TyConBinder ->
+                     Kind ->
+                     BasicTypes.Arity -> DataCon -> BasicTypes.TupleSort -> AlgTyConFlav -> TyCon.
+
 Axiom mkTransCo : Coercion -> Coercion -> Coercion.
 
 Axiom mkTransAppCo : Role ->
                      Coercion ->
                      Type_ -> Type_ -> Role -> Coercion -> Type_ -> Type_ -> Role -> Coercion.
 
+Axiom mkTcTyCon : Name.Name ->
+                  list TyConBinder ->
+                  Kind -> list (Name.Name * TyVar)%type -> TyConFlavour -> TyCon.
+
 Axiom mkTCvSubst : InScopeSet -> (TvSubstEnv * CvSubstEnv)%type -> TCvSubst.
 
+Axiom mkSynonymTyCon : Name.Name ->
+                       list TyConBinder -> Kind -> list Role -> Type_ -> bool -> bool -> TyCon.
+
 Axiom mkSymCo : Coercion -> Coercion.
+
+Axiom mkSumTyCon : Name.Name ->
+                   list TyConBinder ->
+                   Kind -> BasicTypes.Arity -> list TyVar -> list DataCon -> AlgTyConFlav -> TyCon.
 
 Axiom mkSubstLiftingContext : TCvSubst -> LiftingContext.
 
 Axiom mkSubCo : Coercion -> Coercion.
 
+Axiom mkStrictSig : DmdType -> StrictSig.
+
 Axiom mkStrLitTy : FastString.FastString -> Type_.
 
 Axiom mkSpecForAllTys : list TyVar -> Type_ -> Type_.
+
+Axiom mkSProd : list ArgStr -> StrDmd.
+
+Axiom mkSCall : StrDmd -> StrDmd.
 
 Axiom mkRuntimeRepCo : forall `{Util.HasDebugCallStack}, Coercion -> Coercion.
 
@@ -3012,9 +3343,23 @@ Axiom mkReflCo : Role -> Type_ -> Coercion.
 
 Axiom mkProofIrrelCo : Role -> Coercion -> Coercion -> Coercion -> Coercion.
 
+Axiom mkPromotedDataCon : DataCon ->
+                          Name.Name ->
+                          TyConRepName ->
+                          list TyConBinder -> Kind -> list Role -> RuntimeRepInfo -> TyCon.
+
+Axiom mkProdDmd : list Demand -> CleanDemand.
+
+Axiom mkPrimTyCon' : Name.Name ->
+                     list TyConBinder -> Kind -> list Role -> bool -> option TyConRepName -> TyCon.
+
+Axiom mkPrimTyCon : Name.Name -> list TyConBinder -> Kind -> list Role -> TyCon.
+
 Axiom mkPrimEqPredRole : Role -> Type_ -> Type_ -> PredType.
 
 Axiom mkPrimEqPred : Type_ -> Type_ -> Type_.
+
+Axiom mkPrelTyConRepName : Name.Name -> TyConRepName.
 
 Axiom mkPiTys : list TyBinder -> Type_ -> Type_.
 
@@ -3026,6 +3371,17 @@ Axiom mkPiCo : Role -> Var -> Coercion -> Coercion.
 
 Axiom mkPhantomCo : Coercion -> Type_ -> Type_ -> Coercion.
 
+Axiom mkPatSyn : Name.Name ->
+                 bool ->
+                 (list TyVarBinder * ThetaType)%type ->
+                 (list TyVarBinder * ThetaType)%type ->
+                 list Type_ ->
+                 Type_ ->
+                 (Id * bool)%type ->
+                 option (Id * bool)%type -> list FieldLabel.FieldLabel -> PatSyn.
+
+Axiom mkOnceUsedDmd : CleanDemand -> Demand.
+
 Axiom mkNumLitTy : GHC.Num.Integer -> Type_.
 
 Axiom mkNthCoRole : Role -> nat -> Coercion -> Coercion.
@@ -3034,7 +3390,16 @@ Axiom mkNthCo : nat -> Coercion -> Coercion.
 
 Axiom mkNomReflCo : Type_ -> Coercion.
 
+Axiom mkNamedTyConBinders : ArgFlag -> list TyVar -> list TyConBinder.
+
+Axiom mkNamedTyConBinder : ArgFlag -> TyVar -> TyConBinder.
+
+Axiom mkManyUsedDmd : CleanDemand -> Demand.
+
 Axiom mkLiftingContext : list (TyCoVar * Coercion)%type -> LiftingContext.
+
+Axiom mkLiftedPrimTyCon : Name.Name ->
+                          list TyConBinder -> Kind -> list Role -> TyCon.
 
 Axiom mkLamTypes : list Var -> Type_ -> Type_.
 
@@ -3042,7 +3407,14 @@ Axiom mkLamType : Var -> Type_ -> Type_.
 
 Axiom mkLRCo : BasicTypes.LeftOrRight -> Coercion -> Coercion.
 
+Axiom mkKindTyCon : Name.Name ->
+                    list TyConBinder -> Kind -> list Role -> Name.Name -> TyCon.
+
 Axiom mkKindCo : Coercion -> Coercion.
+
+Axiom mkJointDmds : forall {s} {u}, list s -> list u -> list (JointDmd s u).
+
+Axiom mkJointDmd : forall {s} {u}, s -> u -> JointDmd s u.
 
 Axiom mkInvForAllTys : list TyVar -> Type_ -> Type_.
 
@@ -3064,7 +3436,11 @@ Axiom mkHeteroPrimEqPred : Kind -> Kind -> Type_ -> Type_ -> Type_.
 
 Axiom mkHeteroCoercionType : Role -> Kind -> Kind -> Type_ -> Type_ -> Type_.
 
+Axiom mkHeadStrict : CleanDemand -> CleanDemand.
+
 Axiom mkFunTys : list Type_ -> Type_ -> Type_.
+
+Axiom mkFunTyCon : Name.Name -> list TyConBinder -> Name.Name -> TyCon.
 
 Axiom mkFunTy : Type_ -> Type_ -> Type_.
 
@@ -3084,7 +3460,16 @@ Axiom mkForAllCo : TyVar -> Coercion -> Coercion -> Coercion.
 
 Axiom mkFamilyTyConApp : TyCon -> list Type_ -> Type_.
 
+Axiom mkFamilyTyCon : Name.Name ->
+                      list TyConBinder ->
+                      Kind ->
+                      option Name.Name -> FamTyConFlav -> option Class -> Injectivity -> TyCon.
+
+Axiom mkEqSpec : TyVar -> Type_ -> EqSpec.
+
 Axiom mkEmptyTCvSubst : InScopeSet -> TCvSubst.
+
+Axiom mkDmdType : DmdEnv -> list Demand -> DmdResult -> DmdType.
 
 Axiom mkCoherenceRightCo : Coercion -> Coercion -> Coercion.
 
@@ -3102,9 +3487,25 @@ Axiom mkCoVarCo : CoVar -> Coercion.
 
 Axiom mkCoCast : Coercion -> Coercion -> Coercion.
 
+Axiom mkClosedStrictSig : list Demand -> DmdResult -> StrictSig.
+
+Axiom mkClassTyCon : Name.Name ->
+                     list TyConBinder -> list Role -> AlgTyConRhs -> Class -> Name.Name -> TyCon.
+
 Axiom mkClassPred : Class -> list Type_ -> PredType.
 
+Axiom mkClass : Name.Name ->
+                list TyVar ->
+                list (FunDep TyVar) ->
+                list PredType ->
+                list Id ->
+                list ClassATItem -> list ClassOpItem -> ClassMinimalDef -> TyCon -> Class.
+
 Axiom mkCastTy : Type_ -> Coercion -> Type_.
+
+Axiom mkCallDmd : CleanDemand -> CleanDemand.
+
+Axiom mkBothDmdArg : DmdEnv -> BothDmdArg.
 
 Axiom mkAxiomRuleCo : CoAxiomRule -> list Coercion -> Coercion.
 
@@ -3128,7 +3529,28 @@ Axiom mkAppCos : Coercion -> list Coercion -> Coercion.
 
 Axiom mkAppCo : Coercion -> Coercion -> Coercion.
 
+Axiom mkAnonTyConBinders : list TyVar -> list TyConBinder.
+
+Axiom mkAnonTyConBinder : TyVar -> TyConBinder.
+
 Axiom mkAnonBinder : Type_ -> TyBinder.
+
+Axiom mkAlgTyCon : Name.Name ->
+                   list TyConBinder ->
+                   Kind ->
+                   list Role ->
+                   option unit -> list PredType -> AlgTyConRhs -> AlgTyConFlav -> bool -> TyCon.
+
+Axiom mkAbstractClass : Name.Name ->
+                        list TyVar -> list (FunDep TyVar) -> TyCon -> Class.
+
+Axiom mightBeUnsaturatedTyCon : TyCon -> bool.
+
+Axiom markReusedDmd : ArgUse -> ArgUse.
+
+Axiom markReused : UseDmd -> UseDmd.
+
+Axiom markExnStr : ArgStr -> ArgStr.
 
 Axiom mapType : forall {m} {env},
                 forall `{GHC.Base.Monad m}, TyCoMapper env m -> env -> Type_ -> m Type_.
@@ -3139,9 +3561,34 @@ Axiom mapStepResult : forall {ev1} {ev2},
 Axiom mapCoercion : forall {m} {env},
                     forall `{GHC.Base.Monad m}, TyCoMapper env m -> env -> Coercion -> m Coercion.
 
+Axiom makeRecoveryTyCon : TyCon -> TyCon.
+
+Axiom lubUse : UseDmd -> UseDmd -> UseDmd.
+
+Axiom lubStr : StrDmd -> StrDmd -> StrDmd.
+
+Axiom lubExnStr : ExnStr -> ExnStr -> ExnStr.
+
+Axiom lubDmdType : DmdType -> DmdType -> DmdType.
+
+Axiom lubDmdResult : DmdResult -> DmdResult -> DmdResult.
+
+Axiom lubDmd : Demand -> Demand -> Demand.
+
+Axiom lubCount : Count -> Count -> Count.
+
+Axiom lubCPR : CPRResult -> CPRResult -> CPRResult.
+
+Axiom lubArgUse : ArgUse -> ArgUse -> ArgUse.
+
+Axiom lubArgStr : ArgStr -> ArgStr -> ArgStr.
+
 Axiom ltRole : Role -> Role -> bool.
 
 Axiom lookupTyVar : TCvSubst -> TyVar -> option Type_.
+
+Axiom lookupTyConFieldLabel : FieldLabel.FieldLabelString ->
+                              TyCon -> option FieldLabel.FieldLabel.
 
 Axiom lookupCoVar : TCvSubst -> Var -> option Coercion.
 
@@ -3180,31 +3627,107 @@ Axiom lcSubstLeft : LiftingContext -> TCvSubst.
 
 Axiom lcInScopeSet : LiftingContext -> InScopeSet.
 
+Axiom lazyApply2Dmd : Demand.
+
+Axiom lazyApply1Dmd : Demand.
+
+Axiom kindTyConKeys : UniqSet.UniqSet Unique.Unique.
+
+Axiom kill_usage : KillFlags -> Demand -> Demand.
+
+Axiom killUsageSig : DynFlags.DynFlags -> StrictSig -> StrictSig.
+
+Axiom killUsageDemand : DynFlags.DynFlags -> Demand -> Demand.
+
+Axiom killFlags : DynFlags.DynFlags -> option KillFlags.
+
 Axiom is_TYPE : (Type_ -> bool) -> Kind -> bool.
 
+Axiom isWeakDmd : Demand -> bool.
+
+Axiom isVoidRep : PrimRep -> bool.
+
+Axiom isVisibleTyConBinder : forall {tv}, TyVarBndr tv TyConBndrVis -> bool.
+
+Axiom isVisibleTcbVis : TyConBndrVis -> bool.
+
 Axiom isVisibleBinder : TyBinder -> bool.
+
+Axiom isVanillaDataCon : DataCon -> bool.
+
+Axiom isVanillaAlgTyCon : TyCon -> bool.
 
 Axiom isValidTCvSubst : TCvSubst -> bool.
 
 Axiom isValidJoinPointType : BasicTypes.JoinArity -> Type_ -> bool.
 
+Axiom isUsedU : UseDmd -> bool.
+
+Axiom isUsedOnce : Demand -> bool.
+
+Axiom isUsedMU : ArgUse -> bool.
+
 Axiom isUnliftedTypeKind : Kind -> bool.
 
 Axiom isUnliftedType : forall `{Util.HasDebugCallStack}, Type_ -> bool.
 
+Axiom isUnliftedTyCon : TyCon -> bool.
+
 Axiom isUnboxedTupleType : Type_ -> bool.
+
+Axiom isUnboxedTupleTyCon : TyCon -> bool.
+
+Axiom isUnboxedTupleCon : DataCon -> bool.
 
 Axiom isUnboxedSumType : Type_ -> bool.
 
+Axiom isUnboxedSumTyCon : TyCon -> bool.
+
+Axiom isUnboxedSumCon : DataCon -> bool.
+
+Axiom isTypeSynonymTyCon : TyCon -> bool.
+
 Axiom isTypeLevPoly : Type_ -> bool.
 
+Axiom isTypeFamilyTyCon : TyCon -> bool.
+
 Axiom isTyVarTy : Type_ -> bool.
+
+Axiom isTyConWithSrcDataCons : TyCon -> bool.
+
+Axiom isTyConAssoc : TyCon -> bool.
+
+Axiom isTupleTyCon : TyCon -> bool.
+
+Axiom isTupleDataCon : DataCon -> bool.
+
+Axiom isTopSig : StrictSig -> bool.
+
+Axiom isTopRes : DmdResult -> bool.
+
+Axiom isTopDmdType : DmdType -> bool.
+
+Axiom isTopDmd : Demand -> bool.
+
+Axiom isTcTyCon : TyCon -> bool.
+
+Axiom isTcLevPoly : TyCon -> bool.
+
+Axiom isTauTyCon : TyCon -> bool.
 
 Axiom isTauTy : Type_ -> bool.
 
 Axiom isStrictType : forall `{Util.HasDebugCallStack}, Type_ -> bool.
 
+Axiom isStrictDmd : Demand -> bool.
+
 Axiom isStrLitTy : Type_ -> option FastString.FastString.
+
+Axiom isSrcUnpacked : SrcUnpackedness -> bool.
+
+Axiom isSrcStrict : SrcStrictness -> bool.
+
+Axiom isSeqDmd : Demand -> bool.
 
 Axiom isRuntimeRepVar : TyVar -> bool.
 
@@ -3222,17 +3745,43 @@ Axiom isReflCoVar_maybe : CoVar -> option Coercion.
 
 Axiom isReflCo : Coercion -> bool.
 
+Axiom isPromotedTupleTyCon : TyCon -> bool.
+
+Axiom isPromotedDataCon_maybe : TyCon -> option DataCon.
+
+Axiom isPromotedDataCon : TyCon -> bool.
+
+Axiom isProductTyCon : TyCon -> bool.
+
 Axiom isPrimitiveType : Type_ -> bool.
+
+Axiom isPrimTyCon : TyCon -> bool.
 
 Axiom isPredTy : Type_ -> bool.
 
 Axiom isPiTy : Type_ -> bool.
 
+Axiom isOpenTypeFamilyTyCon : TyCon -> bool.
+
+Axiom isOpenFamilyTyCon : TyCon -> bool.
+
 Axiom isNumLitTy : Type_ -> option GHC.Num.Integer.
+
+Axiom isNullarySrcDataCon : DataCon -> bool.
+
+Axiom isNullaryRepDataCon : DataCon -> bool.
 
 Axiom isNomEqPred : PredType -> bool.
 
+Axiom isNoParent : AlgTyConFlav -> bool.
+
+Axiom isNewTyCon : TyCon -> bool.
+
+Axiom isNamedTyConBinder : TyConBinder -> bool.
+
 Axiom isNamedTyBinder : TyBinder -> bool.
+
+Axiom isMarkedStrict : StrictnessMark -> bool.
 
 Axiom isMappedByLC : TyCoVar -> LiftingContext -> bool.
 
@@ -3241,9 +3790,19 @@ Axiom isLiftedType_maybe : forall `{Util.HasDebugCallStack},
 
 Axiom isLiftedTypeKind : Kind -> bool.
 
+Axiom isLazy : ArgStr -> bool.
+
+Axiom isKindTyCon : TyCon -> bool.
+
+Axiom isInvisibleTyConBinder : forall {tv}, TyVarBndr tv TyConBndrVis -> bool.
+
 Axiom isInvisibleBinder : TyBinder -> bool.
 
+Axiom isInjectiveTyCon : TyCon -> Role -> bool.
+
 Axiom isInScope : Var -> TCvSubst -> bool.
+
+Axiom isImplicitTyCon : TyCon -> bool.
 
 Axiom isIPTyCon : TyCon -> bool.
 
@@ -3253,13 +3812,33 @@ Axiom isIPPred : PredType -> bool.
 
 Axiom isIPClass : Class -> bool.
 
+Axiom isHyperStr : ArgStr -> bool.
+
+Axiom isGenerativeTyCon : TyCon -> Role -> bool.
+
+Axiom isGenInjAlgRhs : AlgTyConRhs -> bool.
+
+Axiom isGcPtrRep : PrimRep -> bool.
+
+Axiom isGadtSyntaxTyCon : TyCon -> bool.
+
+Axiom isFunTyCon : TyCon -> bool.
+
 Axiom isFunTy : Type_ -> bool.
 
 Axiom isForAllTy : Type_ -> bool.
 
+Axiom isFamilyTyCon : TyCon -> bool.
+
+Axiom isFamInstTyCon : TyCon -> bool.
+
+Axiom isFamFreeTyCon : TyCon -> bool.
+
 Axiom isFamFreeTy : Type_ -> bool.
 
 Axiom isEqPred : PredType -> bool.
+
+Axiom isEnumerationTyCon : TyCon -> bool.
 
 Axiom isEmptyTCvSubst : TCvSubst -> bool.
 
@@ -3267,7 +3846,17 @@ Axiom isDictTy : Type_ -> bool.
 
 Axiom isDictLikeTy : Type_ -> bool.
 
+Axiom isDataTyCon : TyCon -> bool.
+
+Axiom isDataSumTyCon_maybe : TyCon -> option (list DataCon).
+
+Axiom isDataProductTyCon_maybe : TyCon -> option DataCon.
+
+Axiom isDataFamilyTyCon : TyCon -> bool.
+
 Axiom isDataFamilyAppType : Type_ -> bool.
+
+Axiom isDataFamFlav : FamTyConFlav -> bool.
 
 Axiom isCoercionType : Type_ -> bool.
 
@@ -3277,13 +3866,36 @@ Axiom isCoercionTy : Type_ -> bool.
 
 Axiom isCoVar_maybe : Coercion -> option CoVar.
 
+Axiom isClosedSynFamilyTyConWithAxiom_maybe : TyCon ->
+                                              option (CoAxiom Branched).
+
+Axiom isClassTyCon : TyCon -> bool.
+
 Axiom isClassPred : PredType -> bool.
 
 Axiom isCTupleClass : Class -> bool.
 
+Axiom isBuiltInSynFamTyCon_maybe : TyCon -> option BuiltInSynFamily.
+
+Axiom isBoxedTupleTyCon : TyCon -> bool.
+
+Axiom isBottomingSig : StrictSig -> bool.
+
+Axiom isBotRes : DmdResult -> bool.
+
+Axiom isBanged : HsImplBang -> bool.
+
 Axiom isAnonTyBinder : TyBinder -> bool.
 
 Axiom isAlgType : Type_ -> bool.
+
+Axiom isAlgTyCon : TyCon -> bool.
+
+Axiom isAbstractTyCon : TyCon -> bool.
+
+Axiom isAbstractClass : Class -> bool.
+
+Axiom isAbsDmd : Demand -> bool.
 
 Axiom instNewTyCon_maybe : TyCon ->
                            list Type_ -> option (Type_ * Coercion)%type.
@@ -3291,6 +3903,14 @@ Axiom instNewTyCon_maybe : TyCon ->
 Axiom instCoercions : Coercion -> list Coercion -> option Coercion.
 
 Axiom instCoercion : Pair.Pair Type_ -> Coercion -> Coercion -> option Coercion.
+
+Axiom initRecTc : RecTcChecker.
+
+Axiom increaseStrictSigArity : nat -> StrictSig -> StrictSig.
+
+Axiom hasDemandEnvSig : StrictSig -> bool.
+
+Axiom getUseDmd : forall {s} {u}, JointDmd s u -> u.
 
 Axiom getTyVar_maybe : Type_ -> option TyVar.
 
@@ -3301,6 +3921,8 @@ Axiom getTvSubstEnv : TCvSubst -> TvSubstEnv.
 Axiom getTCvSubstRangeFVs : TCvSubst -> VarSet.
 
 Axiom getTCvInScope : TCvSubst -> InScopeSet.
+
+Axiom getStrDmd : forall {s} {u}, JointDmd s u -> s.
 
 Axiom getRuntimeRep_maybe : forall `{Util.HasDebugCallStack},
                             Type_ -> option Type_.
@@ -3334,7 +3956,26 @@ Axiom funResultTy : Type_ -> Type_.
 
 Axiom funArgTy : Type_ -> Type_.
 
+Axiom findIdDemand : DmdType -> Var -> Demand.
+
 Axiom filterOutInvisibleTypes : TyCon -> list Type_ -> list Type_.
+
+Local Definition Eq___Var_op_zeze__ : Var -> Var -> bool :=
+  fun a b => realUnique a GHC.Base.== realUnique b.
+
+Local Definition Eq___Var_op_zsze__ : Var -> Var -> bool :=
+  fun x y => negb (Eq___Var_op_zeze__ x y).
+
+Program Instance Eq___Var : GHC.Base.Eq_ Var :=
+  fun _ k__ =>
+    k__ {| GHC.Base.op_zeze____ := Eq___Var_op_zeze__ ;
+           GHC.Base.op_zsze____ := Eq___Var_op_zsze__ |}.
+
+Axiom filterEqSpec : list EqSpec -> list TyVar -> list TyVar.
+
+Axiom fieldsOfAlgTcRhs : AlgTyConRhs -> FieldLabel.FieldLabelEnv.
+
+Axiom famTyConFlav_maybe : TyCon -> option FamTyConFlav.
 
 Axiom extendTvSubstWithClone : TCvSubst -> TyVar -> TyVar -> TCvSubst.
 
@@ -3366,6 +4007,18 @@ Axiom extendCvSubst : TCvSubst -> CoVar -> Coercion -> TCvSubst.
 
 Axiom expandTypeSynonyms : Type_ -> Type_.
 
+Axiom expandSynTyCon_maybe : forall {tyco},
+                             TyCon ->
+                             list tyco -> option (list (TyVar * tyco)%type * Type_ * list tyco)%type.
+
+Axiom exnSig : StrictSig.
+
+Axiom exnRes : DmdResult.
+
+Axiom exnDmdType : DmdType.
+
+Axiom evalDmd : Demand.
+
 Axiom equalityTyCon : Role -> TyCon.
 
 Axiom eqVarBndrs : RnEnv2 -> list Var -> list Var -> option RnEnv2.
@@ -3376,17 +4029,29 @@ Axiom eqTypeX : RnEnv2 -> Type_ -> Type_ -> bool.
 
 Axiom eqType : Type_ -> Type_ -> bool.
 
+Axiom eqSpecType : EqSpec -> Type_.
+
+Axiom eqSpecTyVar : EqSpec -> TyVar.
+
+Axiom eqSpecPair : EqSpec -> (TyVar * Type_)%type.
+
 Axiom eqRelRole : EqRel -> Role.
 
 Axiom eqCoercionX : RnEnv2 -> Coercion -> Coercion -> bool.
 
 Axiom eqCoercion : Coercion -> Coercion -> bool.
 
+Axiom dmdTypeDepth : DmdType -> BasicTypes.Arity.
+
+Axiom ensureArgs : BasicTypes.Arity -> DmdType -> DmdType.
+
 Axiom emptyTvSubstEnv : TvSubstEnv.
 
 Axiom emptyTCvSubst : TCvSubst.
 
 Axiom emptyLiftingContext : InScopeSet -> LiftingContext.
+
+Axiom emptyDmdEnv : VarEnv Demand.
 
 Axiom emptyCvSubstEnv : CvSubstEnv.
 
@@ -3398,7 +4063,18 @@ Axiom downgradeRole_maybe : Role -> Role -> Coercion -> option Coercion.
 
 Axiom downgradeRole : Role -> Role -> Coercion -> Coercion.
 
+Axiom dmdTransformSig : StrictSig -> CleanDemand -> DmdType.
+
+Axiom dmdTransformDictSelSig : StrictSig -> CleanDemand -> DmdType.
+
+Axiom dmdTransformDataConSig : BasicTypes.Arity ->
+                               StrictSig -> CleanDemand -> DmdType.
+
 Axiom delBinderVar : VarSet -> TyVarBinder -> VarSet.
+
+Axiom deferAfterIO : DmdType -> DmdType.
+
+Axiom defaultDmd : forall {r}, Termination r -> Demand.
 
 Axiom decomposeFunCo : Coercion -> (Coercion * Coercion)%type.
 
@@ -3408,7 +4084,65 @@ Axiom debug_ppr_ty : BasicTypes.TyPrec -> Type_ -> GHC.Base.String.
 
 Axiom debugPprType : Type_ -> GHC.Base.String.
 
+Axiom dataConWrapId_maybe : DataCon -> option Id.
+
+Axiom dataConWrapId : DataCon -> Id.
+
+Axiom dataConWorkId : DataCon -> Id.
+
+Axiom dataConUserTyVarsArePermuted : DataCon -> bool.
+
+Axiom dataConUserTyVars : DataCon -> list TyVar.
+
+Axiom dataConUserTyVarBinders : DataCon -> list TyVarBinder.
+
+Axiom dataConUnivTyVars : DataCon -> list TyVar.
+
+Axiom dataConUnivAndExTyVars : DataCon -> list TyVar.
+
+Axiom dataConTyCon : DataCon -> TyCon.
+
+Axiom dataConTagZ : DataCon -> BasicTypes.ConTagZ.
+
+Axiom dataConTag : DataCon -> BasicTypes.ConTag.
+
+Axiom dataConStupidTheta : DataCon -> ThetaType.
+
+Axiom dataConSrcBangs : DataCon -> list HsSrcBang.
+
+Axiom dataConSourceArity : DataCon -> BasicTypes.Arity.
+
+Axiom dataConRepType : DataCon -> Type_.
+
+Axiom dataConRepArity : DataCon -> BasicTypes.Arity.
+
+Axiom dataConName : DataCon -> Name.Name.
+
+Axiom dataConIsInfix : DataCon -> bool.
+
+Axiom dataConImplBangs : DataCon -> list HsImplBang.
+
+Axiom dataConFullSig : DataCon ->
+                       (list TyVar * list TyVar * list EqSpec * ThetaType * list Type_ * Type_)%type.
+
+Axiom dataConFieldType_maybe : DataCon ->
+                               FieldLabel.FieldLabelString -> option (FieldLabel.FieldLabel * Type_)%type.
+
+Axiom dataConFieldLabels : DataCon -> list FieldLabel.FieldLabel.
+
+Axiom dataConCannotMatch : list Type_ -> DataCon -> bool.
+
+Axiom dataConBoxer : DataCon -> option unit.
+
 Axiom dVarSetElemsWellScoped : DVarSet -> list Var.
+
+Axiom cprSumRes : BasicTypes.ConTag -> DmdResult.
+
+Axiom cprProdSig : BasicTypes.Arity -> StrictSig.
+
+Axiom cprProdRes : list DmdType -> DmdResult.
+
+Axiom cprProdDmdType : BasicTypes.Arity -> DmdType.
 
 Axiom coreView : Type_ -> option Type_.
 
@@ -3471,84 +4205,193 @@ Axiom cloneTyVarBndrs : TCvSubst ->
 Axiom cloneTyVarBndr : TCvSubst ->
                        TyVar -> Unique.Unique -> (TCvSubst * TyVar)%type.
 
+Axiom cleanUseDmd_maybe : Demand -> option UseDmd.
+
+Axiom cleanEvalProdDmd : BasicTypes.Arity -> CleanDemand.
+
+Axiom cleanEvalDmd : CleanDemand.
+
 Axiom classifyPredType : PredType -> PredTree.
+
+Axiom classTvsFds : Class -> (list TyVar * list (FunDep TyVar))%type.
+
+Axiom classSCTheta : Class -> list PredType.
+
+Axiom classOpItems : Class -> list ClassOpItem.
+
+Axiom classMinimalDef : Class -> ClassMinimalDef.
+
+Axiom classMethods : Class -> list Id.
+
+Axiom classHasFds : Class -> bool.
+
+Axiom classExtraBigSig : Class ->
+                         (list TyVar * list (FunDep TyVar) * list PredType * list Id * list ClassATItem *
+                          list ClassOpItem)%type.
+
+Axiom classBigSig : Class ->
+                    (list TyVar * list PredType * list Id * list ClassOpItem)%type.
+
+Axiom classArity : Class -> BasicTypes.Arity.
+
+Axiom classAllSelIds : Class -> list Id.
+
+Axiom classATs : Class -> list TyCon.
+
+Axiom classATItems : Class -> list ClassATItem.
 
 Axiom checkValidSubst : forall {a},
                         forall `{Util.HasDebugCallStack},
                         TCvSubst -> list Type_ -> list Coercion -> a -> a.
+
+Axiom checkRecTc : RecTcChecker -> TyCon -> option RecTcChecker.
+
+Axiom catchArgDmd : Demand.
 
 Axiom castCoercionKind : Coercion -> Coercion -> Coercion -> Coercion.
 
 Axiom caseBinder : forall {a},
                    TyBinder -> (TyVarBinder -> a) -> (Type_ -> a) -> a.
 
+Axiom bothUse : UseDmd -> UseDmd -> UseDmd.
+
+Axiom bothStr : StrDmd -> StrDmd -> StrDmd.
+
+Axiom bothExnStr : ExnStr -> ExnStr -> ExnStr.
+
+Axiom bothDmdType : DmdType -> BothDmdArg -> DmdType.
+
+Axiom bothDmdResult : DmdResult -> Termination unit -> DmdResult.
+
+Axiom bothDmd : Demand -> Demand -> Demand.
+
+Axiom bothCleanDmd : CleanDemand -> CleanDemand -> CleanDemand.
+
+Axiom bothArgUse : ArgUse -> ArgUse -> ArgUse.
+
+Axiom bothArgStr : ArgStr -> ArgStr -> ArgStr.
+
+Axiom botSig : StrictSig.
+
+Axiom botRes : DmdResult.
+
+Axiom botDmdType : DmdType.
+
+Axiom botDmd : Demand.
+
 Axiom binderRelevantType_maybe : TyBinder -> option Type_.
+
+Axiom argsOneShots : StrictSig ->
+                     BasicTypes.Arity -> list (list BasicTypes.OneShotInfo).
+
+Axiom argOneShots : Demand -> list BasicTypes.OneShotInfo.
 
 Axiom applyTysX : list TyVar -> Type_ -> list Type_ -> Type_.
 
 Axiom applyRoles : TyCon -> list Coercion -> list Coercion.
 
-Definition visibleDataCons : AlgTyConRhs -> list DataCon :=
-  fun arg_0__ =>
-    match arg_0__ with
-    | AbstractTyCon => nil
-    | DataTyCon cs _ => cs
-    | NewTyCon c _ _ _ => cons c nil
-    | TupleTyCon c _ => cons c nil
-    | SumTyCon cs => cs
-    end.
+Axiom appIsBottom : StrictSig -> nat -> bool.
+
+Axiom algTyConRhs : TyCon -> AlgTyConRhs.
+
+Axiom addDemand : Demand -> DmdType -> DmdType.
+
+Axiom absDmd : Demand.
+
+Definition zapUsedOnceInfo : IdInfo -> option IdInfo :=
+  fun info =>
+    Some (let 'Mk_IdInfo arityInfo_0__ ruleInfo_1__ unfoldingInfo_2__ cafInfo_3__
+             oneShotInfo_4__ inlinePragInfo_5__ occInfo_6__ strictnessInfo_7__ demandInfo_8__
+             callArityInfo_9__ levityInfo_10__ := info in
+          Mk_IdInfo arityInfo_0__ ruleInfo_1__ unfoldingInfo_2__ cafInfo_3__
+                    oneShotInfo_4__ inlinePragInfo_5__ occInfo_6__ (zapUsedOnceSig (strictnessInfo
+                                                                                    info)) (zapUsedOnceDemand
+                     (demandInfo info)) callArityInfo_9__ levityInfo_10__).
+
+Definition zapUsageInfo : IdInfo -> option IdInfo :=
+  fun info =>
+    Some (let 'Mk_IdInfo arityInfo_0__ ruleInfo_1__ unfoldingInfo_2__ cafInfo_3__
+             oneShotInfo_4__ inlinePragInfo_5__ occInfo_6__ strictnessInfo_7__ demandInfo_8__
+             callArityInfo_9__ levityInfo_10__ := info in
+          Mk_IdInfo arityInfo_0__ ruleInfo_1__ unfoldingInfo_2__ cafInfo_3__
+                    oneShotInfo_4__ inlinePragInfo_5__ occInfo_6__ strictnessInfo_7__
+                    (zapUsageDemand (demandInfo info)) callArityInfo_9__ levityInfo_10__).
+
+Definition zapUsageEnvInfo : IdInfo -> option IdInfo :=
+  fun info =>
+    if hasDemandEnvSig (strictnessInfo info) : bool
+    then Some (let 'Mk_IdInfo arityInfo_0__ ruleInfo_1__ unfoldingInfo_2__
+                  cafInfo_3__ oneShotInfo_4__ inlinePragInfo_5__ occInfo_6__ strictnessInfo_7__
+                  demandInfo_8__ callArityInfo_9__ levityInfo_10__ := info in
+               Mk_IdInfo arityInfo_0__ ruleInfo_1__ unfoldingInfo_2__ cafInfo_3__
+                         oneShotInfo_4__ inlinePragInfo_5__ occInfo_6__ (zapUsageEnvSig (strictnessInfo
+                                                                                         info)) demandInfo_8__
+                         callArityInfo_9__ levityInfo_10__) else
+    None.
+
+Definition zapLamInfo : IdInfo -> option IdInfo :=
+  fun '((Mk_IdInfo _ _ _ _ _ _ occ _ demand _ _ as info)) =>
+    let is_safe_dmd := fun dmd => negb (isStrictDmd dmd) in
+    let safe_occ :=
+      match occ with
+      | BasicTypes.OneOcc _ _ _ _ =>
+          match occ with
+          | BasicTypes.ManyOccs _ =>
+              GHC.Err.error (GHC.Base.hs_string__ "Partial record update")
+          | BasicTypes.IAmDead =>
+              GHC.Err.error (GHC.Base.hs_string__ "Partial record update")
+          | BasicTypes.OneOcc occ_in_lam_2__ occ_one_br_3__ occ_int_cxt_4__
+          occ_tail_5__ =>
+              BasicTypes.OneOcc true occ_one_br_3__ occ_int_cxt_4__ BasicTypes.NoTailCallInfo
+          | BasicTypes.IAmALoopBreaker _ _ =>
+              GHC.Err.error (GHC.Base.hs_string__ "Partial record update")
+          end
+      | BasicTypes.IAmALoopBreaker _ _ =>
+          match occ with
+          | BasicTypes.ManyOccs occ_tail_12__ =>
+              BasicTypes.ManyOccs BasicTypes.NoTailCallInfo
+          | BasicTypes.IAmDead =>
+              GHC.Err.error (GHC.Base.hs_string__ "Partial record update")
+          | BasicTypes.OneOcc occ_in_lam_13__ occ_one_br_14__ occ_int_cxt_15__
+          occ_tail_16__ =>
+              BasicTypes.OneOcc occ_in_lam_13__ occ_one_br_14__ occ_int_cxt_15__
+                                BasicTypes.NoTailCallInfo
+          | BasicTypes.IAmALoopBreaker occ_rules_only_17__ occ_tail_18__ =>
+              BasicTypes.IAmALoopBreaker occ_rules_only_17__ BasicTypes.NoTailCallInfo
+          end
+      | _other => occ
+      end in
+    let is_safe_occ :=
+      fun arg_27__ =>
+        let 'occ := arg_27__ in
+        if BasicTypes.isAlwaysTailCalled occ : bool then false else
+        match arg_27__ with
+        | BasicTypes.OneOcc in_lam _ _ _ => in_lam
+        | _other => true
+        end in
+    if andb (is_safe_occ occ) (is_safe_dmd demand) : bool then None else
+    Some (let 'Mk_IdInfo arityInfo_31__ ruleInfo_32__ unfoldingInfo_33__
+             cafInfo_34__ oneShotInfo_35__ inlinePragInfo_36__ occInfo_37__
+             strictnessInfo_38__ demandInfo_39__ callArityInfo_40__ levityInfo_41__ :=
+            info in
+          Mk_IdInfo arityInfo_31__ ruleInfo_32__ unfoldingInfo_33__ cafInfo_34__
+                    oneShotInfo_35__ inlinePragInfo_36__ safe_occ strictnessInfo_38__ topDmd
+                    callArityInfo_40__ levityInfo_41__).
+
+Definition zapDemandInfo : IdInfo -> option IdInfo :=
+  fun info =>
+    Some (let 'Mk_IdInfo arityInfo_0__ ruleInfo_1__ unfoldingInfo_2__ cafInfo_3__
+             oneShotInfo_4__ inlinePragInfo_5__ occInfo_6__ strictnessInfo_7__ demandInfo_8__
+             callArityInfo_9__ levityInfo_10__ := info in
+          Mk_IdInfo arityInfo_0__ ruleInfo_1__ unfoldingInfo_2__ cafInfo_3__
+                    oneShotInfo_4__ inlinePragInfo_5__ occInfo_6__ strictnessInfo_7__ topDmd
+                    callArityInfo_9__ levityInfo_10__).
 
 Definition varUnique : Var -> Unique.Unique :=
   fun var => Unique.mkUniqueGrimily (realUnique var).
 
-Definition vanillaCprProdRes : BasicTypes.Arity -> DmdResult :=
-  fun _arity => Dunno RetProd.
-
 Definition vanillaCafInfo : CafInfo :=
   MayHaveCafRefs.
-
-Definition useTop : ArgUse :=
-  Mk_Use Many Used.
-
-Definition zap_usg : KillFlags -> UseDmd -> UseDmd :=
-  fix zap_usg (arg_0__ : KillFlags) (arg_1__ : UseDmd) : UseDmd
-        := let zap_musg (arg_0__ : KillFlags) (arg_1__ : ArgUse) : ArgUse :=
-             match arg_0__, arg_1__ with
-             | kfs, Abs => if kf_abs kfs : bool then useTop else Abs
-             | kfs, Mk_Use c u =>
-                 if kf_used_once kfs : bool then Mk_Use Many (zap_usg kfs u) else
-                 Mk_Use c (zap_usg kfs u)
-             end in
-           match arg_0__, arg_1__ with
-           | kfs, UCall c u =>
-               if kf_called_once kfs : bool then UCall Many (zap_usg kfs u) else
-               UCall c (zap_usg kfs u)
-           | _, _ =>
-               match arg_0__, arg_1__ with
-               | kfs, UProd us => UProd (GHC.Base.map (zap_musg kfs) us)
-               | _, u => u
-               end
-           end.
-
-Definition zap_musg : KillFlags -> ArgUse -> ArgUse :=
-  fun arg_0__ arg_1__ =>
-    match arg_0__, arg_1__ with
-    | kfs, Abs => if kf_abs kfs : bool then useTop else Abs
-    | kfs, Mk_Use c u =>
-        if kf_used_once kfs : bool then Mk_Use Many (zap_usg kfs u) else
-        Mk_Use c (zap_usg kfs u)
-    end.
-
-Definition useCount {u} : Use u -> Count :=
-  fun arg_0__ =>
-    match arg_0__ with
-    | Abs => One
-    | Mk_Use One _ => One
-    | _ => Many
-    end.
-
-Definition useBot : ArgUse :=
-  Abs.
 
 Definition updateVarTypeM {m} `{GHC.Base.Monad m}
    : (Type_ -> m Type_) -> Id -> m Id :=
@@ -3565,24 +4408,6 @@ Definition updateVarType : (Type_ -> Type_) -> Id -> Id :=
        id_info_5__ := id in
     Mk_Id varName_0__ realUnique_1__ (f (varType id)) idScope_3__ id_details_4__
           id_info_5__.
-
-Definition unwrapNewTyCon_maybe
-   : TyCon -> option (list TyVar * Type_ * CoAxiom Unbranched)%type :=
-  fun arg_0__ =>
-    match arg_0__ with
-    | AlgTyCon _ _ _ tvs _ _ _ _ _ _ _ (NewTyCon _ rhs _ co) _ _ =>
-        Some (pair (pair tvs rhs) co)
-    | _ => None
-    end.
-
-Definition unwrapNewTyConEtad_maybe
-   : TyCon -> option (list TyVar * Type_ * CoAxiom Unbranched)%type :=
-  fun arg_0__ =>
-    match arg_0__ with
-    | AlgTyCon _ _ _ _ _ _ _ _ _ _ _ (NewTyCon _ _ (pair tvs rhs) co) _ _ =>
-        Some (pair (pair tvs rhs) co)
-    | _ => None
-    end.
 
 Definition unknownArity : BasicTypes.Arity :=
   #0.
@@ -3650,309 +4475,6 @@ Definition updateTyVarKindM {m} `{(GHC.Base.Monad m)}
                             id_details_4__ id_info_5__ := tv in
                          Mk_Id varName_0__ realUnique_1__ k' idScope_3__ id_details_4__ id_info_5__)).
 
-Definition tyConTuple_maybe : TyCon -> option BasicTypes.TupleSort :=
-  fun arg_0__ =>
-    match arg_0__ with
-    | AlgTyCon _ _ _ _ _ _ _ _ _ _ _ rhs _ _ =>
-        match rhs with
-        | TupleTyCon _ sort => Some sort
-        | _ => None
-        end
-    | _ => None
-    end.
-
-Definition tyConStupidTheta : TyCon -> list PredType :=
-  fun arg_0__ =>
-    match arg_0__ with
-    | AlgTyCon _ _ _ _ _ _ _ _ _ _ stupid _ _ _ => stupid
-    | tycon =>
-        Panic.panicStr (GHC.Base.hs_string__ "tyConStupidTheta") (Panic.someSDoc)
-    end.
-
-Definition tyConSingleDataCon_maybe : TyCon -> option DataCon :=
-  fun arg_0__ =>
-    match arg_0__ with
-    | AlgTyCon _ _ _ _ _ _ _ _ _ _ _ rhs _ _ =>
-        match rhs with
-        | DataTyCon (cons c nil) _ => Some c
-        | TupleTyCon c _ => Some c
-        | NewTyCon c _ _ _ => Some c
-        | _ => None
-        end
-    | _ => None
-    end.
-
-Definition tyConSingleDataCon : TyCon -> DataCon :=
-  fun tc =>
-    match tyConSingleDataCon_maybe tc with
-    | Some c => c
-    | None => Panic.panicStr (GHC.Base.hs_string__ "tyConDataCon") (Panic.someSDoc)
-    end.
-
-Definition tyConSingleAlgDataCon_maybe : TyCon -> option DataCon :=
-  fun arg_0__ =>
-    match arg_0__ with
-    | AlgTyCon _ _ _ _ _ _ _ _ _ _ _ rhs _ _ =>
-        match rhs with
-        | DataTyCon (cons c nil) _ => Some c
-        | TupleTyCon c _ => Some c
-        | _ => None
-        end
-    | _ => None
-    end.
-
-Definition tyConRoles : TyCon -> list Role :=
-  fun tc =>
-    let const_role := fun r => Coq.Lists.List.repeat r (tyConArity tc) in
-    match tc with
-    | FunTyCon _ _ _ _ _ _ _ => const_role Representational
-    | AlgTyCon _ _ _ _ _ _ _ roles _ _ _ _ _ _ => roles
-    | SynonymTyCon _ _ _ _ _ _ _ roles _ _ _ => roles
-    | FamilyTyCon _ _ _ _ _ _ _ _ _ _ _ => const_role Nominal
-    | PrimTyCon _ _ _ _ _ _ roles _ _ => roles
-    | PromotedDataCon _ _ _ _ _ _ roles _ _ _ => roles
-    | TcTyCon _ _ _ _ _ _ _ _ _ => const_role Nominal
-    end.
-
-Definition tyConRepName_maybe : TyCon -> option TyConRepName :=
-  fun arg_0__ =>
-    let j_3__ :=
-      match arg_0__ with
-      | FamilyTyCon _ _ _ _ _ _ _ _ (DataFamilyTyCon rep_nm) _ _ => Some rep_nm
-      | PromotedDataCon _ _ _ _ _ _ _ _ rep_nm _ => Some rep_nm
-      | _ => None
-      end in
-    match arg_0__ with
-    | FunTyCon _ _ _ _ _ _ rep_nm => Some rep_nm
-    | PrimTyCon _ _ _ _ _ _ _ _ mb_rep_nm => mb_rep_nm
-    | AlgTyCon _ _ _ _ _ _ _ _ _ _ _ _ _ parent =>
-        match parent with
-        | VanillaAlgTyCon rep_nm => Some rep_nm
-        | _ =>
-            match parent with
-            | ClassTyCon _ rep_nm => Some rep_nm
-            | _ => match parent with | UnboxedAlgTyCon rep_nm => rep_nm | _ => j_3__ end
-            end
-        end
-    | _ => j_3__
-    end.
-
-Definition tyConRepModOcc
-   : Module.Module -> OccName.OccName -> (Module.Module * OccName.OccName)%type :=
-  fun tc_module tc_occ =>
-    let rep_module :=
-      if tc_module GHC.Base.== PrelNames.gHC_PRIM : bool then PrelNames.gHC_TYPES else
-      tc_module in
-    pair rep_module (OccName.mkTyConRepOcc tc_occ).
-
-Axiom tyConInjectivityInfo : TyCon -> Injectivity.
-
-Definition tyConFlavour : TyCon -> TyConFlavour :=
-  fun arg_0__ =>
-    match arg_0__ with
-    | AlgTyCon _ _ _ _ _ _ _ _ _ _ _ rhs _ parent =>
-        match parent with
-        | ClassTyCon _ _ => ClassFlavour
-        | _ =>
-            match rhs with
-            | TupleTyCon _ sort => TupleFlavour (BasicTypes.tupleSortBoxity sort)
-            | SumTyCon _ => SumFlavour
-            | DataTyCon _ _ => DataTypeFlavour
-            | NewTyCon _ _ _ _ => NewtypeFlavour
-            | AbstractTyCon => AbstractTypeFlavour
-            end
-        end
-    | FamilyTyCon _ _ _ _ _ _ _ _ flav _ _ =>
-        match flav with
-        | DataFamilyTyCon _ => DataFamilyFlavour
-        | OpenSynFamilyTyCon => OpenTypeFamilyFlavour
-        | ClosedSynFamilyTyCon _ => ClosedTypeFamilyFlavour
-        | AbstractClosedSynFamilyTyCon => ClosedTypeFamilyFlavour
-        | BuiltInSynFamTyCon _ => ClosedTypeFamilyFlavour
-        end
-    | SynonymTyCon _ _ _ _ _ _ _ _ _ _ _ => TypeSynonymFlavour
-    | FunTyCon _ _ _ _ _ _ _ => BuiltInTypeFlavour
-    | PrimTyCon _ _ _ _ _ _ _ _ _ => BuiltInTypeFlavour
-    | PromotedDataCon _ _ _ _ _ _ _ _ _ _ => PromotedDataConFlavour
-    | TcTyCon _ _ _ _ _ _ _ _ flav => flav
-    end.
-
-Definition tyConFamilySizeAtMost : TyCon -> nat -> bool :=
-  fun arg_0__ arg_1__ =>
-    match arg_0__, arg_1__ with
-    | (AlgTyCon _ _ _ _ _ _ _ _ _ _ _ rhs _ _ as tc), n =>
-        match rhs with
-        | DataTyCon cons_ _ => Util.lengthAtMost cons_ n
-        | NewTyCon _ _ _ _ => #1 GHC.Base.<= n
-        | TupleTyCon _ _ => #1 GHC.Base.<= n
-        | SumTyCon cons_ => Util.lengthAtMost cons_ n
-        | _ =>
-            Panic.panicStr (GHC.Base.hs_string__ "tyConFamilySizeAtMost 1") (Panic.someSDoc)
-        end
-    | tc, _ =>
-        Panic.panicStr (GHC.Base.hs_string__ "tyConFamilySizeAtMost 2") (Panic.someSDoc)
-    end.
-
-Definition tyConFamilySize : TyCon -> nat :=
-  fun arg_0__ =>
-    match arg_0__ with
-    | (AlgTyCon _ _ _ _ _ _ _ _ _ _ _ rhs _ _ as tc) =>
-        match rhs with
-        | DataTyCon cons_ _ => Coq.Lists.List.length cons_
-        | NewTyCon _ _ _ _ => #1
-        | TupleTyCon _ _ => #1
-        | SumTyCon cons_ => Coq.Lists.List.length cons_
-        | _ =>
-            Panic.panicStr (GHC.Base.hs_string__ "tyConFamilySize 1") (Panic.someSDoc)
-        end
-    | tc =>
-        Panic.panicStr (GHC.Base.hs_string__ "tyConFamilySize 2") (Panic.someSDoc)
-    end.
-
-Definition tyConFamilyResVar_maybe : TyCon -> option Name.Name :=
-  fun arg_0__ =>
-    match arg_0__ with
-    | FamilyTyCon _ _ _ _ _ _ _ res _ _ _ => res
-    | _ => None
-    end.
-
-Definition tyConFamilyCoercion_maybe : TyCon -> option (CoAxiom Unbranched) :=
-  fun arg_0__ =>
-    match arg_0__ with
-    | AlgTyCon _ _ _ _ _ _ _ _ _ _ _ _ _ (DataFamInstTyCon ax _ _) => Some ax
-    | _ => None
-    end.
-
-Definition tyConFamInst_maybe : TyCon -> option (TyCon * list Type_)%type :=
-  fun arg_0__ =>
-    match arg_0__ with
-    | AlgTyCon _ _ _ _ _ _ _ _ _ _ _ _ _ (DataFamInstTyCon _ f ts) =>
-        Some (pair f ts)
-    | _ => None
-    end.
-
-Definition tyConFamInstSig_maybe
-   : TyCon -> option (TyCon * list Type_ * CoAxiom Unbranched)%type :=
-  fun arg_0__ =>
-    match arg_0__ with
-    | AlgTyCon _ _ _ _ _ _ _ _ _ _ _ _ _ (DataFamInstTyCon ax f ts) =>
-        Some (pair (pair f ts) ax)
-    | _ => None
-    end.
-
-Definition tyConDataCons_maybe : TyCon -> option (list DataCon) :=
-  fun arg_0__ =>
-    match arg_0__ with
-    | AlgTyCon _ _ _ _ _ _ _ _ _ _ _ rhs _ _ =>
-        match rhs with
-        | DataTyCon cons_ _ => Some cons_
-        | NewTyCon con _ _ _ => Some (cons con nil)
-        | TupleTyCon con _ => Some (cons con nil)
-        | SumTyCon cons_ => Some cons_
-        | _ => None
-        end
-    | _ => None
-    end.
-
-Definition tyConDataCons : TyCon -> list DataCon :=
-  fun tycon => Maybes.orElse (tyConDataCons_maybe tycon) nil.
-
-Definition tyConClass_maybe : TyCon -> option Class :=
-  fun arg_0__ =>
-    match arg_0__ with
-    | AlgTyCon _ _ _ _ _ _ _ _ _ _ _ _ _ (ClassTyCon clas _) => Some clas
-    | _ => None
-    end.
-
-Definition tyConCType_maybe : TyCon -> option unit :=
-  fun arg_0__ =>
-    match arg_0__ with
-    | (AlgTyCon _ _ _ _ _ _ _ _ _ _ _ _ _ _ as tc) => tyConCType tc
-    | _ => None
-    end.
-
-Definition tyConBinderArgFlag : TyConBinder -> ArgFlag :=
-  fun arg_0__ =>
-    match arg_0__ with
-    | TvBndr _ (NamedTCB vis) => vis
-    | TvBndr _ AnonTCB => Required
-    end.
-
-Definition tyConAssoc_maybe : TyCon -> option Class :=
-  fun arg_0__ =>
-    match arg_0__ with
-    | FamilyTyCon _ _ _ _ _ _ _ _ _ mb_cls _ => mb_cls
-    | _ => None
-    end.
-
-Axiom tyConATs : TyCon -> list TyCon.
-
-Definition trimCPRInfo : bool -> bool -> DmdResult -> DmdResult :=
-  fun trim_all trim_sums res =>
-    let trimC :=
-      fun arg_0__ =>
-        match arg_0__ with
-        | RetSum n => if orb trim_all trim_sums : bool then NoCPR else RetSum n
-        | RetProd => if trim_all : bool then NoCPR else RetProd
-        | NoCPR => NoCPR
-        end in
-    let trimR :=
-      fun arg_5__ =>
-        match arg_5__ with
-        | Dunno c => Dunno (trimC c)
-        | res => res
-        end in
-    trimR res.
-
-Definition strBot : ArgStr :=
-  Mk_Str VanStr HyperStr.
-
-Definition botDmd : Demand :=
-  JD strBot useBot.
-
-Definition topDmd : Demand :=
-  JD Lazy useTop.
-
-Definition resTypeArgDmd {r} : Termination r -> Demand :=
-  fun arg_0__ => match arg_0__ with | Dunno _ => topDmd | _ => botDmd end.
-
-Definition topRes : DmdResult :=
-  Dunno NoCPR.
-
-Definition zapDemandInfo : IdInfo -> option IdInfo :=
-  fun info =>
-    Some (let 'Mk_IdInfo arityInfo_0__ ruleInfo_1__ unfoldingInfo_2__ cafInfo_3__
-             oneShotInfo_4__ inlinePragInfo_5__ occInfo_6__ strictnessInfo_7__ demandInfo_8__
-             callArityInfo_9__ levityInfo_10__ := info in
-          Mk_IdInfo arityInfo_0__ ruleInfo_1__ unfoldingInfo_2__ cafInfo_3__
-                    oneShotInfo_4__ inlinePragInfo_5__ occInfo_6__ strictnessInfo_7__ topDmd
-                    callArityInfo_9__ levityInfo_10__).
-
-Definition toBothDmdArg : DmdType -> BothDmdArg :=
-  fun '(Mk_DmdType fv _ r) =>
-    let go :=
-      fun arg_1__ =>
-        match arg_1__ with
-        | Dunno _ => Dunno tt
-        | ThrowsExn => ThrowsExn
-        | Diverges => Diverges
-        end in
-    pair fv (go r).
-
-Definition tidyPatSynIds : (Id -> Id) -> PatSyn -> PatSyn :=
-  fun arg_0__ arg_1__ =>
-    match arg_0__, arg_1__ with
-    | tidy_fn, (MkPatSyn _ _ _ _ _ _ _ _ _ _ _ matcher builder as ps) =>
-        let tidy_pr := fun '(pair id dummy) => pair (tidy_fn id) dummy in
-        let 'MkPatSyn psName_5__ psUnique_6__ psArgs_7__ psArity_8__ psInfix_9__
-           psFieldLabels_10__ psUnivTyVars_11__ psReqTheta_12__ psExTyVars_13__
-           psProvTheta_14__ psResultTy_15__ psMatcher_16__ psBuilder_17__ := ps in
-        MkPatSyn psName_5__ psUnique_6__ psArgs_7__ psArity_8__ psInfix_9__
-                 psFieldLabels_10__ psUnivTyVars_11__ psReqTheta_12__ psExTyVars_13__
-                 psProvTheta_14__ psResultTy_15__ (tidy_pr matcher) (GHC.Base.fmap tidy_pr
-                  builder)
-    end.
-
 Definition tickishScoped {id} : Tickish id -> TickishScoping :=
   fun arg_0__ =>
     match arg_0__ with
@@ -3994,105 +4516,6 @@ Axiom tickishCounts : forall {id}, Tickish id -> bool.
 
 Definition tickishFloatable {id} : Tickish id -> bool :=
   fun t => andb (tickishScopesLike t SoftScope) (negb (tickishCounts t)).
-
-Definition tcFlavourIsOpen : TyConFlavour -> bool :=
-  fun arg_0__ =>
-    match arg_0__ with
-    | DataFamilyFlavour => true
-    | OpenTypeFamilyFlavour => true
-    | ClosedTypeFamilyFlavour => false
-    | ClassFlavour => false
-    | DataTypeFlavour => false
-    | NewtypeFlavour => false
-    | TupleFlavour _ => false
-    | SumFlavour => false
-    | AbstractTypeFlavour => false
-    | BuiltInTypeFlavour => false
-    | PromotedDataConFlavour => false
-    | TypeSynonymFlavour => false
-    end.
-
-Definition tcFlavourCanBeUnsaturated : TyConFlavour -> bool :=
-  fun arg_0__ =>
-    match arg_0__ with
-    | ClassFlavour => true
-    | DataTypeFlavour => true
-    | NewtypeFlavour => true
-    | DataFamilyFlavour => true
-    | TupleFlavour _ => true
-    | SumFlavour => true
-    | AbstractTypeFlavour => true
-    | BuiltInTypeFlavour => true
-    | PromotedDataConFlavour => true
-    | TypeSynonymFlavour => false
-    | OpenTypeFamilyFlavour => false
-    | ClosedTypeFamilyFlavour => false
-    end.
-
-Definition synTyConRhs_maybe : TyCon -> option Type_ :=
-  fun arg_0__ =>
-    match arg_0__ with
-    | SynonymTyCon _ _ _ _ _ _ _ _ rhs _ _ => Some rhs
-    | _ => None
-    end.
-
-Definition synTyConDefn_maybe : TyCon -> option (list TyVar * Type_)%type :=
-  fun arg_0__ =>
-    match arg_0__ with
-    | SynonymTyCon _ _ _ tyvars _ _ _ _ ty _ _ => Some (pair tyvars ty)
-    | _ => None
-    end.
-
-Definition strictenDmd : Demand -> CleanDemand :=
-  fun '(JD s u) =>
-    let poke_u :=
-      fun arg_1__ => match arg_1__ with | Abs => UHead | Mk_Use _ u => u end in
-    let poke_s :=
-      fun arg_3__ => match arg_3__ with | Lazy => HeadStr | Mk_Str _ s => s end in
-    JD (poke_s s) (poke_u u).
-
-Definition strictSigDmdEnv : StrictSig -> DmdEnv :=
-  fun '(Mk_StrictSig (Mk_DmdType env _ _)) => env.
-
-Definition strictApply1Dmd : Demand :=
-  JD (Mk_Str VanStr (SCall HeadStr)) (Mk_Use Many (UCall One Used)).
-
-Definition strTop : ArgStr :=
-  Lazy.
-
-Definition splitUseProdDmd : nat -> UseDmd -> option (list ArgUse) :=
-  fun arg_0__ arg_1__ =>
-    match arg_0__, arg_1__ with
-    | n, Used => Some (Coq.Lists.List.repeat useTop n)
-    | n, UHead => Some (Coq.Lists.List.repeat Abs n)
-    | n, UProd ds =>
-        Panic.warnPprTrace (negb (Util.lengthIs ds n)) (GHC.Base.hs_string__
-                            "ghc/compiler/basicTypes/Demand.hs") #645 (Datatypes.id (GHC.Base.hs_string__
-                                                                                     "splitUseProdDmd")) (Some ds)
-    | _, UCall _ _ => None
-    end.
-
-Definition splitStrictSig : StrictSig -> (list Demand * DmdResult)%type :=
-  fun '(Mk_StrictSig (Mk_DmdType _ dmds res)) => pair dmds res.
-
-Definition splitStrProdDmd : nat -> StrDmd -> option (list ArgStr) :=
-  fun arg_0__ arg_1__ =>
-    match arg_0__, arg_1__ with
-    | n, HyperStr => Some (Coq.Lists.List.repeat strBot n)
-    | n, HeadStr => Some (Coq.Lists.List.repeat strTop n)
-    | n, SProd ds =>
-        Panic.warnPprTrace (negb (Util.lengthIs ds n)) (GHC.Base.hs_string__
-                            "ghc/compiler/basicTypes/Demand.hs") #359 (Datatypes.id (GHC.Base.hs_string__
-                                                                                     "splitStrProdDmd")) (Some ds)
-    | _, SCall _ => None
-    end.
-
-Definition splitArgStrProdDmd : nat -> ArgStr -> option (list ArgStr) :=
-  fun arg_0__ arg_1__ =>
-    match arg_0__, arg_1__ with
-    | n, Lazy => Some (Coq.Lists.List.repeat Lazy n)
-    | n, Mk_Str _ s => splitStrProdDmd n s
-    end.
 
 Definition sizeVarSet : VarSet -> nat :=
   UniqSet.sizeUniqSet.
@@ -4291,69 +4714,8 @@ Definition setArityInfo : IdInfo -> ArityInfo -> IdInfo :=
 Definition seqVarSet : VarSet -> unit :=
   fun s => GHC.Prim.seq (sizeVarSet s) tt.
 
-Definition seqUseDmd : UseDmd -> unit :=
-  fun x => tt.
-
-Definition seqStrictSig : StrictSig -> unit :=
-  fun x => tt.
-
-Definition seqStrDmdList : list ArgStr -> unit :=
-  fun x => tt.
-
-Definition seqStrDmd : StrDmd -> unit :=
-  fun x => tt.
-
-Definition seqDmdType : DmdType -> unit :=
-  fun x => tt.
-
-Definition seqDmdResult : DmdResult -> unit :=
-  fun x => tt.
-
-Definition seqDmdEnv : DmdEnv -> unit :=
-  fun x => tt.
-
-Definition seqDmd : Demand :=
-  JD (Mk_Str VanStr HeadStr) (Mk_Use One UHead).
-
-Definition seqDemandList : list Demand -> unit :=
-  fun x => tt.
-
-Definition seqDemand : Demand -> unit :=
-  fun x => tt.
-
 Definition seqDVarSet : DVarSet -> unit :=
   fun s => GHC.Prim.seq (sizeDVarSet s) tt.
-
-Definition seqCPRResult : CPRResult -> unit :=
-  fun x => tt.
-
-Definition seqArgUseList : list ArgUse -> unit :=
-  fun x => tt.
-
-Definition seqArgUse : ArgUse -> unit :=
-  fun x => tt.
-
-Definition seqArgStr : ArgStr -> unit :=
-  fun x => tt.
-
-Definition saturatedByOneShots : nat -> Demand -> bool :=
-  fun arg_0__ arg_1__ =>
-    match arg_0__, arg_1__ with
-    | n, JD _ usg =>
-        let fix go arg_2__ arg_3__
-                  := match arg_2__, arg_3__ with
-                     | num_4__, _ =>
-                         if num_4__ GHC.Base.== #0 : bool then true else
-                         match arg_2__, arg_3__ with
-                         | n, UCall One u => go (n GHC.Num.- #1) u
-                         | _, _ => false
-                         end
-                     end in
-        match usg with
-        | Mk_Use _ arg_usg => go n arg_usg
-        | _ => false
-        end
-    end.
 
 Definition sameVis : ArgFlag -> ArgFlag -> bool :=
   fun arg_0__ arg_1__ =>
@@ -4420,59 +4782,6 @@ Definition rhssOfAlts {b} : list (Alt b) -> list (Expr b) :=
     let cont_0__ arg_1__ := let 'pair (pair _ _) e := arg_1__ in cons e nil in
     Coq.Lists.List.flat_map cont_0__ alts.
 
-Definition retCPR_maybe : CPRResult -> option BasicTypes.ConTag :=
-  fun arg_0__ =>
-    match arg_0__ with
-    | RetSum t => Some t
-    | RetProd => Some BasicTypes.fIRST_TAG
-    | NoCPR => None
-    end.
-
-Definition returnsCPR_maybe : DmdResult -> option BasicTypes.ConTag :=
-  fun arg_0__ => match arg_0__ with | Dunno c => retCPR_maybe c | _ => None end.
-
-Definition promoteDataCon : DataCon -> TyCon :=
-  fun '(MkData _ _ _ _ _ _ _ _ _ _ _ _ _ _ _ _ _ _ _ _ _ tc) => tc.
-
-Definition primRepIsFloat : PrimRep -> option bool :=
-  fun arg_0__ =>
-    match arg_0__ with
-    | FloatRep => Some true
-    | DoubleRep => Some true
-    | VecRep _ _ => None
-    | _ => Some false
-    end.
-
-Definition primElemRepSizeB : PrimElemRep -> nat :=
-  fun arg_0__ =>
-    match arg_0__ with
-    | Int8ElemRep => #1
-    | Int16ElemRep => #2
-    | Int32ElemRep => #4
-    | Int64ElemRep => #8
-    | Word8ElemRep => #1
-    | Word16ElemRep => #2
-    | Word32ElemRep => #4
-    | Word64ElemRep => #8
-    | FloatElemRep => #4
-    | DoubleElemRep => #8
-    end.
-
-Definition pprPromotionQuote : TyCon -> GHC.Base.String :=
-  fun tc =>
-    match tc with
-    | PromotedDataCon _ _ _ _ _ _ _ _ _ _ => Panic.someSDoc
-    | _ => Panic.someSDoc
-    end.
-
-Definition postProcessDmdResult : Str unit -> DmdResult -> DmdResult :=
-  fun arg_0__ arg_1__ =>
-    match arg_0__, arg_1__ with
-    | Lazy, _ => topRes
-    | Mk_Str Mk_ExnStr _, ThrowsExn => topRes
-    | _, res => res
-    end.
-
 Definition plusVarEnv_CD {a}
    : (a -> a -> a) -> VarEnv a -> a -> VarEnv a -> a -> VarEnv a :=
   UniqFM.plusUFM_CD.
@@ -4498,96 +4807,6 @@ Definition plusDVarEnv_C {a}
 Definition plusDVarEnv {a} : DVarEnv a -> DVarEnv a -> DVarEnv a :=
   UniqDFM.plusUDFM.
 
-Definition peelUseCall : UseDmd -> option (Count * UseDmd)%type :=
-  fun arg_0__ =>
-    match arg_0__ with
-    | UCall c u => Some (pair c u)
-    | _ => None
-    end.
-
-Program Definition peelManyCalls : nat -> CleanDemand -> DmdShell :=
-          fun arg_0__ arg_1__ =>
-            match arg_0__, arg_1__ with
-            | n, JD str abs =>
-                let go_abs : nat -> UseDmd -> Use unit :=
-                  GHC.Wf.wfFix2 Coq.Init.Peano.lt (fun (arg_2__ : nat) (arg_3__ : UseDmd) =>
-                                   arg_2__) _ (fun (arg_2__ : nat) (arg_3__ : UseDmd) go_abs =>
-                                   match arg_2__, arg_3__ with
-                                   | num_4__, _ =>
-                                       if Bool.Sumbool.sumbool_of_bool (num_4__ GHC.Base.== #0) then Mk_Use One tt else
-                                       match arg_2__, arg_3__ with
-                                       | n, UCall One d' => go_abs (n GHC.Num.- #1) d'
-                                       | _, _ => Mk_Use Many tt
-                                       end
-                                   end) in
-                let go_str : nat -> StrDmd -> Str unit :=
-                  GHC.Wf.wfFix2 Coq.Init.Peano.lt (fun (arg_10__ : nat) (arg_11__ : StrDmd) =>
-                                   arg_10__) _ (fun (arg_10__ : nat) (arg_11__ : StrDmd) go_str =>
-                                   match arg_10__, arg_11__ with
-                                   | num_12__, _ =>
-                                       if Bool.Sumbool.sumbool_of_bool (num_12__ GHC.Base.== #0)
-                                       then Mk_Str VanStr tt else
-                                       match arg_10__, arg_11__ with
-                                       | _, HyperStr => Mk_Str VanStr tt
-                                       | n, SCall d' => go_str (n GHC.Num.- #1) d'
-                                       | _, _ => Lazy
-                                       end
-                                   end) in
-                JD (go_str n str) (go_abs n abs)
-            end.
-Solve Obligations with (solve_dmdTransform).
-
-Definition peelCallDmd : CleanDemand -> (CleanDemand * DmdShell)%type :=
-  fun '(JD s u) =>
-    let 'pair u' us := (match u with
-                          | UCall c u' => pair u' (Mk_Use c tt)
-                          | _ => pair Used (Mk_Use Many tt)
-                          end) in
-    let 'pair s' ss := (match s with
-                          | SCall s' => pair s' (Mk_Str VanStr tt)
-                          | HyperStr => pair HyperStr (Mk_Str VanStr tt)
-                          | _ => pair HeadStr Lazy
-                          end) in
-    pair (JD s' u') (JD ss us).
-
-Definition patSynUnivTyVarBinders : PatSyn -> list TyVarBinder :=
-  psUnivTyVars.
-
-Definition patSynName : PatSyn -> Name.Name :=
-  psName.
-
-Definition patSynMatcher : PatSyn -> (Id * bool)%type :=
-  psMatcher.
-
-Definition patSynIsInfix : PatSyn -> bool :=
-  psInfix.
-
-Definition patSynFieldType : PatSyn -> FieldLabel.FieldLabelString -> Type_ :=
-  fun ps label =>
-    match Data.Foldable.find ((fun arg_0__ => arg_0__ GHC.Base.== label) GHC.Base.∘
-                              (FieldLabel.flLabel GHC.Base.∘ Data.Tuple.fst)) (GHC.List.zip (psFieldLabels ps)
-                                                                                            (psArgs ps)) with
-    | Some (pair _ ty) => ty
-    | None =>
-        Panic.panicStr (GHC.Base.hs_string__ "dataConFieldType") (GHC.Base.mappend
-                                                                  Panic.someSDoc Panic.someSDoc)
-    end.
-
-Definition patSynFieldLabels : PatSyn -> list FieldLabel.FieldLabel :=
-  psFieldLabels.
-
-Definition patSynExTyVarBinders : PatSyn -> list TyVarBinder :=
-  psExTyVars.
-
-Definition patSynBuilder : PatSyn -> option (Id * bool)%type :=
-  psBuilder.
-
-Definition patSynArity : PatSyn -> BasicTypes.Arity :=
-  psArity.
-
-Definition patSynArgs : PatSyn -> list Type_ :=
-  psArgs.
-
 Definition partitionVarEnv {a}
    : (a -> bool) -> VarEnv a -> (VarEnv a * VarEnv a)%type :=
   UniqFM.partitionUFM.
@@ -4603,22 +4822,6 @@ Definition partitionDVarEnv {a}
 Definition otherCons : Unfolding -> list AltCon :=
   fun arg_0__ => nil.
 
-Definition oneifyDmd : Demand -> Demand :=
-  fun arg_0__ =>
-    match arg_0__ with
-    | JD s (Mk_Use _ a) => JD s (Mk_Use One a)
-    | jd => jd
-    end.
-
-Definition okParent : Name.Name -> AlgTyConFlav -> bool :=
-  fun arg_0__ arg_1__ =>
-    match arg_0__, arg_1__ with
-    | _, VanillaAlgTyCon _ => true
-    | _, UnboxedAlgTyCon _ => true
-    | tc_name, ClassTyCon cls _ => tc_name GHC.Base.== tyConName (classTyCon cls)
-    | _, DataFamInstTyCon _ fam_tc tys => Util.lengthAtLeast tys (tyConArity fam_tc)
-    end.
-
 Definition notOrphan : IsOrphan -> bool :=
   fun arg_0__ => match arg_0__ with | NotOrphan _ => true | _ => false end.
 
@@ -4627,51 +4830,6 @@ Definition nonDetCmpVar : Var -> Var -> comparison :=
 
 Definition noUnfolding : Unfolding :=
   NoUnfolding.
-
-Definition newTyConRhs : TyCon -> (list TyVar * Type_)%type :=
-  fun arg_0__ =>
-    match arg_0__ with
-    | AlgTyCon _ _ _ tvs _ _ _ _ _ _ _ (NewTyCon _ rhs _ _) _ _ => pair tvs rhs
-    | tycon => Panic.panicStr (GHC.Base.hs_string__ "newTyConRhs") (Panic.someSDoc)
-    end.
-
-Definition newTyConEtadRhs : TyCon -> (list TyVar * Type_)%type :=
-  fun arg_0__ =>
-    match arg_0__ with
-    | AlgTyCon _ _ _ _ _ _ _ _ _ _ _ (NewTyCon _ _ tvs_rhs _) _ _ => tvs_rhs
-    | tycon =>
-        Panic.panicStr (GHC.Base.hs_string__ "newTyConEtadRhs") (Panic.someSDoc)
-    end.
-
-Definition newTyConEtadArity : TyCon -> nat :=
-  fun arg_0__ =>
-    match arg_0__ with
-    | AlgTyCon _ _ _ _ _ _ _ _ _ _ _ (NewTyCon _ _ tvs_rhs _) _ _ =>
-        Coq.Lists.List.length (Data.Tuple.fst tvs_rhs)
-    | tycon =>
-        Panic.panicStr (GHC.Base.hs_string__ "newTyConEtadArity") (Panic.someSDoc)
-    end.
-
-Definition newTyConDataCon_maybe : TyCon -> option DataCon :=
-  fun arg_0__ =>
-    match arg_0__ with
-    | AlgTyCon _ _ _ _ _ _ _ _ _ _ _ (NewTyCon con _ _ _) _ _ => Some con
-    | _ => None
-    end.
-
-Definition newTyConCo_maybe : TyCon -> option (CoAxiom Unbranched) :=
-  fun arg_0__ =>
-    match arg_0__ with
-    | AlgTyCon _ _ _ _ _ _ _ _ _ _ _ (NewTyCon _ _ _ co) _ _ => Some co
-    | _ => None
-    end.
-
-Definition newTyConCo : TyCon -> CoAxiom Unbranched :=
-  fun tc =>
-    match newTyConCo_maybe tc with
-    | Some co => co
-    | None => Panic.panicStr (GHC.Base.hs_string__ "newTyConCo") (Panic.someSDoc)
-    end.
 
 Definition neverUnfoldGuidance : UnfoldingGuidance -> bool :=
   fun arg_0__ => match arg_0__ with | UnfNever => true | _ => false end.
@@ -4710,100 +4868,11 @@ Definition zipVarEnv {a} : list Var -> list a -> VarEnv a :=
   fun tyvars tys =>
     mkVarEnv (Util.zipEqual (GHC.Base.hs_string__ "zipVarEnv") tyvars tys).
 
-Local Definition Eq___Count_op_zeze__ : Count -> Count -> bool :=
-  fun arg_0__ arg_1__ =>
-    match arg_0__, arg_1__ with
-    | One, One => true
-    | Many, Many => true
-    | _, _ => false
-    end.
-
-Local Definition Eq___Count_op_zsze__ : Count -> Count -> bool :=
-  fun x y => negb (Eq___Count_op_zeze__ x y).
-
-Program Instance Eq___Count : GHC.Base.Eq_ Count :=
-  fun _ k__ =>
-    k__ {| GHC.Base.op_zeze____ := Eq___Count_op_zeze__ ;
-           GHC.Base.op_zsze____ := Eq___Count_op_zsze__ |}.
-
-Local Definition Eq___Use_op_zeze__ {inst_u} `{GHC.Base.Eq_ inst_u}
-   : Use inst_u -> Use inst_u -> bool :=
-  fun arg_0__ arg_1__ =>
-    match arg_0__, arg_1__ with
-    | Abs, Abs => true
-    | Mk_Use a1 a2, Mk_Use b1 b2 =>
-        (andb ((a1 GHC.Base.== b1)) ((a2 GHC.Base.== b2)))
-    | _, _ => false
-    end.
-
-Local Definition Eq___Use_op_zsze__ {inst_u} `{GHC.Base.Eq_ inst_u}
-   : Use inst_u -> Use inst_u -> bool :=
-  fun x y => negb (Eq___Use_op_zeze__ x y).
-
-Program Instance Eq___Use {u} `{GHC.Base.Eq_ u} : GHC.Base.Eq_ (Use u) :=
-  fun _ k__ =>
-    k__ {| GHC.Base.op_zeze____ := Eq___Use_op_zeze__ ;
-           GHC.Base.op_zsze____ := Eq___Use_op_zsze__ |}.
-
-Local Definition Eq___UseDmd_op_zeze__ : UseDmd -> UseDmd -> bool :=
-  fix UseDmd_eq x y
-        := let eq' : GHC.Base.Eq_ UseDmd := GHC.Base.eq_default UseDmd_eq in
-           match x, y with
-           | UCall a1 a2, UCall b1 b2 => andb (a1 GHC.Base.== b1) (a2 GHC.Base.== b2)
-           | UProd a1, UProd b1 => a1 GHC.Base.== b1
-           | UHead, UHead => true
-           | Used, Used => true
-           | _, _ => false
-           end.
-
-Local Definition Eq___UseDmd_op_zsze__ : UseDmd -> UseDmd -> bool :=
-  fun x y => negb (Eq___UseDmd_op_zeze__ x y).
-
-Program Instance Eq___UseDmd : GHC.Base.Eq_ UseDmd :=
-  fun _ k__ =>
-    k__ {| GHC.Base.op_zeze____ := Eq___UseDmd_op_zeze__ ;
-           GHC.Base.op_zsze____ := Eq___UseDmd_op_zsze__ |}.
-
-Definition mkUProd : list ArgUse -> UseDmd :=
-  fun ux =>
-    if Data.Foldable.all (fun arg_0__ => arg_0__ GHC.Base.== Abs) ux : bool
-    then UHead else
-    UProd ux.
-
-Definition mkUCall : Count -> UseDmd -> UseDmd :=
-  fun c a => UCall c a.
-
-Program Definition mkWorkerDemand : nat -> Demand :=
-          fun n =>
-            let go :=
-              GHC.Wf.wfFix1 Coq.Init.Peano.lt (fun arg_0__ => arg_0__) _ (fun arg_0__ go =>
-                               let 'num_1__ := arg_0__ in
-                               if Bool.Sumbool.sumbool_of_bool (num_1__ GHC.Base.== #0) then Used else
-                               let 'n := arg_0__ in
-                               mkUCall One (go (n GHC.Num.- #1))) in
-            JD Lazy (Mk_Use One (go n)).
-Solve Obligations with (solve_mkWorkerDemand).
-
 Definition mkTyVarBinder : ArgFlag -> Var -> TyVarBinder :=
   fun vis var => TvBndr var vis.
 
 Definition mkTyVarBinders : ArgFlag -> list TyVar -> list TyVarBinder :=
   fun vis => GHC.Base.map (mkTyVarBinder vis).
-
-Definition tyConTyVarBinders : list TyConBinder -> list TyVarBinder :=
-  fun tc_bndrs =>
-    let mk_binder :=
-      fun '(TvBndr tv tc_vis) =>
-        let vis :=
-          match tc_vis with
-          | AnonTCB => Specified
-          | NamedTCB Required => Specified
-          | NamedTCB vis => vis
-          end in
-        mkTyVarBinder vis tv in
-    GHC.Base.map mk_binder tc_bndrs.
-
-Axiom mkTyConKind : list TyConBinder -> Kind -> Kind.
 
 Definition mkTyBind : TyVar -> Type_ -> CoreBind :=
   fun tv ty => NonRec tv (Mk_Type ty).
@@ -4818,113 +4887,14 @@ Definition mkTyArg {b} : Type_ -> Expr b :=
 Definition mkTyApps {b} : Expr b -> list Type_ -> Expr b :=
   fun f args => Data.Foldable.foldl (fun e a => App e (mkTyArg a)) f args.
 
-Definition mkSumTyCon
-   : Name.Name ->
-     list TyConBinder ->
-     Kind ->
-     BasicTypes.Arity -> list TyVar -> list DataCon -> AlgTyConFlav -> TyCon :=
-  fun name binders res_kind arity tyvars cons_ parent =>
-    AlgTyCon (Name.nameUnique name) name binders tyvars res_kind (mkTyConKind
-              binders res_kind) arity (Coq.Lists.List.repeat Representational arity) None
-             false nil (SumTyCon cons_) FastStringEnv.emptyDFsEnv parent.
-
 Definition mkStringLit {b} : GHC.Base.String -> Expr b :=
   fun s => Lit (mkMachString s).
-
-Definition mkStrictSig : DmdType -> StrictSig :=
-  fun dmd_ty => Mk_StrictSig dmd_ty.
-
-Definition mkSCall : StrDmd -> StrDmd :=
-  fun arg_0__ => match arg_0__ with | HyperStr => HyperStr | s => SCall s end.
 
 Definition mkRuleEnv : RuleBase -> list Module.Module -> RuleEnv :=
   fun rules vis_orphs => Mk_RuleEnv rules (Module.mkModuleSet vis_orphs).
 
-Definition mkPromotedDataCon
-   : DataCon ->
-     Name.Name ->
-     TyConRepName ->
-     list TyConBinder -> Kind -> list Role -> RuntimeRepInfo -> TyCon :=
-  fun con name rep_name binders res_kind roles rep_info =>
-    PromotedDataCon (Name.nameUnique name) name binders res_kind (mkTyConKind
-                     binders res_kind) (Coq.Lists.List.length roles) roles con rep_name rep_info.
-
-Definition mkPrimTyCon'
-   : Name.Name ->
-     list TyConBinder -> Kind -> list Role -> bool -> option TyConRepName -> TyCon :=
-  fun name binders res_kind roles is_unlifted rep_nm =>
-    PrimTyCon (Name.nameUnique name) name binders res_kind (mkTyConKind binders
-               res_kind) (Coq.Lists.List.length roles) roles is_unlifted rep_nm.
-
-Definition mkPrelTyConRepName : Name.Name -> TyConRepName :=
-  fun tc_name =>
-    let name_uniq := Name.nameUnique tc_name in
-    let name_mod := Name.nameModule tc_name in
-    let name_occ := Name.nameOccName tc_name in
-    let rep_uniq :=
-      if OccName.isTcOcc name_occ : bool then Unique.tyConRepNameUnique name_uniq else
-      Unique.dataConRepNameUnique name_uniq in
-    let 'pair rep_mod rep_occ := tyConRepModOcc name_mod name_occ in
-    Name.mkExternalName rep_uniq rep_mod rep_occ (Name.nameSrcSpan tc_name).
-
-Definition mkPrimTyCon
-   : Name.Name -> list TyConBinder -> Kind -> list Role -> TyCon :=
-  fun name binders res_kind roles =>
-    mkPrimTyCon' name binders res_kind roles true (Some (mkPrelTyConRepName name)).
-
-Definition mkPatSyn
-   : Name.Name ->
-     bool ->
-     (list TyVarBinder * ThetaType)%type ->
-     (list TyVarBinder * ThetaType)%type ->
-     list Type_ ->
-     Type_ ->
-     (Id * bool)%type ->
-     option (Id * bool)%type -> list FieldLabel.FieldLabel -> PatSyn :=
-  fun arg_0__ arg_1__ arg_2__ arg_3__ arg_4__ arg_5__ arg_6__ arg_7__ arg_8__ =>
-    match arg_0__
-        , arg_1__
-        , arg_2__
-        , arg_3__
-        , arg_4__
-        , arg_5__
-        , arg_6__
-        , arg_7__
-        , arg_8__ with
-    | name
-    , declared_infix
-    , pair univ_tvs req_theta
-    , pair ex_tvs prov_theta
-    , orig_args
-    , orig_res_ty
-    , matcher
-    , builder
-    , field_labels =>
-        MkPatSyn name (Unique.getUnique name) orig_args (Coq.Lists.List.length
-                  orig_args) declared_infix field_labels univ_tvs req_theta ex_tvs prov_theta
-                 orig_res_ty matcher builder
-    end.
-
-Definition mkOnceUsedDmd : CleanDemand -> Demand :=
-  fun '(JD s a) => JD (Mk_Str VanStr s) (Mk_Use One a).
-
-Definition mkNamedTyConBinder : ArgFlag -> TyVar -> TyConBinder :=
-  fun vis tv => TvBndr tv (NamedTCB vis).
-
-Definition mkNamedTyConBinders : ArgFlag -> list TyVar -> list TyConBinder :=
-  fun vis tvs => GHC.Base.map (mkNamedTyConBinder vis) tvs.
-
-Definition mkManyUsedDmd : CleanDemand -> Demand :=
-  fun '(JD s a) => JD (Mk_Str VanStr s) (Mk_Use Many a).
-
 Definition mkLocalVar : IdDetails -> Name.Name -> Type_ -> IdInfo -> Id :=
   fun details name ty info => mk_id name ty (LocalId NotExported) details info.
-
-Definition mkLiftedPrimTyCon
-   : Name.Name -> list TyConBinder -> Kind -> list Role -> TyCon :=
-  fun name binders res_kind roles =>
-    let rep_nm := mkPrelTyConRepName name in
-    mkPrimTyCon' name binders res_kind roles false (Some rep_nm).
 
 Definition mkLetRec {b} : list (b * Expr b)%type -> Expr b -> Expr b :=
   fun arg_0__ arg_1__ =>
@@ -4949,58 +4919,11 @@ Definition mkLets {b} : list (Bind b) -> Expr b -> Expr b :=
 Definition mkLams {b} : list b -> Expr b -> Expr b :=
   fun binders body => Data.Foldable.foldr Lam body binders.
 
-Definition mkKindTyCon
-   : Name.Name -> list TyConBinder -> Kind -> list Role -> Name.Name -> TyCon :=
-  fun name binders res_kind roles rep_nm =>
-    let tc := mkPrimTyCon' name binders res_kind roles false (Some rep_nm) in tc.
-
-Definition mkJointDmd {s} {u} : s -> u -> JointDmd s u :=
-  fun s u => JD s u.
-
-Definition mkJointDmds {s} {u} : list s -> list u -> list (JointDmd s u) :=
-  fun ss as_ =>
-    Util.zipWithEqual (GHC.Base.hs_string__ "mkJointDmds") mkJointDmd ss as_.
-
-Definition splitProdDmd_maybe : Demand -> option (list Demand) :=
-  fun '(JD s u) =>
-    let scrut_1__ := pair s u in
-    let j_3__ :=
-      match scrut_1__ with
-      | pair Lazy (Mk_Use _ (UProd ux)) =>
-          Some (mkJointDmds (Coq.Lists.List.repeat Lazy (Coq.Lists.List.length ux)) ux)
-      | _ => None
-      end in
-    let j_5__ :=
-      match scrut_1__ with
-      | pair (Mk_Str _ s) (Mk_Use _ (UProd ux)) =>
-          match splitStrProdDmd (Coq.Lists.List.length ux) s with
-          | Some sx => Some (mkJointDmds sx ux)
-          | _ => j_3__
-          end
-      | _ => j_3__
-      end in
-    match scrut_1__ with
-    | pair (Mk_Str _ (SProd sx)) (Mk_Use _ u) =>
-        match splitUseProdDmd (Coq.Lists.List.length sx) u with
-        | Some ux => Some (mkJointDmds sx ux)
-        | _ => j_5__
-        end
-    | _ => j_5__
-    end.
-
 Definition mkInScopeSet : VarSet -> InScopeSet :=
   fun in_scope => InScope in_scope #1.
 
-Definition mkHeadStrict : CleanDemand -> CleanDemand :=
-  fun '(JD sd_0__ ud_1__) => JD HeadStr ud_1__.
-
 Definition mkGlobalVar : IdDetails -> Name.Name -> Type_ -> IdInfo -> Id :=
   fun details name ty info => mk_id name ty GlobalId details info.
-
-Definition mkFunTyCon : Name.Name -> list TyConBinder -> Name.Name -> TyCon :=
-  fun name binders rep_nm =>
-    FunTyCon (Name.nameUnique name) name binders liftedTypeKind (mkTyConKind binders
-              liftedTypeKind) (Coq.Lists.List.length binders) rep_nm.
 
 Definition mkFloatLit {b} : GHC.Real.Rational -> Expr b :=
   fun f => Lit (mkMachFloat f).
@@ -5009,14 +4932,8 @@ Definition mkExportedLocalVar
    : IdDetails -> Name.Name -> Type_ -> IdInfo -> Id :=
   fun details name ty info => mk_id name ty (LocalId Exported) details info.
 
-Definition mkEqSpec : TyVar -> Type_ -> EqSpec :=
-  fun tv ty => Mk_EqSpec tv ty.
-
 Definition mkDoubleLit {b} : GHC.Real.Rational -> Expr b :=
   fun d => Lit (mkMachDouble d).
-
-Definition mkDmdType : DmdEnv -> list Demand -> DmdResult -> DmdType :=
-  fun fv ds res => Mk_DmdType fv ds res.
 
 Definition mkCoBind : CoVar -> Coercion -> CoreBind :=
   fun cv co => NonRec cv (Mk_Coercion co).
@@ -5024,47 +4941,14 @@ Definition mkCoBind : CoVar -> Coercion -> CoreBind :=
 Definition mkCoApps {b} : Expr b -> list Coercion -> Expr b :=
   fun f args => Data.Foldable.foldl (fun e a => App e (Mk_Coercion a)) f args.
 
-Definition mkClass
-   : Name.Name ->
-     list TyVar ->
-     list (FunDep TyVar) ->
-     list PredType ->
-     list Id ->
-     list ClassATItem -> list ClassOpItem -> ClassMinimalDef -> TyCon -> Class :=
-  fun cls_name
-  tyvars
-  fds
-  super_classes
-  superdict_sels
-  at_stuff
-  op_stuff
-  mindef
-  tycon =>
-    Mk_Class tycon cls_name (Name.nameUnique cls_name) tyvars fds (ConcreteClass
-              super_classes superdict_sels at_stuff op_stuff mindef).
-
 Definition mkCharLit {b} : GHC.Char.Char -> Expr b :=
   fun c => Lit (mkMachChar c).
-
-Definition mkCallDmd : CleanDemand -> CleanDemand :=
-  fun '(JD d u) => JD (mkSCall d) (mkUCall One u).
-
-Definition mkBothDmdArg : DmdEnv -> BothDmdArg :=
-  fun env => pair env (Dunno tt).
 
 Definition mkApps {b} : Expr b -> list (Arg b) -> Expr b :=
   fun f args => Data.Foldable.foldl App f args.
 
-Definition mkAnonTyConBinder : TyVar -> TyConBinder :=
-  fun tv => TvBndr tv AnonTCB.
-
-Definition mkAnonTyConBinders : list TyVar -> list TyConBinder :=
-  fun tvs => GHC.Base.map mkAnonTyConBinder tvs.
-
-Definition mkAbstractClass
-   : Name.Name -> list TyVar -> list (FunDep TyVar) -> TyCon -> Class :=
-  fun cls_name tyvars fds tycon =>
-    Mk_Class tycon cls_name (Name.nameUnique cls_name) tyvars fds AbstractClass.
+Definition mkConApp {b} : DataCon -> list (Arg b) -> Expr b :=
+  fun con args => mkApps (Mk_Var (dataConWorkId con)) args.
 
 Definition minusVarSet : VarSet -> VarSet -> VarSet :=
   UniqSet.minusUniqSet.
@@ -5078,111 +4962,17 @@ Definition minusDVarSet : DVarSet -> DVarSet -> DVarSet :=
 Definition minusDVarEnv {a} {a'} : DVarEnv a -> DVarEnv a' -> DVarEnv a :=
   UniqDFM.minusUDFM.
 
-Definition mightBeUnsaturatedTyCon : TyCon -> bool :=
-  tcFlavourCanBeUnsaturated GHC.Base.∘ tyConFlavour.
-
 Definition maybeUnfoldingTemplate : Unfolding -> option CoreExpr :=
   fun arg_0__ => None.
 
 Definition mayHaveCafRefs : CafInfo -> bool :=
   fun arg_0__ => match arg_0__ with | MayHaveCafRefs => true | _ => false end.
 
-Definition markReused : UseDmd -> UseDmd :=
-  fix markReused (arg_0__ : UseDmd) : UseDmd
-        := let markReusedDmd (arg_0__ : ArgUse) : ArgUse :=
-             match arg_0__ with
-             | Abs => Abs
-             | Mk_Use _ a => Mk_Use Many (markReused a)
-             end in
-           match arg_0__ with
-           | UCall _ u => UCall Many u
-           | UProd ux => UProd (GHC.Base.map markReusedDmd ux)
-           | u => u
-           end.
-
-Definition markReusedDmd : ArgUse -> ArgUse :=
-  fun arg_0__ =>
-    match arg_0__ with
-    | Abs => Abs
-    | Mk_Use _ a => Mk_Use Many (markReused a)
-    end.
-
-Definition markExnStr : ArgStr -> ArgStr :=
-  fun arg_0__ =>
-    match arg_0__ with
-    | Mk_Str VanStr s => Mk_Str Mk_ExnStr s
-    | s => s
-    end.
-
-Definition postProcessDmd : DmdShell -> Demand -> Demand :=
-  fun arg_0__ arg_1__ =>
-    match arg_0__, arg_1__ with
-    | JD ss us, JD s a =>
-        let a' :=
-          match us with
-          | Abs => Abs
-          | Mk_Use Many _ => markReusedDmd a
-          | Mk_Use One _ => a
-          end in
-        let s' :=
-          match ss with
-          | Lazy => Lazy
-          | Mk_Str Mk_ExnStr _ => markExnStr s
-          | Mk_Str VanStr _ => s
-          end in
-        JD s' a'
-    end.
-
 Definition mapVarEnv {a} {b} : (a -> b) -> VarEnv a -> VarEnv b :=
   UniqFM.mapUFM.
 
-Definition reuseEnv : DmdEnv -> DmdEnv :=
-  mapVarEnv (postProcessDmd (JD (Mk_Str VanStr tt) (Mk_Use Many tt))).
-
 Definition mapDVarEnv {a} {b} : (a -> b) -> DVarEnv a -> DVarEnv b :=
   UniqDFM.mapUDFM.
-
-Axiom lubUse : UseDmd -> UseDmd -> UseDmd.
-
-Definition lubExnStr : ExnStr -> ExnStr -> ExnStr :=
-  fun arg_0__ arg_1__ =>
-    match arg_0__, arg_1__ with
-    | VanStr, VanStr => VanStr
-    | _, _ => Mk_ExnStr
-    end.
-
-Definition lubCount : Count -> Count -> Count :=
-  fun arg_0__ arg_1__ =>
-    match arg_0__, arg_1__ with
-    | _, Many => Many
-    | Many, _ => Many
-    | x, _ => x
-    end.
-
-Definition lubCPR : CPRResult -> CPRResult -> CPRResult :=
-  fun arg_0__ arg_1__ =>
-    let j_2__ :=
-      match arg_0__, arg_1__ with
-      | RetProd, RetProd => RetProd
-      | _, _ => NoCPR
-      end in
-    match arg_0__, arg_1__ with
-    | RetSum t1, RetSum t2 => if t1 GHC.Base.== t2 : bool then RetSum t1 else j_2__
-    | _, _ => j_2__
-    end.
-
-Definition lubDmdResult : DmdResult -> DmdResult -> DmdResult :=
-  fun arg_0__ arg_1__ =>
-    match arg_0__, arg_1__ with
-    | Diverges, r => r
-    | ThrowsExn, Diverges => ThrowsExn
-    | ThrowsExn, r => r
-    | Dunno c1, Diverges => Dunno c1
-    | Dunno c1, ThrowsExn => Dunno c1
-    | Dunno c1, Dunno c2 => Dunno (lubCPR c1 c2)
-    end.
-
-Axiom lubArgUse : ArgUse -> ArgUse -> ArgUse.
 
 Definition lookupDVarEnv {a} : DVarEnv a -> Var -> option a :=
   UniqDFM.lookupUDFM.
@@ -5257,197 +5047,11 @@ Definition lazySetIdInfo : Id -> IdInfo -> Var :=
        id_info_5__ := id in
     Mk_Id varName_0__ realUnique_1__ varType_2__ idScope_3__ id_details_4__ info.
 
-Definition lazyApply2Dmd : Demand :=
-  JD Lazy (Mk_Use One (UCall One (UCall One Used))).
-
-Definition lazyApply1Dmd : Demand :=
-  JD Lazy (Mk_Use One (UCall One Used)).
-
-Axiom kindTyConKeys : UniqSet.UniqSet Unique.Unique.
-
-Definition kill_usage : KillFlags -> Demand -> Demand :=
-  fun arg_0__ arg_1__ =>
-    match arg_0__, arg_1__ with
-    | kfs, JD s u => JD s (zap_musg kfs u)
-    end.
-
-Definition zapUsageDemand : Demand -> Demand :=
-  kill_usage (Mk_KillFlags true true true).
-
-Definition zapUsageInfo : IdInfo -> option IdInfo :=
-  fun info =>
-    Some (let 'Mk_IdInfo arityInfo_0__ ruleInfo_1__ unfoldingInfo_2__ cafInfo_3__
-             oneShotInfo_4__ inlinePragInfo_5__ occInfo_6__ strictnessInfo_7__ demandInfo_8__
-             callArityInfo_9__ levityInfo_10__ := info in
-          Mk_IdInfo arityInfo_0__ ruleInfo_1__ unfoldingInfo_2__ cafInfo_3__
-                    oneShotInfo_4__ inlinePragInfo_5__ occInfo_6__ strictnessInfo_7__
-                    (zapUsageDemand (demandInfo info)) callArityInfo_9__ levityInfo_10__).
-
-Definition zapUsedOnceDemand : Demand -> Demand :=
-  kill_usage (Mk_KillFlags false true false).
-
-Definition zapUsedOnceSig : StrictSig -> StrictSig :=
-  fun '(Mk_StrictSig (Mk_DmdType env ds r)) =>
-    Mk_StrictSig (Mk_DmdType env (GHC.Base.map zapUsedOnceDemand ds) r).
-
-Definition zapUsedOnceInfo : IdInfo -> option IdInfo :=
-  fun info =>
-    Some (let 'Mk_IdInfo arityInfo_0__ ruleInfo_1__ unfoldingInfo_2__ cafInfo_3__
-             oneShotInfo_4__ inlinePragInfo_5__ occInfo_6__ strictnessInfo_7__ demandInfo_8__
-             callArityInfo_9__ levityInfo_10__ := info in
-          Mk_IdInfo arityInfo_0__ ruleInfo_1__ unfoldingInfo_2__ cafInfo_3__
-                    oneShotInfo_4__ inlinePragInfo_5__ occInfo_6__ (zapUsedOnceSig (strictnessInfo
-                                                                                    info)) (zapUsedOnceDemand
-                     (demandInfo info)) callArityInfo_9__ levityInfo_10__).
-
-Definition killFlags : DynFlags.DynFlags -> option KillFlags :=
-  fun dflags =>
-    let kf_used_once := DynFlags.gopt DynFlags.Opt_KillOneShot dflags in
-    let kf_called_once := kf_used_once in
-    let kf_abs := DynFlags.gopt DynFlags.Opt_KillAbsence dflags in
-    if andb (negb kf_abs) (negb kf_used_once) : bool then None else
-    Some (Mk_KillFlags kf_abs kf_used_once kf_called_once).
-
-Definition killUsageDemand : DynFlags.DynFlags -> Demand -> Demand :=
-  fun dflags dmd =>
-    match killFlags dflags with
-    | Some kfs => kill_usage kfs dmd
-    | _ => dmd
-    end.
-
-Definition killUsageSig : DynFlags.DynFlags -> StrictSig -> StrictSig :=
-  fun arg_0__ arg_1__ =>
-    match arg_0__, arg_1__ with
-    | dflags, (Mk_StrictSig (Mk_DmdType env ds r) as sig) =>
-        match killFlags dflags with
-        | Some kfs => Mk_StrictSig (Mk_DmdType env (GHC.Base.map (kill_usage kfs) ds) r)
-        | _ => sig
-        end
-    end.
-
-Definition isVoidRep : PrimRep -> bool :=
-  fun arg_0__ => match arg_0__ with | VoidRep => true | _other => false end.
-
 Definition isVisibleArgFlag : ArgFlag -> bool :=
   fun arg_0__ => match arg_0__ with | Required => true | _ => false end.
 
-Definition isVisibleTcbVis : TyConBndrVis -> bool :=
-  fun arg_0__ =>
-    match arg_0__ with
-    | NamedTCB vis => isVisibleArgFlag vis
-    | AnonTCB => true
-    end.
-
-Definition isVisibleTyConBinder {tv} : TyVarBndr tv TyConBndrVis -> bool :=
-  fun '(TvBndr _ tcb_vis) => isVisibleTcbVis tcb_vis.
-
-Definition tyConVisibleTyVars : TyCon -> list TyVar :=
-  fun tc =>
-    let cont_0__ arg_1__ :=
-      let 'TvBndr tv vis := arg_1__ in
-      if isVisibleTcbVis vis : bool then cons tv nil else
-      nil in
-    Coq.Lists.List.flat_map cont_0__ (tyConBinders tc).
-
-Definition isVanillaDataCon : DataCon -> bool :=
-  fun dc => dcVanilla dc.
-
-Definition isVanillaAlgTyCon : TyCon -> bool :=
-  fun arg_0__ =>
-    match arg_0__ with
-    | AlgTyCon _ _ _ _ _ _ _ _ _ _ _ _ _ (VanillaAlgTyCon _) => true
-    | _ => false
-    end.
-
 Definition isValueUnfolding : Unfolding -> bool :=
   fun arg_0__ => false.
-
-Definition isUsedU : UseDmd -> bool :=
-  fix isUsedU (arg_0__ : UseDmd) : bool
-        := let isUsedMU (arg_0__ : ArgUse) : bool :=
-             match arg_0__ with
-             | Abs => true
-             | Mk_Use One _ => false
-             | Mk_Use Many u => isUsedU u
-             end in
-           match arg_0__ with
-           | Used => true
-           | UHead => true
-           | UProd us => Data.Foldable.all isUsedMU us
-           | UCall One _ => false
-           | UCall Many _ => true
-           end.
-
-Definition isUsedOnce : Demand -> bool :=
-  fun '(JD _ a) => match useCount a with | One => true | Many => false end.
-
-Definition isUsedMU : ArgUse -> bool :=
-  fun arg_0__ =>
-    match arg_0__ with
-    | Abs => true
-    | Mk_Use One _ => false
-    | Mk_Use Many u => isUsedU u
-    end.
-
-Definition isUnliftedTyCon : TyCon -> bool :=
-  fun arg_0__ =>
-    let j_2__ :=
-      match arg_0__ with
-      | AlgTyCon _ _ _ _ _ _ _ _ _ _ _ rhs _ _ =>
-          match rhs with
-          | SumTyCon _ => true
-          | _ => false
-          end
-      | _ => false
-      end in
-    match arg_0__ with
-    | PrimTyCon _ _ _ _ _ _ _ is_unlifted _ => is_unlifted
-    | AlgTyCon _ _ _ _ _ _ _ _ _ _ _ rhs _ _ =>
-        match rhs with
-        | TupleTyCon _ sort =>
-            negb (BasicTypes.isBoxed (BasicTypes.tupleSortBoxity sort))
-        | _ => j_2__
-        end
-    | _ => j_2__
-    end.
-
-Definition isUnboxedTupleTyCon : TyCon -> bool :=
-  fun arg_0__ =>
-    match arg_0__ with
-    | AlgTyCon _ _ _ _ _ _ _ _ _ _ _ rhs _ _ =>
-        match rhs with
-        | TupleTyCon _ sort =>
-            negb (BasicTypes.isBoxed (BasicTypes.tupleSortBoxity sort))
-        | _ => false
-        end
-    | _ => false
-    end.
-
-Definition isUnboxedTupleCon : DataCon -> bool :=
-  fun '(MkData _ _ _ _ _ _ _ _ _ _ _ _ _ _ _ _ _ _ tc _ _ _) =>
-    isUnboxedTupleTyCon tc.
-
-Definition isUnboxedSumTyCon : TyCon -> bool :=
-  fun arg_0__ =>
-    match arg_0__ with
-    | AlgTyCon _ _ _ _ _ _ _ _ _ _ _ rhs _ _ =>
-        match rhs with
-        | SumTyCon _ => true
-        | _ => false
-        end
-    | _ => false
-    end.
-
-Definition isUnboxedSumCon : DataCon -> bool :=
-  fun '(MkData _ _ _ _ _ _ _ _ _ _ _ _ _ _ _ _ _ _ tc _ _ _) =>
-    isUnboxedSumTyCon tc.
-
-Definition isTypeSynonymTyCon : TyCon -> bool :=
-  fun arg_0__ =>
-    match arg_0__ with
-    | SynonymTyCon _ _ _ _ _ _ _ _ _ _ _ => true
-    | _ => false
-    end.
 
 Definition isTypeArg {b} : Expr b -> bool :=
   fun arg_0__ => match arg_0__ with | Mk_Type _ => true | _ => false end.
@@ -5461,9 +5065,6 @@ Definition valArgCount {b} : list (Arg b) -> nat :=
 Definition isTyVar : Var -> bool :=
   fun arg_0__ => false.
 
-Definition isTyConAssoc : TyCon -> bool :=
-  fun tc => Data.Maybe.isJust (tyConAssoc_maybe tc).
-
 Definition isTyCoArg {b} : Expr b -> bool :=
   fun arg_0__ =>
     match arg_0__ with
@@ -5472,113 +5073,8 @@ Definition isTyCoArg {b} : Expr b -> bool :=
     | _ => false
     end.
 
-Definition isTupleTyCon : TyCon -> bool :=
-  fun arg_0__ =>
-    match arg_0__ with
-    | AlgTyCon _ _ _ _ _ _ _ _ _ _ _ (TupleTyCon _ _) _ _ => true
-    | _ => false
-    end.
-
-Definition isTupleDataCon : DataCon -> bool :=
-  fun '(MkData _ _ _ _ _ _ _ _ _ _ _ _ _ _ _ _ _ _ tc _ _ _) => isTupleTyCon tc.
-
-Definition isTopRes : DmdResult -> bool :=
-  fun arg_0__ => match arg_0__ with | Dunno NoCPR => true | _ => false end.
-
-Definition isTopDmd : Demand -> bool :=
-  fun arg_0__ =>
-    match arg_0__ with
-    | JD Lazy (Mk_Use Many Used) => true
-    | _ => false
-    end.
-
 Definition isTcTyVar : Var -> bool :=
   fun arg_0__ => false.
-
-Definition isTcTyCon : TyCon -> bool :=
-  fun arg_0__ =>
-    match arg_0__ with
-    | TcTyCon _ _ _ _ _ _ _ _ _ => true
-    | _ => false
-    end.
-
-Definition isTcLevPoly : TyCon -> bool :=
-  fun arg_0__ =>
-    match arg_0__ with
-    | FunTyCon _ _ _ _ _ _ _ => false
-    | AlgTyCon _ _ _ _ _ _ _ _ _ _ _ _ _ (UnboxedAlgTyCon _) => true
-    | AlgTyCon _ _ _ _ _ _ _ _ _ _ _ _ _ _ => false
-    | SynonymTyCon _ _ _ _ _ _ _ _ _ _ _ => true
-    | FamilyTyCon _ _ _ _ _ _ _ _ _ _ _ => true
-    | PrimTyCon _ _ _ _ _ _ _ _ _ => false
-    | TcTyCon _ _ _ _ _ _ _ _ _ => false
-    | (PromotedDataCon _ _ _ _ _ _ _ _ _ _ as tc) =>
-        Panic.panicStr (GHC.Base.hs_string__ "isTcLevPoly datacon") (Panic.someSDoc)
-    end.
-
-Definition isTauTyCon : TyCon -> bool :=
-  fun arg_0__ =>
-    match arg_0__ with
-    | SynonymTyCon _ _ _ _ _ _ _ _ _ is_tau _ => is_tau
-    | _ => true
-    end.
-
-Definition isStrictDmd : Demand -> bool :=
-  fun arg_0__ =>
-    match arg_0__ with
-    | JD _ Abs => false
-    | JD Lazy _ => false
-    | _ => true
-    end.
-
-Definition zapLamInfo : IdInfo -> option IdInfo :=
-  fun '((Mk_IdInfo _ _ _ _ _ _ occ _ demand _ _ as info)) =>
-    let is_safe_dmd := fun dmd => negb (isStrictDmd dmd) in
-    let safe_occ :=
-      match occ with
-      | BasicTypes.OneOcc _ _ _ _ =>
-          match occ with
-          | BasicTypes.ManyOccs _ =>
-              GHC.Err.error (GHC.Base.hs_string__ "Partial record update")
-          | BasicTypes.IAmDead =>
-              GHC.Err.error (GHC.Base.hs_string__ "Partial record update")
-          | BasicTypes.OneOcc occ_in_lam_2__ occ_one_br_3__ occ_int_cxt_4__
-          occ_tail_5__ =>
-              BasicTypes.OneOcc true occ_one_br_3__ occ_int_cxt_4__ BasicTypes.NoTailCallInfo
-          | BasicTypes.IAmALoopBreaker _ _ =>
-              GHC.Err.error (GHC.Base.hs_string__ "Partial record update")
-          end
-      | BasicTypes.IAmALoopBreaker _ _ =>
-          match occ with
-          | BasicTypes.ManyOccs occ_tail_12__ =>
-              BasicTypes.ManyOccs BasicTypes.NoTailCallInfo
-          | BasicTypes.IAmDead =>
-              GHC.Err.error (GHC.Base.hs_string__ "Partial record update")
-          | BasicTypes.OneOcc occ_in_lam_13__ occ_one_br_14__ occ_int_cxt_15__
-          occ_tail_16__ =>
-              BasicTypes.OneOcc occ_in_lam_13__ occ_one_br_14__ occ_int_cxt_15__
-                                BasicTypes.NoTailCallInfo
-          | BasicTypes.IAmALoopBreaker occ_rules_only_17__ occ_tail_18__ =>
-              BasicTypes.IAmALoopBreaker occ_rules_only_17__ BasicTypes.NoTailCallInfo
-          end
-      | _other => occ
-      end in
-    let is_safe_occ :=
-      fun arg_27__ =>
-        let 'occ := arg_27__ in
-        if BasicTypes.isAlwaysTailCalled occ : bool then false else
-        match arg_27__ with
-        | BasicTypes.OneOcc in_lam _ _ _ => in_lam
-        | _other => true
-        end in
-    if andb (is_safe_occ occ) (is_safe_dmd demand) : bool then None else
-    Some (let 'Mk_IdInfo arityInfo_31__ ruleInfo_32__ unfoldingInfo_33__
-             cafInfo_34__ oneShotInfo_35__ inlinePragInfo_36__ occInfo_37__
-             strictnessInfo_38__ demandInfo_39__ callArityInfo_40__ levityInfo_41__ :=
-            info in
-          Mk_IdInfo arityInfo_31__ ruleInfo_32__ unfoldingInfo_33__ cafInfo_34__
-                    oneShotInfo_35__ inlinePragInfo_36__ safe_occ strictnessInfo_38__ topDmd
-                    callArityInfo_40__ levityInfo_41__).
 
 Definition isStableUnfolding : Unfolding -> bool :=
   fun arg_0__ => false.
@@ -5591,92 +5087,11 @@ Definition isStableSource : UnfoldingSource -> bool :=
     | InlineRhs => false
     end.
 
-Definition isSrcUnpacked : SrcUnpackedness -> bool :=
-  fun arg_0__ => match arg_0__ with | SrcUnpack => true | _ => false end.
-
-Definition isSrcStrict : SrcStrictness -> bool :=
-  fun arg_0__ => match arg_0__ with | SrcStrict => true | _ => false end.
-
-Definition isSeqDmd : Demand -> bool :=
-  fun arg_0__ =>
-    match arg_0__ with
-    | JD (Mk_Str VanStr HeadStr) (Mk_Use _ UHead) => true
-    | _ => false
-    end.
-
 Definition isRuntimeArg : CoreExpr -> bool :=
   isValArg.
 
-Axiom isPromotedTupleTyCon : TyCon -> bool.
-
-Definition isPromotedDataCon_maybe : TyCon -> option DataCon :=
-  fun arg_0__ =>
-    match arg_0__ with
-    | PromotedDataCon _ _ _ _ _ _ _ dc _ _ => Some dc
-    | _ => None
-    end.
-
-Definition isPromotedDataCon : TyCon -> bool :=
-  fun arg_0__ =>
-    match arg_0__ with
-    | PromotedDataCon _ _ _ _ _ _ _ _ _ _ => true
-    | _ => false
-    end.
-
-Axiom isProductTyCon : TyCon -> bool.
-
-Definition isPrimTyCon : TyCon -> bool :=
-  fun arg_0__ =>
-    match arg_0__ with
-    | PrimTyCon _ _ _ _ _ _ _ _ _ => true
-    | _ => false
-    end.
-
 Definition isOrphan : IsOrphan -> bool :=
   fun arg_0__ => match arg_0__ with | Mk_IsOrphan => true | _ => false end.
-
-Definition isOpenTypeFamilyTyCon : TyCon -> bool :=
-  fun arg_0__ =>
-    match arg_0__ with
-    | FamilyTyCon _ _ _ _ _ _ _ _ OpenSynFamilyTyCon _ _ => true
-    | _ => false
-    end.
-
-Definition isOpenFamilyTyCon : TyCon -> bool :=
-  fun arg_0__ =>
-    match arg_0__ with
-    | FamilyTyCon _ _ _ _ _ _ _ _ flav _ _ =>
-        match flav with
-        | OpenSynFamilyTyCon => true
-        | _ => match flav with | DataFamilyTyCon _ => true | _ => false end
-        end
-    | _ => false
-    end.
-
-Definition isNoParent : AlgTyConFlav -> bool :=
-  fun arg_0__ => match arg_0__ with | VanillaAlgTyCon _ => true | _ => false end.
-
-Definition isTyConWithSrcDataCons : TyCon -> bool :=
-  fun arg_0__ =>
-    match arg_0__ with
-    | AlgTyCon _ _ _ _ _ _ _ _ _ _ _ rhs _ parent =>
-        let isSrcParent := isNoParent parent in
-        match rhs with
-        | DataTyCon _ _ => isSrcParent
-        | NewTyCon _ _ _ _ => isSrcParent
-        | TupleTyCon _ _ => isSrcParent
-        | _ => false
-        end
-    | FamilyTyCon _ _ _ _ _ _ _ _ (DataFamilyTyCon _) _ _ => true
-    | _ => false
-    end.
-
-Definition isNewTyCon : TyCon -> bool :=
-  fun arg_0__ =>
-    match arg_0__ with
-    | AlgTyCon _ _ _ _ _ _ _ _ _ _ _ (NewTyCon _ _ _ _) _ _ => true
-    | _ => false
-    end.
 
 Definition isNeverLevPolyIdInfo : IdInfo -> bool :=
   fun info =>
@@ -5684,16 +5099,6 @@ Definition isNeverLevPolyIdInfo : IdInfo -> bool :=
     | NeverLevityPolymorphic => true
     | _ => false
     end.
-
-Definition isNamedTyConBinder : TyConBinder -> bool :=
-  fun arg_0__ =>
-    match arg_0__ with
-    | TvBndr _ (NamedTCB _) => true
-    | _ => false
-    end.
-
-Definition isMarkedStrict : StrictnessMark -> bool :=
-  fun arg_0__ => match arg_0__ with | NotMarkedStrict => false | _ => true end.
 
 Definition isLocalRule : CoreRule -> bool :=
   ru_local.
@@ -5715,14 +5120,6 @@ Definition setIdNotExported : Id -> Id :=
          Mk_Id varName_0__ realUnique_1__ varType_2__ (LocalId NotExported)
                id_details_4__ id_info_5__.
 
-Definition isLazy : ArgStr -> bool :=
-  fun arg_0__ => match arg_0__ with | Lazy => true | Mk_Str _ _ => false end.
-
-Definition isWeakDmd : Demand -> bool :=
-  fun '(JD s a) => andb (isLazy s) (isUsedMU a).
-
-Axiom isKindTyCon : TyCon -> bool.
-
 Definition isJoinIdDetails_maybe : IdDetails -> option BasicTypes.JoinArity :=
   fun arg_0__ =>
     match arg_0__ with
@@ -5730,29 +5127,8 @@ Definition isJoinIdDetails_maybe : IdDetails -> option BasicTypes.JoinArity :=
     | _ => None
     end.
 
-Definition isInvisibleTyConBinder {tv} : TyVarBndr tv TyConBndrVis -> bool :=
-  fun tcb => negb (isVisibleTyConBinder tcb).
-
 Definition isInvisibleArgFlag : ArgFlag -> bool :=
   negb GHC.Base.∘ isVisibleArgFlag.
-
-Axiom isInjectiveTyCon : TyCon -> Role -> bool.
-
-Definition isImplicitTyCon : TyCon -> bool :=
-  fun arg_0__ =>
-    match arg_0__ with
-    | FunTyCon _ _ _ _ _ _ _ => true
-    | PrimTyCon _ _ _ _ _ _ _ _ _ => true
-    | PromotedDataCon _ _ _ _ _ _ _ _ _ _ => true
-    | AlgTyCon _ name _ _ _ _ _ _ _ _ _ rhs _ _ =>
-        match rhs with
-        | TupleTyCon _ _ => Name.isWiredInName name
-        | _ => match rhs with | SumTyCon _ => true | _ => false end
-        end
-    | FamilyTyCon _ _ _ _ _ _ _ _ _ parent _ => Data.Maybe.isJust parent
-    | SynonymTyCon _ _ _ _ _ _ _ _ _ _ _ => false
-    | TcTyCon _ _ _ _ _ _ _ _ _ => false
-    end.
 
 Definition isId : Var -> bool :=
   fun '(Mk_Id _ _ _ _ _ _) => true.
@@ -5762,53 +5138,6 @@ Definition isRuntimeVar : Var -> bool :=
 
 Definition valBndrCount : list CoreBndr -> nat :=
   Util.count isId.
-
-Definition isHyperStr : ArgStr -> bool :=
-  fun arg_0__ => match arg_0__ with | Mk_Str _ HyperStr => true | _ => false end.
-
-Definition mkSProd : list ArgStr -> StrDmd :=
-  fun sx =>
-    if Data.Foldable.any isHyperStr sx : bool then HyperStr else
-    if Data.Foldable.all isLazy sx : bool then HeadStr else
-    SProd sx.
-
-Definition lubStr : StrDmd -> StrDmd -> StrDmd :=
-  fix lubStr (arg_0__ arg_1__ : StrDmd) : StrDmd
-        := let lubArgStr (arg_0__ arg_1__ : ArgStr) : ArgStr :=
-             match arg_0__, arg_1__ with
-             | Lazy, _ => Lazy
-             | _, Lazy => Lazy
-             | Mk_Str x1 s1, Mk_Str x2 s2 => Mk_Str (lubExnStr x1 x2) (lubStr s1 s2)
-             end in
-           match arg_0__, arg_1__ with
-           | HyperStr, s => s
-           | SCall s1, HyperStr => SCall s1
-           | SCall _, HeadStr => HeadStr
-           | SCall s1, SCall s2 => SCall (lubStr s1 s2)
-           | SCall _, SProd _ => HeadStr
-           | SProd sx, HyperStr => SProd sx
-           | SProd _, HeadStr => HeadStr
-           | SProd s1, SProd s2 =>
-               if Util.equalLength s1 s2 : bool
-               then mkSProd (GHC.List.zipWith lubArgStr s1 s2) else
-               HeadStr
-           | SProd _, SCall _ => HeadStr
-           | HeadStr, _ => HeadStr
-           end.
-
-Definition lubArgStr : ArgStr -> ArgStr -> ArgStr :=
-  fun arg_0__ arg_1__ =>
-    match arg_0__, arg_1__ with
-    | Lazy, _ => Lazy
-    | _, Lazy => Lazy
-    | Mk_Str x1 s1, Mk_Str x2 s2 => Mk_Str (lubExnStr x1 x2) (lubStr s1 s2)
-    end.
-
-Definition lubDmd : Demand -> Demand -> Demand :=
-  fun arg_0__ arg_1__ =>
-    match arg_0__, arg_1__ with
-    | JD s1 a1, JD s2 a2 => JD (lubArgStr s1 s2) (lubArgUse a1 a2)
-    end.
 
 Definition isGlobalId : Var -> bool :=
   fun arg_0__ =>
@@ -5823,59 +5152,11 @@ Definition isLocalVar : Var -> bool :=
 Definition mustHaveLocalBinding : Var -> bool :=
   fun var => isLocalVar var.
 
-Axiom isGenerativeTyCon : TyCon -> Role -> bool.
-
-Definition isGenInjAlgRhs : AlgTyConRhs -> bool :=
-  fun arg_0__ =>
-    match arg_0__ with
-    | TupleTyCon _ _ => true
-    | SumTyCon _ => true
-    | DataTyCon _ _ => true
-    | AbstractTyCon => false
-    | NewTyCon _ _ _ _ => false
-    end.
-
-Definition isGcPtrRep : PrimRep -> bool :=
-  fun arg_0__ =>
-    match arg_0__ with
-    | LiftedRep => true
-    | UnliftedRep => true
-    | _ => false
-    end.
-
-Definition isGadtSyntaxTyCon : TyCon -> bool :=
-  fun arg_0__ =>
-    match arg_0__ with
-    | AlgTyCon _ _ _ _ _ _ _ _ _ res _ _ _ _ => res
-    | _ => false
-    end.
-
-Definition isFunTyCon : TyCon -> bool :=
-  fun arg_0__ =>
-    match arg_0__ with
-    | FunTyCon _ _ _ _ _ _ _ => true
-    | _ => false
-    end.
-
 Definition isFragileUnfolding : Unfolding -> bool :=
   fun arg_0__ => false.
 
 Definition zapFragileUnfolding : Unfolding -> Unfolding :=
   fun unf => if isFragileUnfolding unf : bool then noUnfolding else unf.
-
-Definition isFamilyTyCon : TyCon -> bool :=
-  fun arg_0__ =>
-    match arg_0__ with
-    | FamilyTyCon _ _ _ _ _ _ _ _ _ _ _ => true
-    | _ => false
-    end.
-
-Definition isFamInstTyCon : TyCon -> bool :=
-  fun arg_0__ =>
-    match arg_0__ with
-    | AlgTyCon _ _ _ _ _ _ _ _ _ _ _ _ _ (DataFamInstTyCon _ _ _) => true
-    | _ => false
-    end.
 
 Definition isExportedId : Var -> bool :=
   fun arg_0__ =>
@@ -5890,18 +5171,6 @@ Definition isExpandableUnfolding : Unfolding -> bool :=
 
 Definition isEvaldUnfolding : Unfolding -> bool :=
   fun arg_0__ => false.
-
-Definition isEnumerationTyCon : TyCon -> bool :=
-  fun arg_0__ =>
-    match arg_0__ with
-    | AlgTyCon _ _ _ _ _ _ arity _ _ _ _ rhs _ _ =>
-        match rhs with
-        | DataTyCon _ res => res
-        | TupleTyCon _ _ => arity GHC.Base.== #0
-        | _ => false
-        end
-    | _ => false
-    end.
 
 Definition isEmptyVarSet : VarSet -> bool :=
   UniqSet.isEmptyUniqSet.
@@ -5927,18 +5196,6 @@ Definition transCloVarSet : (VarSet -> VarSet) -> VarSet -> VarSet :=
 Definition isEmptyVarEnv {a} : VarEnv a -> bool :=
   UniqFM.isNullUFM.
 
-Definition isTopDmdType : DmdType -> bool :=
-  fun arg_0__ =>
-    match arg_0__ with
-    | Mk_DmdType env nil res =>
-        if andb (isTopRes res) (isEmptyVarEnv env) : bool then true else
-        false
-    | _ => false
-    end.
-
-Definition isTopSig : StrictSig -> bool :=
-  fun '(Mk_StrictSig ty) => isTopDmdType ty.
-
 Definition isEmptyRuleInfo : RuleInfo -> bool :=
   fun x => true.
 
@@ -5959,49 +5216,6 @@ Definition transCloDVarSet : (DVarSet -> DVarSet) -> DVarSet -> DVarSet :=
 
 Definition isEmptyDVarEnv {a} : DVarEnv a -> bool :=
   UniqDFM.isNullUDFM.
-
-Definition isDataTyCon : TyCon -> bool :=
-  fun arg_0__ =>
-    match arg_0__ with
-    | AlgTyCon _ _ _ _ _ _ _ _ _ _ _ rhs _ _ =>
-        match rhs with
-        | TupleTyCon _ sort => BasicTypes.isBoxed (BasicTypes.tupleSortBoxity sort)
-        | SumTyCon _ => false
-        | DataTyCon _ _ => true
-        | NewTyCon _ _ _ _ => false
-        | AbstractTyCon => false
-        end
-    | _ => false
-    end.
-
-Axiom isDataSumTyCon_maybe : TyCon -> option (list DataCon).
-
-Axiom isDataProductTyCon_maybe : TyCon -> option DataCon.
-
-Definition isDataFamFlav : FamTyConFlav -> bool :=
-  fun arg_0__ => match arg_0__ with | DataFamilyTyCon _ => true | _ => false end.
-
-Definition isDataFamilyTyCon : TyCon -> bool :=
-  fun arg_0__ =>
-    match arg_0__ with
-    | FamilyTyCon _ _ _ _ _ _ _ _ flav _ _ => isDataFamFlav flav
-    | _ => false
-    end.
-
-Definition isFamFreeTyCon : TyCon -> bool :=
-  fun arg_0__ =>
-    match arg_0__ with
-    | SynonymTyCon _ _ _ _ _ _ _ _ _ _ fam_free => fam_free
-    | FamilyTyCon _ _ _ _ _ _ _ _ flav _ _ => isDataFamFlav flav
-    | _ => true
-    end.
-
-Definition isTypeFamilyTyCon : TyCon -> bool :=
-  fun arg_0__ =>
-    match arg_0__ with
-    | FamilyTyCon _ _ _ _ _ _ _ _ flav _ _ => negb (isDataFamFlav flav)
-    | _ => false
-    end.
 
 Definition isConLikeUnfolding : Unfolding -> bool :=
   fun arg_0__ => false.
@@ -6030,26 +5244,16 @@ Definition varToCoreExpr {b} : CoreBndr -> Expr b :=
           #1920)
     else Mk_Var v.
 
+Definition mkConApp2 {b} : DataCon -> list Type_ -> list Var -> Expr b :=
+  fun con tys arg_ids =>
+    mkApps (mkApps (Mk_Var (dataConWorkId con)) (GHC.Base.map Mk_Type tys))
+           (GHC.Base.map varToCoreExpr arg_ids).
+
 Definition mkVarApps {b} : Expr b -> list Var -> Expr b :=
   fun f vars => Data.Foldable.foldl (fun e a => App e (varToCoreExpr a)) f vars.
 
 Definition varsToCoreExprs {b} : list CoreBndr -> list (Expr b) :=
   fun vs => GHC.Base.map varToCoreExpr vs.
-
-Definition isClosedSynFamilyTyConWithAxiom_maybe
-   : TyCon -> option (CoAxiom Branched) :=
-  fun arg_0__ =>
-    match arg_0__ with
-    | FamilyTyCon _ _ _ _ _ _ _ _ (ClosedSynFamilyTyCon mb) _ _ => mb
-    | _ => None
-    end.
-
-Definition isClassTyCon : TyCon -> bool :=
-  fun arg_0__ =>
-    match arg_0__ with
-    | AlgTyCon _ _ _ _ _ _ _ _ _ _ _ _ _ (ClassTyCon _ _) => true
-    | _ => false
-    end.
 
 Definition isCheapUnfolding : Unfolding -> bool :=
   fun arg_0__ => false.
@@ -6061,45 +5265,8 @@ Definition isBuiltinRule : CoreRule -> bool :=
     | _ => false
     end.
 
-Definition isBuiltInSynFamTyCon_maybe : TyCon -> option BuiltInSynFamily :=
-  fun arg_0__ =>
-    match arg_0__ with
-    | FamilyTyCon _ _ _ _ _ _ _ _ (BuiltInSynFamTyCon ops) _ _ => Some ops
-    | _ => None
-    end.
-
-Definition isBoxedTupleTyCon : TyCon -> bool :=
-  fun arg_0__ =>
-    match arg_0__ with
-    | AlgTyCon _ _ _ _ _ _ _ _ _ _ _ rhs _ _ =>
-        match rhs with
-        | TupleTyCon _ sort => BasicTypes.isBoxed (BasicTypes.tupleSortBoxity sort)
-        | _ => false
-        end
-    | _ => false
-    end.
-
-Definition isBotRes : DmdResult -> bool :=
-  fun arg_0__ =>
-    match arg_0__ with
-    | Diverges => true
-    | ThrowsExn => true
-    | Dunno _ => false
-    end.
-
-Definition isBottomingSig : StrictSig -> bool :=
-  fun '(Mk_StrictSig (Mk_DmdType _ _ res)) => isBotRes res.
-
 Definition isBootUnfolding : Unfolding -> bool :=
   fun arg_0__ => false.
-
-Definition isBanged : HsImplBang -> bool :=
-  fun arg_0__ =>
-    match arg_0__ with
-    | HsUnpack _ => true
-    | HsStrict => true
-    | HsLazy => false
-    end.
 
 Definition isAutoRule : CoreRule -> bool :=
   fun arg_0__ =>
@@ -6107,42 +5274,6 @@ Definition isAutoRule : CoreRule -> bool :=
     | BuiltinRule _ _ _ _ => false
     | Rule _ _ _ _ _ _ _ is_auto _ _ _ => is_auto
     end.
-
-Definition isAlgTyCon : TyCon -> bool :=
-  fun arg_0__ =>
-    match arg_0__ with
-    | AlgTyCon _ _ _ _ _ _ _ _ _ _ _ _ _ _ => true
-    | _ => false
-    end.
-
-Definition tyConFieldLabelEnv : TyCon -> FieldLabel.FieldLabelEnv :=
-  fun tc =>
-    if isAlgTyCon tc : bool then algTcFields tc else
-    FastStringEnv.emptyDFsEnv.
-
-Definition lookupTyConFieldLabel
-   : FieldLabel.FieldLabelString -> TyCon -> option FieldLabel.FieldLabel :=
-  fun lbl tc => FastStringEnv.lookupDFsEnv (tyConFieldLabelEnv tc) lbl.
-
-Definition tyConFieldLabels : TyCon -> list FieldLabel.FieldLabel :=
-  fun tc => FastStringEnv.dFsEnvElts (tyConFieldLabelEnv tc).
-
-Definition isAbstractTyCon : TyCon -> bool :=
-  fun arg_0__ =>
-    match arg_0__ with
-    | AlgTyCon _ _ _ _ _ _ _ _ _ _ _ AbstractTyCon _ _ => true
-    | _ => false
-    end.
-
-Definition isAbstractClass : Class -> bool :=
-  fun arg_0__ =>
-    match arg_0__ with
-    | Mk_Class _ _ _ _ _ AbstractClass => true
-    | _ => false
-    end.
-
-Definition isAbsDmd : Demand -> bool :=
-  fun arg_0__ => match arg_0__ with | JD _ Abs => true | _ => false end.
 
 Definition intersectsVarEnv {a} : VarEnv a -> VarEnv a -> bool :=
   fun e1 e2 => negb (isEmptyVarEnv (UniqFM.intersectUFM e1 e2)).
@@ -6153,17 +5284,6 @@ Definition intersectVarSet : VarSet -> VarSet -> VarSet :=
 Definition intersectDVarSet : DVarSet -> DVarSet -> DVarSet :=
   UniqDSet.intersectUniqDSets.
 
-Definition initRecTc : RecTcChecker :=
-  RC #100 NameEnv.emptyNameEnv.
-
-Definition increaseStrictSigArity : nat -> StrictSig -> StrictSig :=
-  fun arg_0__ arg_1__ =>
-    match arg_0__, arg_1__ with
-    | arity_increase, Mk_StrictSig (Mk_DmdType env dmds res) =>
-        Mk_StrictSig (Mk_DmdType env (Coq.Init.Datatypes.app (Coq.Lists.List.repeat
-                                                              topDmd arity_increase) dmds) res)
-    end.
-
 Definition idInfo `{Util.HasDebugCallStack} : Id -> IdInfo :=
   fun '(Mk_Id _ _ _ _ _ info) => info.
 
@@ -6173,24 +5293,11 @@ Definition idDetails : Id -> IdDetails :=
 Definition hasSomeUnfolding : Unfolding -> bool :=
   fun '(NoUnfolding) => false.
 
-Definition hasDemandEnvSig : StrictSig -> bool :=
-  fun '(Mk_StrictSig (Mk_DmdType env _ _)) => negb (isEmptyVarEnv env).
-
 Definition globaliseId : Id -> Id :=
   fun '(Mk_Id varName_0__ realUnique_1__ varType_2__ idScope_3__ id_details_4__
   id_info_5__) =>
     Mk_Id varName_0__ realUnique_1__ varType_2__ GlobalId id_details_4__
           id_info_5__.
-
-Definition getUseDmd {s} {u} : JointDmd s u -> u :=
-  ud.
-
-Definition getStrDmd {s} {u} : JointDmd s u -> s :=
-  sd.
-
-Definition mkProdDmd : list Demand -> CleanDemand :=
-  fun dx =>
-    JD (mkSProd (GHC.Base.map getStrDmd dx)) (mkUProd (GHC.Base.map getUseDmd dx)).
 
 Definition getInScopeVars : InScopeSet -> VarSet :=
   fun '(InScope vs _) => vs.
@@ -6232,13 +5339,6 @@ Definition filterDVarSet : (Var -> bool) -> DVarSet -> DVarSet :=
 
 Definition filterDVarEnv {a} : (a -> bool) -> DVarEnv a -> DVarEnv a :=
   UniqDFM.filterUDFM.
-
-Definition famTyConFlav_maybe : TyCon -> option FamTyConFlav :=
-  fun arg_0__ =>
-    match arg_0__ with
-    | FamilyTyCon _ _ _ _ _ _ _ _ flav _ _ => Some flav
-    | _ => None
-    end.
 
 Definition extendDVarEnv {a} : DVarEnv a -> Var -> a -> DVarEnv a :=
   UniqDFM.addToUDFM.
@@ -6323,55 +5423,6 @@ Definition exprToCoercion_maybe : CoreExpr -> option Coercion :=
 Definition expandUnfolding_maybe : Unfolding -> option CoreExpr :=
   fun arg_0__ => None.
 
-Definition expandSynTyCon_maybe {tyco}
-   : TyCon ->
-     list tyco -> option (list (TyVar * tyco)%type * Type_ * list tyco)%type :=
-  fun tc tys =>
-    match tc with
-    | SynonymTyCon _ _ _ tvs _ _ arity _ rhs _ _ =>
-        match Util.listLengthCmp tys arity with
-        | Gt =>
-            Some (pair (pair (GHC.List.zip tvs tys) rhs) (Coq.Lists.List.skipn arity tys))
-        | Eq => Some (pair (pair (GHC.List.zip tvs tys) rhs) nil)
-        | Lt => None
-        end
-    | _ => None
-    end.
-
-Definition exnRes : DmdResult :=
-  ThrowsExn.
-
-Definition evalDmd : Demand :=
-  JD (Mk_Str VanStr HeadStr) useTop.
-
-Definition eqSpecType : EqSpec -> Type_ :=
-  fun '(Mk_EqSpec _ ty) => ty.
-
-Definition eqSpecTyVar : EqSpec -> TyVar :=
-  fun '(Mk_EqSpec tv _) => tv.
-
-Local Definition Eq___Var_op_zeze__ : Var -> Var -> bool :=
-  fun a b => realUnique a GHC.Base.== realUnique b.
-
-Local Definition Eq___Var_op_zsze__ : Var -> Var -> bool :=
-  fun x y => negb (Eq___Var_op_zeze__ x y).
-
-Program Instance Eq___Var : GHC.Base.Eq_ Var :=
-  fun _ k__ =>
-    k__ {| GHC.Base.op_zeze____ := Eq___Var_op_zeze__ ;
-           GHC.Base.op_zsze____ := Eq___Var_op_zsze__ |}.
-
-Definition filterEqSpec : list EqSpec -> list TyVar -> list TyVar :=
-  fun eq_spec =>
-    let not_in_eq_spec :=
-      fun var =>
-        Data.Foldable.all (negb GHC.Base.∘
-                           ((fun arg_0__ => arg_0__ GHC.Base.== var) GHC.Base.∘ eqSpecTyVar)) eq_spec in
-    GHC.List.filter not_in_eq_spec.
-
-Definition eqSpecPair : EqSpec -> (TyVar * Type_)%type :=
-  fun '(Mk_EqSpec tv ty) => pair tv ty.
-
 Definition emptyVarSet : VarSet :=
   UniqSet.emptyUniqSet.
 
@@ -6393,29 +5444,19 @@ Definition nukeRnEnvR : RnEnv2 -> RnEnv2 :=
   fun '(RV2 envL_0__ envR_1__ in_scope_2__) =>
     RV2 envL_0__ emptyVarEnv in_scope_2__.
 
-Definition splitFVs : bool -> DmdEnv -> (DmdEnv * DmdEnv)%type :=
-  fun is_thunk rhs_fvs =>
-    let add :=
-      fun arg_0__ arg_1__ arg_2__ =>
-        match arg_0__, arg_1__, arg_2__ with
-        | uniq, (JD s u as dmd), pair lazy_fv sig_fv =>
-            match s with
-            | Lazy => pair (UniqFM.addToUFM_Directly lazy_fv uniq dmd) sig_fv
-            | _ =>
-                pair (UniqFM.addToUFM_Directly lazy_fv uniq (JD Lazy u))
-                     (UniqFM.addToUFM_Directly sig_fv uniq (JD s Abs))
-            end
-        end in
-    if is_thunk : bool
-    then UniqFM.nonDetFoldUFM_Directly add (pair emptyVarEnv emptyVarEnv)
-         rhs_fvs else
-    partitionVarEnv isWeakDmd rhs_fvs.
-
 Definition emptyTidyEnv : TidyEnv :=
   pair OccName.emptyTidyOccEnv emptyVarEnv.
 
 Definition emptyRuleInfo :=
   EmptyRuleInfo.
+
+Definition vanillaIdInfo : IdInfo :=
+  Mk_IdInfo unknownArity emptyRuleInfo noUnfolding vanillaCafInfo
+            BasicTypes.NoOneShotInfo BasicTypes.defaultInlinePragma BasicTypes.noOccInfo
+            nopSig topDmd unknownArity NoLevityInfo.
+
+Definition noCafIdInfo : IdInfo :=
+  setCafInfo vanillaIdInfo NoCafRefs.
 
 Definition zapFragileInfo : IdInfo -> option IdInfo :=
   fun '((Mk_IdInfo _ _ unf _ _ _ occ _ _ _ _ as info)) =>
@@ -6429,83 +5470,6 @@ Definition emptyRuleEnv : RuleEnv :=
 
 Definition emptyInScopeSet : InScopeSet :=
   InScope emptyVarSet #1.
-
-Definition emptyDmdEnv : VarEnv Demand :=
-  emptyVarEnv.
-
-Definition exnDmdType : DmdType :=
-  Mk_DmdType emptyDmdEnv nil exnRes.
-
-Definition exnSig : StrictSig :=
-  Mk_StrictSig exnDmdType.
-
-Definition mkClosedStrictSig : list Demand -> DmdResult -> StrictSig :=
-  fun ds res => mkStrictSig (Mk_DmdType emptyDmdEnv ds res).
-
-Definition zapUsageEnvSig : StrictSig -> StrictSig :=
-  fun '(Mk_StrictSig (Mk_DmdType _ ds r)) => mkClosedStrictSig ds r.
-
-Definition zapUsageEnvInfo : IdInfo -> option IdInfo :=
-  fun info =>
-    if hasDemandEnvSig (strictnessInfo info) : bool
-    then Some (let 'Mk_IdInfo arityInfo_0__ ruleInfo_1__ unfoldingInfo_2__
-                  cafInfo_3__ oneShotInfo_4__ inlinePragInfo_5__ occInfo_6__ strictnessInfo_7__
-                  demandInfo_8__ callArityInfo_9__ levityInfo_10__ := info in
-               Mk_IdInfo arityInfo_0__ ruleInfo_1__ unfoldingInfo_2__ cafInfo_3__
-                         oneShotInfo_4__ inlinePragInfo_5__ occInfo_6__ (zapUsageEnvSig (strictnessInfo
-                                                                                         info)) demandInfo_8__
-                         callArityInfo_9__ levityInfo_10__) else
-    None.
-
-Definition nopDmdType : DmdType :=
-  Mk_DmdType emptyDmdEnv nil topRes.
-
-Definition nopSig : StrictSig :=
-  Mk_StrictSig nopDmdType.
-
-Definition vanillaIdInfo : IdInfo :=
-  Mk_IdInfo unknownArity emptyRuleInfo noUnfolding vanillaCafInfo
-            BasicTypes.NoOneShotInfo BasicTypes.defaultInlinePragma BasicTypes.noOccInfo
-            nopSig topDmd unknownArity NoLevityInfo.
-
-Definition noCafIdInfo : IdInfo :=
-  setCafInfo vanillaIdInfo NoCafRefs.
-
-Definition postProcessDmdEnv : DmdShell -> DmdEnv -> DmdEnv :=
-  fun arg_0__ arg_1__ =>
-    match arg_0__, arg_1__ with
-    | (JD ss us as ds), env =>
-        match us with
-        | Abs => emptyDmdEnv
-        | _ =>
-            let j_2__ := mapVarEnv (postProcessDmd ds) env in
-            match ss with
-            | Mk_Str VanStr _ => match us with | Mk_Use One _ => env | _ => j_2__ end
-            | _ => j_2__
-            end
-        end
-    end.
-
-Definition postProcessDmdType : DmdShell -> DmdType -> BothDmdArg :=
-  fun arg_0__ arg_1__ =>
-    match arg_0__, arg_1__ with
-    | (JD ss _ as du), Mk_DmdType fv _ res_ty =>
-        let term_info :=
-          match postProcessDmdResult ss res_ty with
-          | Dunno _ => Dunno tt
-          | ThrowsExn => ThrowsExn
-          | Diverges => Diverges
-          end in
-        pair (postProcessDmdEnv du fv) term_info
-    end.
-
-Definition postProcessUnsat : DmdShell -> DmdType -> DmdType :=
-  fun arg_0__ arg_1__ =>
-    match arg_0__, arg_1__ with
-    | (JD ss _ as ds), Mk_DmdType fv args res_ty =>
-        Mk_DmdType (postProcessDmdEnv ds fv) (GHC.Base.map (postProcessDmd ds) args)
-        (postProcessDmdResult ss res_ty)
-    end.
 
 Definition emptyDVarSet : DVarSet :=
   UniqDSet.emptyUniqDSet.
@@ -6687,73 +5651,6 @@ Definition rnEtaR : RnEnv2 -> Var -> (RnEnv2 * Var)%type :=
                   (extendInScopeSet in_scope new_b)) new_b
     end.
 
-Definition dmdTypeDepth : DmdType -> BasicTypes.Arity :=
-  fun '(Mk_DmdType _ ds _) => Coq.Lists.List.length ds.
-
-Definition dmdTransformSig : StrictSig -> CleanDemand -> DmdType :=
-  fun arg_0__ arg_1__ =>
-    match arg_0__, arg_1__ with
-    | Mk_StrictSig (Mk_DmdType _ arg_ds _ as dmd_ty), cd =>
-        postProcessUnsat (peelManyCalls (Coq.Lists.List.length arg_ds) cd) dmd_ty
-    end.
-
-Definition dmdTransformDictSelSig : StrictSig -> CleanDemand -> DmdType :=
-  fun arg_0__ arg_1__ =>
-    match arg_0__, arg_1__ with
-    | Mk_StrictSig (Mk_DmdType _ (cons dict_dmd nil) _), cd =>
-        let enhance :=
-          fun cd old => if isAbsDmd old : bool then old else mkOnceUsedDmd cd in
-        let 'pair cd' defer_use := peelCallDmd cd in
-        match splitProdDmd_maybe dict_dmd with
-        | Some jds =>
-            postProcessUnsat defer_use (Mk_DmdType emptyDmdEnv (cons (mkOnceUsedDmd
-                                                                      (mkProdDmd (GHC.Base.map (enhance cd') jds))) nil)
-                                                   topRes)
-        | _ => nopDmdType
-        end
-    | _, _ => Panic.panic (GHC.Base.hs_string__ "dmdTransformDictSelSig: no args")
-    end.
-
-Program Definition dmdTransformDataConSig
-           : BasicTypes.Arity -> StrictSig -> CleanDemand -> DmdType :=
-          fun arg_0__ arg_1__ arg_2__ =>
-            match arg_0__, arg_1__, arg_2__ with
-            | arity, Mk_StrictSig (Mk_DmdType _ _ con_res), JD str abs =>
-                let fix go_abs arg_3__ arg_4__
-                          := match arg_3__, arg_4__ with
-                             | num_5__, dmd =>
-                                 if Bool.Sumbool.sumbool_of_bool (num_5__ GHC.Base.== #0)
-                                 then splitUseProdDmd arity dmd else
-                                 match arg_3__, arg_4__ with
-                                 | n, UCall One u' => go_abs (n GHC.Num.- #1) u'
-                                 | _, _ => None
-                                 end
-                             end in
-                let go_str :=
-                  GHC.Wf.wfFix2 Coq.Init.Peano.lt (fun arg_10__ arg_11__ => arg_10__) _
-                                (fun arg_10__ arg_11__ go_str =>
-                                   match arg_10__, arg_11__ with
-                                   | num_12__, dmd =>
-                                       if Bool.Sumbool.sumbool_of_bool (num_12__ GHC.Base.== #0)
-                                       then splitStrProdDmd arity dmd else
-                                       match arg_10__, arg_11__ with
-                                       | n, SCall s' => go_str (n GHC.Num.- #1) s'
-                                       | n, HyperStr => go_str (n GHC.Num.- #1) HyperStr
-                                       | _, _ => None
-                                       end
-                                   end) in
-                match go_str arity str with
-                | Some str_dmds =>
-                    match go_abs arity abs with
-                    | Some abs_dmds =>
-                        Mk_DmdType emptyDmdEnv (mkJointDmds str_dmds abs_dmds) con_res
-                    | _ => nopDmdType
-                    end
-                | _ => nopDmdType
-                end
-            end.
-Solve Obligations with (solve_dmdTransform).
-
 Definition disjointVarSet : VarSet -> VarSet -> bool :=
   fun s1 s2 => UniqFM.disjointUFM (UniqSet.getUniqSet s1) (UniqSet.getUniqSet s2).
 
@@ -6922,120 +5819,6 @@ Definition deAnnBind : forall {b} {annot}, AnnBind b annot -> Bind b :=
 Definition deAnnAlt {bndr} {annot} : AnnAlt bndr annot -> Alt bndr :=
   fun '(pair (pair con args) rhs) => pair (pair con args) (deAnnotate rhs).
 
-Definition dataConWrapId_maybe : DataCon -> option Id :=
-  fun dc =>
-    match dcRep dc with
-    | NoDataConRep => None
-    | DCR wrap_id _ _ _ _ => Some wrap_id
-    end.
-
-Definition dataConWrapId : DataCon -> Id :=
-  fun dc =>
-    match dcRep dc with
-    | NoDataConRep => dcWorkId dc
-    | DCR wrap_id _ _ _ _ => wrap_id
-    end.
-
-Definition dataConWorkId : DataCon -> Id :=
-  fun dc => dcWorkId dc.
-
-Definition mkConApp {b} : DataCon -> list (Arg b) -> Expr b :=
-  fun con args => mkApps (Mk_Var (dataConWorkId con)) args.
-
-Definition mkConApp2 {b} : DataCon -> list Type_ -> list Var -> Expr b :=
-  fun con tys arg_ids =>
-    mkApps (mkApps (Mk_Var (dataConWorkId con)) (GHC.Base.map Mk_Type tys))
-           (GHC.Base.map varToCoreExpr arg_ids).
-
-Definition dataConUserTyVarBinders : DataCon -> list TyVarBinder :=
-  dcUserTyVarBinders.
-
-Definition dataConUnivTyVars : DataCon -> list TyVar :=
-  fun '(MkData _ _ _ _ tvbs _ _ _ _ _ _ _ _ _ _ _ _ _ _ _ _ _) => tvbs.
-
-Definition dataConUnivAndExTyVars : DataCon -> list TyVar :=
-  fun '(MkData _ _ _ _ univ_tvs ex_tvs _ _ _ _ _ _ _ _ _ _ _ _ _ _ _ _) =>
-    Coq.Init.Datatypes.app univ_tvs ex_tvs.
-
-Definition dataConTyCon : DataCon -> TyCon :=
-  dcRepTyCon.
-
-Definition dataConTag : DataCon -> BasicTypes.ConTag :=
-  dcTag.
-
-Definition dataConTagZ : DataCon -> BasicTypes.ConTagZ :=
-  fun con => dataConTag con GHC.Num.- BasicTypes.fIRST_TAG.
-
-Definition dataConStupidTheta : DataCon -> ThetaType :=
-  fun dc => dcStupidTheta dc.
-
-Definition dataConSrcBangs : DataCon -> list HsSrcBang :=
-  dcSrcBangs.
-
-Definition dataConSourceArity : DataCon -> BasicTypes.Arity :=
-  fun '(MkData _ _ _ _ _ _ _ _ _ _ _ _ _ _ _ _ _ arity _ _ _ _) => arity.
-
-Definition isNullarySrcDataCon : DataCon -> bool :=
-  fun dc => dataConSourceArity dc GHC.Base.== #0.
-
-Definition dataConRepType : DataCon -> Type_ :=
-  dcRepType.
-
-Definition dataConRepArity : DataCon -> BasicTypes.Arity :=
-  fun '(MkData _ _ _ _ _ _ _ _ _ _ _ _ _ _ _ _ arity _ _ _ _ _) => arity.
-
-Definition isNullaryRepDataCon : DataCon -> bool :=
-  fun dc => dataConRepArity dc GHC.Base.== #0.
-
-Definition dataConName : DataCon -> Name.Name :=
-  dcName.
-
-Definition dataConIsInfix : DataCon -> bool :=
-  dcInfix.
-
-Definition dataConImplBangs : DataCon -> list HsImplBang :=
-  fun dc =>
-    match dcRep dc with
-    | NoDataConRep => Coq.Lists.List.repeat HsLazy (dcSourceArity dc)
-    | DCR _ _ _ _ bangs => bangs
-    end.
-
-Definition dataConFullSig
-   : DataCon ->
-     (list TyVar * list TyVar * list EqSpec * ThetaType * list Type_ * Type_)%type :=
-  fun '(MkData _ _ _ _ univ_tvs ex_tvs _ eq_spec theta _ arg_tys res_ty _ _ _ _ _
-  _ _ _ _ _) =>
-    pair (pair (pair (pair (pair univ_tvs ex_tvs) eq_spec) theta) arg_tys) res_ty.
-
-Definition dataConFieldType_maybe
-   : DataCon ->
-     FieldLabel.FieldLabelString -> option (FieldLabel.FieldLabel * Type_)%type :=
-  fun con label =>
-    Data.Foldable.find ((fun arg_0__ => arg_0__ GHC.Base.== label) GHC.Base.∘
-                        (FieldLabel.flLabel GHC.Base.∘ Data.Tuple.fst)) (GHC.List.zip (dcFields con)
-                                                                                      (dcOrigArgTys con)).
-
-Definition dataConFieldLabels : DataCon -> list FieldLabel.FieldLabel :=
-  dcFields.
-
-Definition fieldsOfAlgTcRhs : AlgTyConRhs -> FieldLabel.FieldLabelEnv :=
-  fun rhs =>
-    let dataConsFields :=
-      fun dcs => Data.Foldable.concatMap dataConFieldLabels dcs in
-    FastStringEnv.mkDFsEnv (Coq.Lists.List.flat_map (fun fl =>
-                                                       cons (pair (FieldLabel.flLabel fl) fl) nil) (dataConsFields
-                                                     (visibleDataCons rhs))).
-
-Axiom dataConCannotMatch : list Type_ -> DataCon -> bool.
-
-Definition dataConBoxer : DataCon -> option unit :=
-  fun arg_0__ =>
-    match arg_0__ with
-    | MkData _ _ _ _ _ _ _ _ _ _ _ _ _ _ _ (DCR _ boxer _ _ _) _ _ _ _ _ _ =>
-        Some boxer
-    | _ => None
-    end.
-
 Definition dVarSetToVarSet : DVarSet -> VarSet :=
   UniqSet.unsafeUFMToUniqSet GHC.Base.∘ UniqDFM.udfmToUfm.
 
@@ -7050,18 +5833,6 @@ Definition dVarSetElems : DVarSet -> list Var :=
 
 Definition dVarEnvElts {a} : DVarEnv a -> list a :=
   UniqDFM.eltsUDFM.
-
-Definition cprSumRes : BasicTypes.ConTag -> DmdResult :=
-  fun tag => Dunno (RetSum tag).
-
-Definition cprProdRes : list DmdType -> DmdResult :=
-  fun _arg_tys => Dunno RetProd.
-
-Definition cprProdDmdType : BasicTypes.Arity -> DmdType :=
-  fun arity => Mk_DmdType emptyDmdEnv nil (vanillaCprProdRes arity).
-
-Definition cprProdSig : BasicTypes.Arity -> StrictSig :=
-  fun arity => Mk_StrictSig (cprProdDmdType arity).
 
 Definition collectValBinders : CoreExpr -> (list Id * CoreExpr)%type :=
   fun expr =>
@@ -7208,220 +5979,14 @@ Definition ltAlt {a} {b}
    : (AltCon * a * b)%type -> (AltCon * a * b)%type -> bool :=
   fun a1 a2 => (cmpAlt a1 a2) GHC.Base.== Lt.
 
-Definition cleanUseDmd_maybe : Demand -> option UseDmd :=
-  fun arg_0__ => match arg_0__ with | JD _ (Mk_Use _ u) => Some u | _ => None end.
-
-Definition cleanEvalProdDmd : BasicTypes.Arity -> CleanDemand :=
-  fun n => JD HeadStr (UProd (Coq.Lists.List.repeat useTop n)).
-
-Definition cleanEvalDmd : CleanDemand :=
-  JD HeadStr Used.
-
-Definition classTvsFds : Class -> (list TyVar * list (FunDep TyVar))%type :=
-  fun c => pair (classTyVars c) (classFunDeps c).
-
-Definition classSCTheta : Class -> list PredType :=
-  fun arg_0__ =>
-    match arg_0__ with
-    | Mk_Class _ _ _ _ _ (ConcreteClass theta_stuff _ _ _ _) => theta_stuff
-    | _ => nil
-    end.
-
-Definition classOpItems : Class -> list ClassOpItem :=
-  fun arg_0__ =>
-    match arg_0__ with
-    | Mk_Class _ _ _ _ _ (ConcreteClass _ _ _ op_stuff _) => op_stuff
-    | _ => nil
-    end.
-
-Definition classMinimalDef : Class -> ClassMinimalDef :=
-  fun arg_0__ =>
-    match arg_0__ with
-    | Mk_Class _ _ _ _ _ (ConcreteClass _ _ _ _ d) => d
-    | _ => BooleanFormula.mkTrue
-    end.
-
-Definition classMethods : Class -> list Id :=
-  fun arg_0__ =>
-    match arg_0__ with
-    | Mk_Class _ _ _ _ _ (ConcreteClass _ _ _ op_stuff _) =>
-        let cont_1__ arg_2__ := let 'pair op_sel _ := arg_2__ in cons op_sel nil in
-        Coq.Lists.List.flat_map cont_1__ op_stuff
-    | _ => nil
-    end.
-
-Definition classHasFds : Class -> bool :=
-  fun '(Mk_Class _ _ _ _ fds _) => negb (Data.Foldable.null fds).
-
-Definition classExtraBigSig
-   : Class ->
-     (list TyVar * list (FunDep TyVar) * list PredType * list Id * list ClassATItem *
-      list ClassOpItem)%type :=
-  fun arg_0__ =>
-    match arg_0__ with
-    | Mk_Class _ _ _ tyvars fundeps AbstractClass =>
-        pair (pair (pair (pair (pair tyvars fundeps) nil) nil) nil) nil
-    | Mk_Class _ _ _ tyvars fundeps (ConcreteClass sc_theta sc_sels ats op_stuff
-     _) =>
-        pair (pair (pair (pair (pair tyvars fundeps) sc_theta) sc_sels) ats) op_stuff
-    end.
-
-Definition classBigSig
-   : Class -> (list TyVar * list PredType * list Id * list ClassOpItem)%type :=
-  fun arg_0__ =>
-    match arg_0__ with
-    | Mk_Class _ _ _ tyvars _ AbstractClass => pair (pair (pair tyvars nil) nil) nil
-    | Mk_Class _ _ _ tyvars _ (ConcreteClass sc_theta sc_sels _ op_stuff _) =>
-        pair (pair (pair tyvars sc_theta) sc_sels) op_stuff
-    end.
-
-Definition classArity : Class -> BasicTypes.Arity :=
-  fun clas => Coq.Lists.List.length (classTyVars clas).
-
-Definition classAllSelIds : Class -> list Id :=
-  fun arg_0__ =>
-    match arg_0__ with
-    | (Mk_Class _ _ _ _ _ (ConcreteClass _ sc_sels _ _ _) as c) =>
-        Coq.Init.Datatypes.app sc_sels (classMethods c)
-    | c =>
-        if andb Util.debugIsOn (negb (Data.Foldable.null (classMethods c))) : bool
-        then (Panic.assertPanic (GHC.Base.hs_string__ "ghc/compiler/types/Class.hs")
-              #244)
-        else nil
-    end.
-
-Definition classATs : Class -> list TyCon :=
-  fun arg_0__ =>
-    match arg_0__ with
-    | Mk_Class _ _ _ _ _ (ConcreteClass _ _ at_stuff _ _) =>
-        let cont_1__ arg_2__ := let 'ATI tc _ := arg_2__ in cons tc nil in
-        Coq.Lists.List.flat_map cont_1__ at_stuff
-    | _ => nil
-    end.
-
-Definition classATItems : Class -> list ClassATItem :=
-  fun arg_0__ =>
-    match arg_0__ with
-    | Mk_Class _ _ _ _ _ (ConcreteClass _ _ at_stuff _ _) => at_stuff
-    | _ => nil
-    end.
-
 Definition chooseOrphanAnchor (local_names : list Name.Name) : IsOrphan :=
   match GHC.Base.map Name.nameOccName local_names with
   | cons hd tl => NotOrphan (Data.Foldable.foldr GHC.Base.min hd tl)
   | nil => Mk_IsOrphan
   end.
 
-Definition checkRecTc : RecTcChecker -> TyCon -> option RecTcChecker :=
-  fun arg_0__ arg_1__ =>
-    match arg_0__, arg_1__ with
-    | RC bound rec_nts, tc =>
-        let tc_name := tyConName tc in
-        match NameEnv.lookupNameEnv rec_nts tc_name with
-        | Some n =>
-            if n GHC.Base.>= bound : bool then None else
-            Some (RC bound (NameEnv.extendNameEnv rec_nts tc_name (n GHC.Num.+ #1)))
-        | None => Some (RC bound (NameEnv.extendNameEnv rec_nts tc_name #1))
-        end
-    end.
-
-Definition catchArgDmd : Demand :=
-  JD (Mk_Str Mk_ExnStr (SCall HeadStr)) (Mk_Use One (UCall One Used)).
-
 Definition canUnfold : Unfolding -> bool :=
   fun arg_0__ => false.
-
-Axiom bothUse : UseDmd -> UseDmd -> UseDmd.
-
-Definition bothExnStr : ExnStr -> ExnStr -> ExnStr :=
-  fun arg_0__ arg_1__ =>
-    match arg_0__, arg_1__ with
-    | Mk_ExnStr, Mk_ExnStr => Mk_ExnStr
-    | _, _ => VanStr
-    end.
-
-Definition bothStr : StrDmd -> StrDmd -> StrDmd :=
-  fix bothStr (arg_0__ arg_1__ : StrDmd) : StrDmd
-        := let bothArgStr (arg_0__ arg_1__ : ArgStr) : ArgStr :=
-             match arg_0__, arg_1__ with
-             | Lazy, s => s
-             | s, Lazy => s
-             | Mk_Str x1 s1, Mk_Str x2 s2 => Mk_Str (bothExnStr x1 x2) (bothStr s1 s2)
-             end in
-           match arg_0__, arg_1__ with
-           | HyperStr, _ => HyperStr
-           | HeadStr, s => s
-           | SCall _, HyperStr => HyperStr
-           | SCall s1, HeadStr => SCall s1
-           | SCall s1, SCall s2 => SCall (bothStr s1 s2)
-           | SCall _, SProd _ => HyperStr
-           | SProd _, HyperStr => HyperStr
-           | SProd s1, HeadStr => SProd s1
-           | SProd s1, SProd s2 =>
-               if Util.equalLength s1 s2 : bool
-               then mkSProd (GHC.List.zipWith bothArgStr s1 s2) else
-               HyperStr
-           | SProd _, SCall _ => HyperStr
-           end.
-
-Definition bothDmdResult : DmdResult -> Termination unit -> DmdResult :=
-  fun arg_0__ arg_1__ =>
-    match arg_0__, arg_1__ with
-    | _, Diverges => Diverges
-    | r, ThrowsExn => match r with | Diverges => r | _ => ThrowsExn end
-    | r, Dunno _ => r
-    end.
-
-Definition bothCleanDmd : CleanDemand -> CleanDemand -> CleanDemand :=
-  fun arg_0__ arg_1__ =>
-    match arg_0__, arg_1__ with
-    | JD s1 a1, JD s2 a2 => JD (bothStr s1 s2) (bothUse a1 a2)
-    end.
-
-Axiom bothArgUse : ArgUse -> ArgUse -> ArgUse.
-
-Definition bothArgStr : ArgStr -> ArgStr -> ArgStr :=
-  fun arg_0__ arg_1__ =>
-    match arg_0__, arg_1__ with
-    | Lazy, s => s
-    | s, Lazy => s
-    | Mk_Str x1 s1, Mk_Str x2 s2 => Mk_Str (bothExnStr x1 x2) (bothStr s1 s2)
-    end.
-
-Definition bothDmd : Demand -> Demand -> Demand :=
-  fun arg_0__ arg_1__ =>
-    match arg_0__, arg_1__ with
-    | JD s1 a1, JD s2 a2 => JD (bothArgStr s1 s2) (bothArgUse a1 a2)
-    end.
-
-Definition botRes : DmdResult :=
-  Diverges.
-
-Definition botDmdType : DmdType :=
-  Mk_DmdType emptyDmdEnv nil botRes.
-
-Definition botSig : StrictSig :=
-  Mk_StrictSig botDmdType.
-
-Definition ensureArgs : BasicTypes.Arity -> DmdType -> DmdType :=
-  fun n d =>
-    let 'Mk_DmdType fv ds r := d in
-    let ds' :=
-      Coq.Lists.List.firstn n (app ds (Coq.Lists.List.repeat (resTypeArgDmd r) n)) in
-    let r' := match r with | Dunno _ => topRes | _ => r end in
-    let depth := dmdTypeDepth d in
-    if n GHC.Base.== depth : bool then d else
-    Mk_DmdType fv ds' r'.
-
-Definition removeDmdTyArgs : DmdType -> DmdType :=
-  ensureArgs #0.
-
-Definition splitDmdTy : DmdType -> (Demand * DmdType)%type :=
-  fun arg_0__ =>
-    match arg_0__ with
-    | Mk_DmdType fv (cons dmd dmds) res_ty => pair dmd (Mk_DmdType fv dmds res_ty)
-    | (Mk_DmdType _ nil res_ty as ty) => pair (resTypeArgDmd res_ty) ty
-    end.
 
 Definition boringCxtOk : bool :=
   true.
@@ -7448,135 +6013,11 @@ Definition binderVar {tv} {argf} : TyVarBndr tv argf -> tv :=
 Definition binderVars {tv} {argf} : list (TyVarBndr tv argf) -> list tv :=
   fun tvbs => GHC.Base.map binderVar tvbs.
 
-Definition dataConUserTyVars : DataCon -> list TyVar :=
-  fun '(MkData _ _ _ _ _ _ tvbs _ _ _ _ _ _ _ _ _ _ _ _ _ _ _) => binderVars tvbs.
-
-Definition dataConUserTyVarsArePermuted : DataCon -> bool :=
-  fun '(MkData _ _ _ _ univ_tvs ex_tvs user_tvbs eq_spec _ _ _ _ _ _ _ _ _ _ _ _ _
-  _) =>
-    (Coq.Init.Datatypes.app (filterEqSpec eq_spec univ_tvs) ex_tvs) GHC.Base./=
-    binderVars user_tvbs.
-
-Definition mkAlgTyCon
-   : Name.Name ->
-     list TyConBinder ->
-     Kind ->
-     list Role ->
-     option unit -> list PredType -> AlgTyConRhs -> AlgTyConFlav -> bool -> TyCon :=
-  fun name binders res_kind roles cType stupid rhs parent gadt_syn =>
-    AlgTyCon (Name.nameUnique name) name binders (binderVars binders) res_kind
-             (mkTyConKind binders res_kind) (Coq.Lists.List.length binders) roles cType
-             gadt_syn stupid rhs (fieldsOfAlgTcRhs rhs) (if andb Util.debugIsOn (negb
-                                                                  (okParent name parent)) : bool
-              then (GHC.Err.error Panic.someSDoc)
-              else parent).
-
-Definition mkClassTyCon
-   : Name.Name ->
-     list TyConBinder -> list Role -> AlgTyConRhs -> Class -> Name.Name -> TyCon :=
-  fun name binders roles rhs clas tc_rep_name =>
-    mkAlgTyCon name binders constraintKind roles None nil rhs (ClassTyCon clas
-                                                               tc_rep_name) false.
-
-Definition mkFamilyTyCon
-   : Name.Name ->
-     list TyConBinder ->
-     Kind ->
-     option Name.Name -> FamTyConFlav -> option Class -> Injectivity -> TyCon :=
-  fun name binders res_kind resVar flav parent inj =>
-    FamilyTyCon (Name.nameUnique name) name binders (binderVars binders) res_kind
-                (mkTyConKind binders res_kind) (Coq.Lists.List.length binders) resVar flav
-                parent inj.
-
-Definition mkSynonymTyCon
-   : Name.Name ->
-     list TyConBinder -> Kind -> list Role -> Type_ -> bool -> bool -> TyCon :=
-  fun name binders res_kind roles rhs is_tau is_fam_free =>
-    SynonymTyCon (Name.nameUnique name) name binders (binderVars binders) res_kind
-                 (mkTyConKind binders res_kind) (Coq.Lists.List.length binders) roles rhs is_tau
-                 is_fam_free.
-
-Definition mkTcTyCon
-   : Name.Name ->
-     list TyConBinder ->
-     Kind -> list (Name.Name * TyVar)%type -> TyConFlavour -> TyCon :=
-  fun name binders res_kind scoped_tvs flav =>
-    TcTyCon (Unique.getUnique name) name binders (binderVars binders) res_kind
-            (mkTyConKind binders res_kind) (Coq.Lists.List.length binders) scoped_tvs flav.
-
-Definition makeRecoveryTyCon : TyCon -> TyCon :=
-  fun tc =>
-    mkTcTyCon (tyConName tc) (tyConBinders tc) (tyConResKind tc) nil (tyConFlavour
-                                                                      tc).
-
-Definition mkTupleTyCon
-   : Name.Name ->
-     list TyConBinder ->
-     Kind ->
-     BasicTypes.Arity -> DataCon -> BasicTypes.TupleSort -> AlgTyConFlav -> TyCon :=
-  fun name binders res_kind arity con sort parent =>
-    AlgTyCon (Name.nameUnique name) name binders (binderVars binders) res_kind
-             (mkTyConKind binders res_kind) arity (Coq.Lists.List.repeat Representational
-                                                                         arity) None false nil (TupleTyCon con sort)
-             FastStringEnv.emptyDFsEnv parent.
-
-Definition patSynExTyVars : PatSyn -> list TyVar :=
-  fun ps => binderVars (psExTyVars ps).
-
-Definition patSynSig
-   : PatSyn ->
-     (list TyVar * ThetaType * list TyVar * ThetaType * list Type_ * Type_)%type :=
-  fun '(MkPatSyn _ _ arg_tys _ _ _ univ_tvs req ex_tvs prov res_ty _ _) =>
-    pair (pair (pair (pair (pair (binderVars univ_tvs) req) (binderVars ex_tvs))
-                     prov) arg_tys) res_ty.
-
 Definition binderKind {argf} : TyVarBndr TyVar argf -> Kind :=
   fun '(TvBndr tv _) => tyVarKind tv.
 
 Definition binderArgFlag {tv} {argf} : TyVarBndr tv argf -> argf :=
   fun '(TvBndr _ argf) => argf.
-
-Definition argOneShots : Demand -> list BasicTypes.OneShotInfo :=
-  fun '(JD _ usg) =>
-    let fix go arg_1__
-              := match arg_1__ with
-                 | UCall One u => cons BasicTypes.OneShotLam (go u)
-                 | UCall Many u => cons BasicTypes.NoOneShotInfo (go u)
-                 | _ => nil
-                 end in
-    match usg with
-    | Mk_Use _ arg_usg => go arg_usg
-    | _ => nil
-    end.
-
-Definition argsOneShots
-   : StrictSig -> BasicTypes.Arity -> list (list BasicTypes.OneShotInfo) :=
-  fun arg_0__ arg_1__ =>
-    match arg_0__, arg_1__ with
-    | Mk_StrictSig (Mk_DmdType _ arg_ds _), n_val_args =>
-        let cons_ :=
-          fun arg_2__ arg_3__ =>
-            match arg_2__, arg_3__ with
-            | nil, nil => nil
-            | a, as_ => cons a as_
-            end in
-        let fix go arg_6__
-                  := match arg_6__ with
-                     | nil => nil
-                     | cons arg_d arg_ds => cons_ (argOneShots arg_d) (go arg_ds)
-                     end in
-        let unsaturated_call := Util.lengthExceeds arg_ds n_val_args in
-        if unsaturated_call : bool then nil else
-        go arg_ds
-    end.
-
-Definition appIsBottom : StrictSig -> nat -> bool :=
-  fun arg_0__ arg_1__ =>
-    match arg_0__, arg_1__ with
-    | Mk_StrictSig (Mk_DmdType _ ds res), n =>
-        if isBotRes res : bool then negb (Util.lengthExceeds ds n) else
-        false
-    end.
 
 Definition anyVarSet : (Var -> bool) -> VarSet -> bool :=
   UniqSet.uniqSetAny.
@@ -7593,69 +6034,11 @@ Definition allVarSet : (Var -> bool) -> VarSet -> bool :=
 Definition allDVarSet : (Var -> bool) -> DVarSet -> bool :=
   UniqDFM.allUDFM.
 
-Definition algTyConRhs : TyCon -> AlgTyConRhs :=
-  fun arg_0__ =>
-    match arg_0__ with
-    | AlgTyCon _ _ _ _ _ _ _ _ _ _ _ rhs _ _ => rhs
-    | other => Panic.panicStr (GHC.Base.hs_string__ "algTyConRhs") (Panic.someSDoc)
-    end.
-
 Definition addRnInScopeSet : RnEnv2 -> VarSet -> RnEnv2 :=
   fun env vs =>
     if isEmptyVarSet vs : bool then env else
     let 'RV2 envL_0__ envR_1__ in_scope_2__ := env in
     RV2 envL_0__ envR_1__ (extendInScopeSetSet (in_scope env) vs).
-
-Definition addDemand : Demand -> DmdType -> DmdType :=
-  fun arg_0__ arg_1__ =>
-    match arg_0__, arg_1__ with
-    | dmd, Mk_DmdType fv ds res => Mk_DmdType fv (cons dmd ds) res
-    end.
-
-Definition absDmd : Demand :=
-  JD Lazy Abs.
-
-Definition defaultDmd {r} : Termination r -> Demand :=
-  fun arg_0__ => match arg_0__ with | Dunno _ => absDmd | _ => botDmd end.
-
-Definition bothDmdType : DmdType -> BothDmdArg -> DmdType :=
-  fun arg_0__ arg_1__ =>
-    match arg_0__, arg_1__ with
-    | Mk_DmdType fv1 ds1 r1, pair fv2 t2 =>
-        Mk_DmdType (plusVarEnv_CD bothDmd fv1 (defaultDmd r1) fv2 (defaultDmd t2)) ds1
-        (bothDmdResult r1 t2)
-    end.
-
-Definition findIdDemand : DmdType -> Var -> Demand :=
-  fun arg_0__ arg_1__ =>
-    match arg_0__, arg_1__ with
-    | Mk_DmdType fv _ res, id => Maybes.orElse (lookupVarEnv fv id) (defaultDmd res)
-    end.
-
-Definition lubDmdType : DmdType -> DmdType -> DmdType :=
-  fun d1 d2 =>
-    let n := GHC.Base.max (dmdTypeDepth d1) (dmdTypeDepth d2) in
-    let 'Mk_DmdType fv1 ds1 r1 := ensureArgs n d1 in
-    let 'Mk_DmdType fv2 ds2 r2 := ensureArgs n d2 in
-    let lub_fv := plusVarEnv_CD lubDmd fv1 (defaultDmd r1) fv2 (defaultDmd r2) in
-    let lub_ds :=
-      Util.zipWithEqual (GHC.Base.hs_string__ "lubDmdType") lubDmd ds1 ds2 in
-    let lub_res := lubDmdResult r1 r2 in Mk_DmdType lub_fv lub_ds lub_res.
-
-Definition deferAfterIO : DmdType -> DmdType :=
-  fun '((Mk_DmdType _ _ res as d)) =>
-    let defer_res :=
-      fun arg_1__ => match arg_1__ with | (Dunno _ as r) => r | _ => topRes end in
-    let 'Mk_DmdType fv ds _ := lubDmdType d nopDmdType in
-    Mk_DmdType fv ds (defer_res res).
-
-Definition peelFV : DmdType -> Var -> (DmdType * Demand)%type :=
-  fun arg_0__ arg_1__ =>
-    match arg_0__, arg_1__ with
-    | Mk_DmdType fv ds res, id =>
-        let dmd := Maybes.orElse (lookupVarEnv fv id) (defaultDmd res) in
-        let fv' := delVarEnv fv id in pair (Mk_DmdType fv' ds res) dmd
-    end.
 
 (* Skipping all instances of class `Outputable.Outputable', including
    `Core.Outputable__InScopeSet' *)
@@ -8875,51 +7258,40 @@ Program Instance Eq___Class : GHC.Base.Eq_ Class :=
            GHC.Base.op_zsze____ := Eq___Class_op_zsze__ |}.
 
 (* External variables:
-     Bool.Sumbool.sumbool_of_bool BranchIndex Branched BuiltInSynFamily CoAxBranch
-     CoAxiom CoAxiomRule Coercion Eq Gt Kind Literal Lt Nominal None PredType
-     Representational Role Some ThetaType TyBinder TyThing Type Type_ Unbranched andb
-     app bool comparison cons constraintKind false liftedTypeKind list mkMachChar
-     mkMachDouble mkMachFloat mkMachString nat negb nil op_zt__ option orb pair
-     size_AnnExpr' snd true tt unit BasicTypes.Activation BasicTypes.AlwaysActive
-     BasicTypes.Arity BasicTypes.Boxity BasicTypes.ConTag BasicTypes.ConTagZ
-     BasicTypes.DefMethSpec BasicTypes.IAmALoopBreaker BasicTypes.IAmDead
-     BasicTypes.InlinePragma BasicTypes.JoinArity BasicTypes.LeftOrRight
-     BasicTypes.ManyOccs BasicTypes.NoOneShotInfo BasicTypes.NoTailCallInfo
-     BasicTypes.OccInfo BasicTypes.OneOcc BasicTypes.OneShotInfo
-     BasicTypes.OneShotLam BasicTypes.RuleName BasicTypes.SourceText
-     BasicTypes.TupleSort BasicTypes.TyPrec BasicTypes.defaultInlinePragma
-     BasicTypes.fIRST_TAG BasicTypes.isAlwaysTailCalled BasicTypes.isBoxed
-     BasicTypes.noOccInfo BasicTypes.tupleSortBoxity BasicTypes.zapFragileOcc
-     BinNat.N.of_nat BinNums.N BooleanFormula.BooleanFormula BooleanFormula.mkTrue
-     Coq.Init.Datatypes.app Coq.Init.Peano.lt Coq.Lists.List.firstn
-     Coq.Lists.List.flat_map Coq.Lists.List.length Coq.Lists.List.repeat
-     Coq.Lists.List.skipn Data.Foldable.all Data.Foldable.any Data.Foldable.concatMap
-     Data.Foldable.find Data.Foldable.foldl Data.Foldable.foldr Data.Foldable.null
-     Data.Function.on Data.Maybe.isJust Data.Tuple.fst Datatypes.id DynFlags.DynFlags
-     DynFlags.Opt_KillAbsence DynFlags.Opt_KillOneShot DynFlags.gopt
-     FastString.FastString FastStringEnv.dFsEnvElts FastStringEnv.emptyDFsEnv
-     FastStringEnv.lookupDFsEnv FastStringEnv.mkDFsEnv FieldLabel.FieldLabel
-     FieldLabel.FieldLabelEnv FieldLabel.FieldLabelString FieldLabel.flLabel
-     GHC.Base.Eq_ GHC.Base.Monad GHC.Base.Ord GHC.Base.String GHC.Base.compare
-     GHC.Base.compare__ GHC.Base.eq_default GHC.Base.fmap GHC.Base.map
-     GHC.Base.mappend GHC.Base.max GHC.Base.max__ GHC.Base.min GHC.Base.min__
-     GHC.Base.op_z2218U__ GHC.Base.op_zeze__ GHC.Base.op_zeze____ GHC.Base.op_zg__
-     GHC.Base.op_zg____ GHC.Base.op_zgze__ GHC.Base.op_zgze____ GHC.Base.op_zgzgze__
-     GHC.Base.op_zl__ GHC.Base.op_zl____ GHC.Base.op_zlze__ GHC.Base.op_zlze____
-     GHC.Base.op_zsze__ GHC.Base.op_zsze____ GHC.Base.return_ GHC.Char.Char
-     GHC.DeferredFix.deferredFix1 GHC.DeferredFix.deferredFix2 GHC.Err.Build_Default
-     GHC.Err.Default GHC.Err.default GHC.Err.error GHC.List.filter GHC.List.reverse
-     GHC.List.zip GHC.List.zipWith GHC.Num.Integer GHC.Num.fromInteger
-     GHC.Num.op_zm__ GHC.Num.op_zp__ GHC.Num.op_zt__ GHC.Prim.coerce GHC.Prim.seq
-     GHC.Real.Rational GHC.Wf.wfFix1 GHC.Wf.wfFix2 GHC.Wf.wfFix3 Maybes.orElse
-     Module.Module Module.ModuleSet Module.emptyModuleSet Module.mkModuleSet
-     Name.Name Name.NamedThing Name.getName__ Name.getOccName__ Name.isWiredInName
-     Name.mkExternalName Name.nameModule Name.nameOccName Name.nameSrcSpan
-     Name.nameUnique Name.setNameUnique NameEnv.NameEnv NameEnv.emptyNameEnv
-     NameEnv.extendNameEnv NameEnv.lookupNameEnv OccName.HasOccName OccName.OccName
-     OccName.TidyOccEnv OccName.emptyTidyOccEnv OccName.isTcOcc OccName.mkTyConRepOcc
-     OccName.occName__ Pair.Pair Panic.assertPanic Panic.panic Panic.panicStr
-     Panic.someSDoc Panic.warnPprTrace PrelNames.gHC_PRIM PrelNames.gHC_TYPES
+     BranchIndex Branched BuiltInSynFamily CoAxBranch CoAxiom CoAxiomRule Coercion Eq
+     Gt Kind Literal Lt None PredType Role Some ThetaType TyBinder TyThing Type Type_
+     Unbranched andb bool comparison cons false list mkMachChar mkMachDouble
+     mkMachFloat mkMachString nat negb nil op_zt__ option orb pair size_AnnExpr' snd
+     true tt unit BasicTypes.Activation BasicTypes.AlwaysActive BasicTypes.Arity
+     BasicTypes.Boxity BasicTypes.ConTag BasicTypes.ConTagZ BasicTypes.DefMethSpec
+     BasicTypes.IAmALoopBreaker BasicTypes.IAmDead BasicTypes.InlinePragma
+     BasicTypes.JoinArity BasicTypes.LeftOrRight BasicTypes.ManyOccs
+     BasicTypes.NoOneShotInfo BasicTypes.NoTailCallInfo BasicTypes.OccInfo
+     BasicTypes.OneOcc BasicTypes.OneShotInfo BasicTypes.RuleName
+     BasicTypes.SourceText BasicTypes.TupleSort BasicTypes.TyPrec
+     BasicTypes.defaultInlinePragma BasicTypes.isAlwaysTailCalled
+     BasicTypes.noOccInfo BasicTypes.zapFragileOcc BinNat.N.of_nat BinNums.N
+     BooleanFormula.BooleanFormula Coq.Init.Datatypes.app Coq.Init.Peano.lt
+     Coq.Lists.List.flat_map Coq.Lists.List.length Data.Foldable.foldl
+     Data.Foldable.foldr Data.Function.on Data.Tuple.fst Datatypes.id
+     DynFlags.DynFlags FastString.FastString FieldLabel.FieldLabel
+     FieldLabel.FieldLabelEnv FieldLabel.FieldLabelString GHC.Base.Eq_ GHC.Base.Monad
+     GHC.Base.Ord GHC.Base.String GHC.Base.compare GHC.Base.compare__
+     GHC.Base.eq_default GHC.Base.map GHC.Base.mappend GHC.Base.max__ GHC.Base.min
+     GHC.Base.min__ GHC.Base.op_z2218U__ GHC.Base.op_zeze__ GHC.Base.op_zeze____
+     GHC.Base.op_zg__ GHC.Base.op_zg____ GHC.Base.op_zgze__ GHC.Base.op_zgze____
+     GHC.Base.op_zgzgze__ GHC.Base.op_zl__ GHC.Base.op_zl____ GHC.Base.op_zlze__
+     GHC.Base.op_zlze____ GHC.Base.op_zsze__ GHC.Base.op_zsze____ GHC.Base.return_
+     GHC.Char.Char GHC.DeferredFix.deferredFix1 GHC.DeferredFix.deferredFix2
+     GHC.Err.Build_Default GHC.Err.Default GHC.Err.default GHC.Err.error
+     GHC.List.reverse GHC.Num.Integer GHC.Num.fromInteger GHC.Num.op_zm__
+     GHC.Num.op_zp__ GHC.Num.op_zt__ GHC.Prim.coerce GHC.Prim.seq GHC.Real.Rational
+     GHC.Wf.wfFix2 GHC.Wf.wfFix3 Maybes.orElse Module.Module Module.ModuleSet
+     Module.emptyModuleSet Module.mkModuleSet Name.Name Name.NamedThing
+     Name.getName__ Name.getOccName__ Name.nameOccName Name.nameUnique
+     Name.setNameUnique NameEnv.NameEnv NameEnv.emptyNameEnv OccName.HasOccName
+     OccName.OccName OccName.TidyOccEnv OccName.emptyTidyOccEnv OccName.occName__
+     Pair.Pair Panic.assertPanic Panic.panicStr Panic.someSDoc Panic.warnPprTrace
      SrcLoc.RealSrcSpan SrcLoc.SrcSpan UniqDFM.UniqDFM UniqDFM.addListToUDFM
      UniqDFM.addToUDFM UniqDFM.addToUDFM_C UniqDFM.allUDFM UniqDFM.alterUDFM
      UniqDFM.anyUDFM UniqDFM.delFromUDFM UniqDFM.delListFromUDFM UniqDFM.disjointUDFM
@@ -8941,21 +7313,18 @@ Program Instance Eq___Class : GHC.Base.Eq_ Class :=
      UniqFM.emptyUFM UniqFM.filterUFM UniqFM.filterUFM_Directly UniqFM.intersectUFM
      UniqFM.isNullUFM UniqFM.listToUFM UniqFM.listToUFM_Directly UniqFM.lookupUFM
      UniqFM.lookupUFM_Directly UniqFM.lookupWithDefaultUFM UniqFM.mapUFM
-     UniqFM.minusUFM UniqFM.nonDetFoldUFM_Directly UniqFM.nonDetUFMToList
-     UniqFM.partitionUFM UniqFM.plusMaybeUFM_C UniqFM.plusUFM UniqFM.plusUFMList
-     UniqFM.plusUFM_C UniqFM.plusUFM_CD UniqFM.unitUFM UniqSet.UniqSet
-     UniqSet.addListToUniqSet UniqSet.addOneToUniqSet UniqSet.delListFromUniqSet
-     UniqSet.delOneFromUniqSet UniqSet.delOneFromUniqSet_Directly
-     UniqSet.elemUniqSet_Directly UniqSet.elementOfUniqSet UniqSet.emptyUniqSet
-     UniqSet.filterUniqSet UniqSet.getUniqSet UniqSet.intersectUniqSets
-     UniqSet.isEmptyUniqSet UniqSet.lookupUniqSet UniqSet.lookupUniqSet_Directly
-     UniqSet.minusUniqSet UniqSet.mkUniqSet UniqSet.sizeUniqSet
-     UniqSet.unionManyUniqSets UniqSet.unionUniqSets UniqSet.uniqSetAll
-     UniqSet.uniqSetAny UniqSet.unitUniqSet UniqSet.unsafeUFMToUniqSet
-     UniqSupply.UniqSupply Unique.Uniquable Unique.Unique Unique.dataConRepNameUnique
+     UniqFM.minusUFM UniqFM.nonDetUFMToList UniqFM.partitionUFM UniqFM.plusMaybeUFM_C
+     UniqFM.plusUFM UniqFM.plusUFMList UniqFM.plusUFM_C UniqFM.plusUFM_CD
+     UniqFM.unitUFM UniqSet.UniqSet UniqSet.addListToUniqSet UniqSet.addOneToUniqSet
+     UniqSet.delListFromUniqSet UniqSet.delOneFromUniqSet
+     UniqSet.delOneFromUniqSet_Directly UniqSet.elemUniqSet_Directly
+     UniqSet.elementOfUniqSet UniqSet.emptyUniqSet UniqSet.filterUniqSet
+     UniqSet.getUniqSet UniqSet.intersectUniqSets UniqSet.isEmptyUniqSet
+     UniqSet.lookupUniqSet UniqSet.lookupUniqSet_Directly UniqSet.minusUniqSet
+     UniqSet.mkUniqSet UniqSet.sizeUniqSet UniqSet.unionManyUniqSets
+     UniqSet.unionUniqSets UniqSet.uniqSetAll UniqSet.uniqSetAny UniqSet.unitUniqSet
+     UniqSet.unsafeUFMToUniqSet UniqSupply.UniqSupply Unique.Uniquable Unique.Unique
      Unique.deriveUnique Unique.getKey Unique.getUnique Unique.getUnique__
-     Unique.mkUniqueGrimily Unique.nonDetCmpUnique Unique.tyConRepNameUnique
-     Util.HasDebugCallStack Util.count Util.debugIsOn Util.equalLength Util.foldl2
-     Util.lengthAtLeast Util.lengthAtMost Util.lengthExceeds Util.lengthIs
-     Util.listLengthCmp Util.zipEqual Util.zipWithEqual
+     Unique.mkUniqueGrimily Unique.nonDetCmpUnique Util.HasDebugCallStack Util.count
+     Util.debugIsOn Util.foldl2 Util.zipEqual
 *)
